starting over

dev/lf/dot_rec.v
@@ -17,16 +17,9 @@ Inductive label: Set :=
 | label_typ: typ_label -> label
 | label_trm: trm_label -> label.
 
-Inductive fvar : Set :=
-| in_sto : var -> fvar
-| in_ctx : var -> fvar.
-
 Inductive avar : Set :=
-  | avar_b : nat -> avar
-  | avar_f : fvar -> avar.
-
-Definition avar_s x := avar_f (in_sto x).
-Definition avar_c x := avar_f (in_ctx x).
+  | avar_b : nat -> avar  (* bound var (de Bruijn index) *)
+  | avar_f : var -> avar. (* free var ("name"), refers to store or ctx *)
 
 Inductive typ : Set :=
   | typ_top  : typ
@@ -90,13 +83,13 @@ Definition defs_hasnt(ds: defs)(l: label) := get_def l ds = None.
 (** Opening replaces in some syntax a bound variable with dangling index (k)
    by a free variable x. *)
 
-Definition open_rec_avar (k: nat) (u: fvar) (a: avar) : avar :=
+Definition open_rec_avar (k: nat) (u: var) (a: avar) : avar :=
   match a with
   | avar_b i => If k = i then avar_f u else avar_b i
-  | avar_f v => avar_f v
+  | avar_f x => avar_f x
   end.
 
-Fixpoint open_rec_typ (k: nat) (u: fvar) (T: typ): typ :=
+Fixpoint open_rec_typ (k: nat) (u: var) (T: typ): typ :=
   match T with
   | typ_top        => typ_top
   | typ_bot        => typ_bot
@@ -106,13 +99,13 @@ Fixpoint open_rec_typ (k: nat) (u: fvar) (T: typ): typ :=
   | typ_bnd T      => typ_bnd (open_rec_typ (S k) u T)
   | typ_all T1 T2  => typ_all (open_rec_typ k u T1) (open_rec_typ (S k) u T2)
   end
-with open_rec_dec (k: nat) (u: fvar) (D: dec): dec :=
+with open_rec_dec (k: nat) (u: var) (D: dec): dec :=
   match D with
   | dec_typ L T U => dec_typ L (open_rec_typ k u T) (open_rec_typ k u U)
   | dec_trm m T => dec_trm m (open_rec_typ k u T)
   end.
 
-Fixpoint open_rec_trm (k: nat) (u: fvar) (t: trm): trm :=
+Fixpoint open_rec_trm (k: nat) (u: var) (t: trm): trm :=
   match t with
   | trm_var a      => trm_var (open_rec_avar k u a)
   | trm_val v      => trm_val (open_rec_val k u v)
@@ -120,17 +113,17 @@ Fixpoint open_rec_trm (k: nat) (u: fvar) (t: trm): trm :=
   | trm_app f a    => trm_app (open_rec_avar k u f) (open_rec_avar k u a)
   | trm_let t1 t2  => trm_let (open_rec_trm k u t1) (open_rec_trm (S k) u t2)
   end
-with open_rec_val (k: nat) (u: fvar) (v: val): val :=
+with open_rec_val (k: nat) (u: var) (v: val): val :=
   match v with
   | val_new T ds => val_new (open_rec_typ (S k) u T) (open_rec_defs (S k) u ds)
   | val_lambda T e => val_lambda (open_rec_typ k u T) (open_rec_trm (S k) u e)
   end
-with open_rec_def (k: nat) (u: fvar) (d: def): def :=
+with open_rec_def (k: nat) (u: var) (d: def): def :=
   match d with
   | def_typ L T => def_typ L (open_rec_typ k u T)
   | def_trm m e => def_trm m (open_rec_trm k u e)
   end
-with open_rec_defs (k: nat) (u: fvar) (ds: defs): defs :=
+with open_rec_defs (k: nat) (u: var) (ds: defs): defs :=
   match ds with
   | defs_nil => defs_nil
   | defs_cons tl d => defs_cons (open_rec_defs k u tl) (open_rec_def k u d)
@@ -147,18 +140,10 @@ Definition open_defs u l := open_rec_defs  0 u l.
 (* ###################################################################### *)
 (** ** Free variables *)
 
-Definition var_of (v: fvar): var :=
-  match v with
-  | in_sto x => x
-  | in_ctx x => x
-  end.
-
-Definition fv_fvar (v: fvar) : vars := \{var_of v}.
-
 Definition fv_avar (a: avar) : vars :=
   match a with
   | avar_b i => \{}
-  | avar_f v => fv_fvar v
+  | avar_f x => \{x}
   end.
 
 Fixpoint fv_typ (T: typ) : vars :=
@@ -202,7 +187,6 @@ with fv_defs(ds: defs) : vars :=
   end.
 
 Definition fv_ctx_types(G: ctx): vars := (fv_in_values (fun T => fv_typ T) G).
-Definition fv_sto_vals(s: sto): vars := (fv_in_values (fun T => fv_val T) s).
 
 (* ###################################################################### *)
 (** ** Operational Semantics *)
@@ -210,16 +194,16 @@ Definition fv_sto_vals(s: sto): vars := (fv_in_values (fun T => fv_val T) s).
 Inductive red : trm -> sto -> trm -> sto -> Prop :=
 | red_sel : forall x m s t T ds,
     binds x (val_new T ds) s ->
-    defs_has (open_defs (in_sto x) ds) (def_trm m t) ->
-    red (trm_sel (avar_s x) m) s t s
+    defs_has (open_defs x ds) (def_trm m t) ->
+    red (trm_sel (avar_f x) m) s t s
 | red_app : forall f a s T t,
     binds f (val_lambda T t) s ->
-    red (trm_app (avar_s f) (avar_s a)) s (open_trm (in_sto a) t) s
+    red (trm_app (avar_f f) (avar_f a)) s (open_trm a t) s
 | red_let : forall v t s x,
     x # s ->
-    red (trm_let (trm_val v) t) s (open_trm (in_sto x) t) (s & x ~ v)
+    red (trm_let (trm_val v) t) s (open_trm x t) (s & x ~ v)
 | red_let_var : forall t s x,
-    red (trm_let (trm_var (avar_s x)) t) s (open_trm (in_sto x) t) s
+    red (trm_let (trm_var (avar_f x)) t) s (open_trm x t) s
 | red_let_tgt : forall t0 t s t0' s',
     red t0 s t0' s' ->
     red (trm_let t0 t) s (trm_let t0' t) s'.
@@ -227,130 +211,107 @@ Inductive red : trm -> sto -> trm -> sto -> Prop :=
 (* ###################################################################### *)
 (** ** Typing *)
 
-Inductive tymode: Set := ty_precise | ty_general | ty_tight: nat -> tymode.
-(* ty_tight bounds the number of unpacking *)
+Inductive tymode: Set := ty_precise | ty_general.
+Inductive submode: Set := sub_tight | sub_general.
 
-Inductive restricted_by : var -> ctx -> ctx -> Prop :=
-| lim_ctx : forall x T G G1 G2,
-              G = G1 & (x ~ T) & G2 ->
-              restricted_by x G (G1 & (x ~ T)).
-
-Inductive ty_trm : tymode -> ctx -> ctx -> trm -> typ -> Prop :=
-| ty_var_s : forall m Gs G x T,
-    binds x T Gs ->
-    ty_trm m Gs G (trm_var (avar_s x)) T
-| ty_var_c : forall m Gs G x T,
+Inductive ty_trm : tymode -> submode -> ctx -> trm -> typ -> Prop :=
+| ty_var : forall m1 m2 G x T,
     binds x T G ->
-    ty_trm m Gs G (trm_var (avar_c x)) T
-| ty_all_intro : forall L m Gs G T t U,
+    ty_trm m1 m2 G (trm_var (avar_f x)) T
+| ty_all_intro : forall L m1 m2 G T t U,
     (forall x, x \notin L ->
-      ty_trm ty_general Gs (G & x ~ T) (open_trm (in_ctx x) t) (open_typ (in_ctx x) U)) ->
-    ty_trm m Gs G (trm_val (val_lambda T t)) (typ_all T U)
-| ty_all_elim : forall Gs G x z S T,
-    ty_trm ty_general Gs G (trm_var (avar_f x)) (typ_all S T) ->
-    ty_trm ty_general Gs G (trm_var (avar_f z)) S ->
-    ty_trm ty_general Gs G (trm_app (avar_f x) (avar_f z)) (open_typ z T)
-| ty_new_intro : forall L m Gs G T ds,
+      ty_trm ty_general sub_general (G & x ~ T) (open_trm x t) (open_typ x U)) ->
+    ty_trm m1 m2 G (trm_val (val_lambda T t)) (typ_all T U)
+| ty_all_elim : forall m2 G x z S T,
+    ty_trm ty_general m2 G (trm_var (avar_f x)) (typ_all S T) ->
+    ty_trm ty_general m2 G (trm_var (avar_f z)) S ->
+    ty_trm ty_general m2 G (trm_app (avar_f x) (avar_f z)) (open_typ z T)
+| ty_new_intro : forall L m1 m2 G T ds,
     (forall x, x \notin L ->
-      ty_defs Gs (G & (x ~ open_typ (in_ctx x) T)) (open_defs (in_ctx x) ds) (open_typ (in_ctx x) T)) ->
-    ty_trm m Gs G (trm_val (val_new T ds)) (typ_bnd T)
-| ty_new_elim : forall Gs G x a T,
-    ty_trm ty_general Gs G (trm_var (avar_f x)) (typ_rcd (dec_trm a T)) ->
-    ty_trm ty_general Gs G (trm_sel (avar_f x) a) T
-| ty_let : forall L Gs G t u T U,
-    ty_trm ty_general Gs G t T ->
+      ty_defs (G & (x ~ open_typ x T)) (open_defs x ds) (open_typ x T)) ->
+    ty_trm m1 m2 G (trm_val (val_new T ds)) (typ_bnd T)
+| ty_new_elim : forall m2 G x m T,
+    ty_trm ty_general m2 G (trm_var (avar_f x)) (typ_rcd (dec_trm m T)) ->
+    ty_trm ty_general m2 G (trm_sel (avar_f x) m) T
+| ty_let : forall L m2 G t u T U,
+    ty_trm ty_general m2 G t T ->
     (forall x, x \notin L ->
-      ty_trm ty_general Gs (G & x ~ T) (open_trm (in_ctx x) u) U) ->
-    ty_trm ty_general Gs G (trm_let t u) U
-| ty_rec_intro : forall Gs G x T,
-    ty_trm ty_general Gs G (trm_var (avar_f x)) (open_typ x T) ->
-    ty_trm ty_general Gs G (trm_var (avar_f x)) (typ_bnd T)
-| ty_rec_intro_tight : forall n Gs G x T,
-    ty_trm (ty_tight n) Gs G (trm_var (avar_f x)) (open_typ x T) ->
-    ty_trm (ty_tight (S n)) Gs G (trm_var (avar_f x)) (typ_bnd T)
-| ty_rec_elim : forall m Gs G x T,
-    ty_trm m Gs G (trm_var (avar_f x)) (typ_bnd T) ->
-    ty_trm m Gs G (trm_var (avar_f x)) (open_typ x T)
-| ty_and_intro : forall m Gs G x T U, m <> ty_precise ->
-    ty_trm m Gs G (trm_var (avar_f x)) T ->
-    ty_trm m Gs G (trm_var (avar_f x)) U ->
-    ty_trm m Gs G (trm_var (avar_f x)) (typ_and T U)
-| ty_sub : forall m Gs G t T U,
-    (m <> ty_general -> exists x, t = trm_var (avar_f x)) ->
-    ty_trm m Gs G t T ->
-    subtyp m Gs G T U ->
-    ty_trm m Gs G t U
-| ty_monotone_tight : forall n1 n2 Gs G t T,
-    ty_trm (ty_tight n1) Gs G t T -> n1 <= n2 ->
-    ty_trm (ty_tight n2) Gs G t T
-
-with ty_def : ctx -> ctx -> def -> dec -> Prop :=
-| ty_def_typ : forall Gs G A T,
-    ty_def Gs G (def_typ A T) (dec_typ A T T)
-| ty_def_trm : forall Gs G a t T,
-    ty_trm ty_general Gs G t T ->
-    ty_def Gs G (def_trm a t) (dec_trm a T)
-with ty_defs : ctx -> ctx -> defs -> typ -> Prop :=
-| ty_defs_one : forall Gs G d D,
-    ty_def Gs G d D ->
-    ty_defs Gs G (defs_cons defs_nil d) (typ_rcd D)
-| ty_defs_cons : forall Gs G ds d T D,
-    ty_defs Gs G ds T ->
-    ty_def Gs G d D ->
+      ty_trm ty_general sub_general (G & x ~ T) (open_trm x u) U) ->
+    ty_trm ty_general m2 G (trm_let t u) U
+| ty_rec_intro : forall m2 G x T,
+    ty_trm ty_general m2 G (trm_var (avar_f x)) (open_typ x T) ->
+    ty_trm ty_general m2 G (trm_var (avar_f x)) (typ_bnd T)
+| ty_rec_elim : forall m1 m2 G x T,
+    ty_trm m1 m2 G (trm_var (avar_f x)) (typ_bnd T) ->
+    ty_trm m1 m2 G (trm_var (avar_f x)) (open_typ x T)
+| ty_and_intro : forall m2 G x T U,
+    ty_trm ty_general m2 G (trm_var (avar_f x)) T ->
+    ty_trm ty_general m2 G (trm_var (avar_f x)) U ->
+    ty_trm ty_general m2 G (trm_var (avar_f x)) (typ_and T U)
+| ty_sub : forall m1 m2 G t T U,
+    (m1 = ty_precise -> exists x, t = trm_var (avar_f x)) ->
+    ty_trm m1 m2 G t T ->
+    subtyp m1 m2 G T U ->
+    ty_trm m1 m2 G t U
+with ty_def : ctx -> def -> dec -> Prop :=
+| ty_def_typ : forall G A T,
+    ty_def G (def_typ A T) (dec_typ A T T)
+| ty_def_trm : forall G a t T,
+    ty_trm ty_general sub_general G t T ->
+    ty_def G (def_trm a t) (dec_trm a T)
+with ty_defs : ctx -> defs -> typ -> Prop :=
+| ty_defs_one : forall G d D,
+    ty_def G d D ->
+    ty_defs G (defs_cons defs_nil d) (typ_rcd D)
+| ty_defs_cons : forall G ds d T D,
+    ty_defs G ds T ->
+    ty_def G d D ->
     defs_hasnt ds (label_of_def d) ->
-    ty_defs Gs G (defs_cons ds d) (typ_and T (typ_rcd D))
+    ty_defs G (defs_cons ds d) (typ_and T (typ_rcd D))
 
-with subtyp : tymode -> ctx -> ctx -> typ -> typ -> Prop :=
-| subtyp_top: forall m Gs G T, m <> ty_precise ->
-    subtyp m Gs G T typ_top
-| subtyp_bot: forall m Gs G T, m <> ty_precise ->
-    subtyp m Gs G typ_bot T
-| subtyp_refl: forall m Gs G T, m <> ty_precise ->
-    subtyp m Gs G T T
-| subtyp_trans: forall m Gs G S T U,
-    subtyp m Gs G S T ->
-    subtyp m Gs G T U ->
-    subtyp m Gs G S U
-| subtyp_and11: forall m Gs G T U,
-    subtyp m Gs G (typ_and T U) T
-| subtyp_and12: forall m Gs G T U,
-    subtyp m Gs G (typ_and T U) U
-| subtyp_and2: forall m Gs G S T U, m <> ty_precise ->
-    subtyp m Gs G S T ->
-    subtyp m Gs G S U ->
-    subtyp m Gs G S (typ_and T U)
-| subtyp_fld: forall m Gs G a T U, m <> ty_precise ->
-    subtyp m Gs G T U ->
-    subtyp m Gs G (typ_rcd (dec_trm a T)) (typ_rcd (dec_trm a U))
-| subtyp_typ: forall m Gs G A S1 T1 S2 T2, m <> ty_precise ->
-    subtyp m Gs G S2 S1 ->
-    subtyp m Gs G T1 T2 ->
-    subtyp m Gs G (typ_rcd (dec_typ A S1 T1)) (typ_rcd (dec_typ A S2 T2))
-| subtyp_sel2_c: forall m Gs G G' x A S T, m <> ty_precise ->
-    restricted_by x G G' ->
-    ty_trm m Gs G' (trm_var (avar_c x)) (typ_rcd (dec_typ A S T)) ->
-    subtyp m Gs G S (typ_sel (avar_c x) A)
-| subtyp_sel1_c: forall m Gs G G' x A S T, m <> ty_precise ->
-    restricted_by x G G' ->
-    ty_trm m Gs G' (trm_var (avar_c x)) (typ_rcd (dec_typ A S T)) ->
-    subtyp m Gs G (typ_sel (avar_c x) A) T
-| subtyp_sel2_s: forall m mt Gs G x A S T, m <> ty_precise ->
-    ((m = ty_general /\ mt = ty_general) \/ (m <> ty_general /\ mt = ty_precise)) ->
-    ty_trm mt Gs G (trm_var (avar_s x)) (typ_rcd (dec_typ A S T)) ->
-    subtyp m Gs G S (typ_sel (avar_s x) A)
-| subtyp_sel1_s: forall m mt Gs G x A S T, m <> ty_precise ->
-    ((m = ty_general /\ mt = ty_general) \/ (m <> ty_general /\ mt = ty_precise)) ->
-    ty_trm mt Gs G (trm_var (avar_s x)) (typ_rcd (dec_typ A S T)) ->
-    subtyp m Gs G (typ_sel (avar_s x) A) T
-| subtyp_all: forall L m Gs G S1 T1 S2 T2, m <> ty_precise ->
-    subtyp ty_general Gs G S2 S1 ->
+with subtyp : tymode -> submode -> ctx -> typ -> typ -> Prop :=
+| subtyp_top: forall m2 G T,
+    subtyp ty_general m2 G T typ_top
+| subtyp_bot: forall m2 G T,
+    subtyp ty_general m2 G typ_bot T
+| subtyp_refl: forall m2 G T,
+    subtyp ty_general m2 G T T
+| subtyp_trans: forall m1 m2 G S T U,
+    subtyp m1 m2 G S T ->
+    subtyp m1 m2 G T U ->
+    subtyp m1 m2 G S U
+| subtyp_and11: forall m1 m2 G T U,
+    subtyp m1 m2 G (typ_and T U) T
+| subtyp_and12: forall m1 m2 G T U,
+    subtyp m1 m2 G (typ_and T U) U
+| subtyp_and2: forall m2 G S T U,
+    subtyp ty_general m2 G S T ->
+    subtyp ty_general m2 G S U ->
+    subtyp ty_general m2 G S (typ_and T U)
+| subtyp_fld: forall m2 G a T U,
+    subtyp ty_general m2 G T U ->
+    subtyp ty_general m2 G (typ_rcd (dec_trm a T)) (typ_rcd (dec_trm a U))
+| subtyp_typ: forall m2 G A S1 T1 S2 T2,
+    subtyp ty_general m2 G S2 S1 ->
+    subtyp ty_general m2 G T1 T2 ->
+    subtyp ty_general m2 G (typ_rcd (dec_typ A S1 T1)) (typ_rcd (dec_typ A S2 T2))
+| subtyp_sel2: forall G x A S T,
+    ty_trm ty_general sub_general G (trm_var (avar_f x)) (typ_rcd (dec_typ A S T)) ->
+    subtyp ty_general sub_general G S (typ_sel (avar_f x) A)
+| subtyp_sel1: forall G x A S T,
+    ty_trm ty_general sub_general G (trm_var (avar_f x)) (typ_rcd (dec_typ A S T)) ->
+    subtyp ty_general sub_general G (typ_sel (avar_f x) A) T
+| subtyp_sel2_tight: forall G x A T,
+    ty_trm ty_precise sub_general G (trm_var (avar_f x)) (typ_rcd (dec_typ A T T)) ->
+    subtyp ty_general sub_tight G T (typ_sel (avar_f x) A)
+| subtyp_sel1_tight: forall G x A T,
+    ty_trm ty_precise sub_general G (trm_var (avar_f x)) (typ_rcd (dec_typ A T T)) ->
+    subtyp ty_general sub_tight G (typ_sel (avar_f x) A) T
+| subtyp_all: forall L m2 G S1 T1 S2 T2,
+    subtyp ty_general m2 G S2 S1 ->
     (forall x, x \notin L ->
-       subtyp ty_general Gs (G & x ~ S2) (open_typ (in_ctx x) T1) (open_typ (in_ctx x) T2)) ->
-    subtyp m Gs G (typ_all S1 T1) (typ_all S2 T2)
-| subtyp_bnd: forall L m Gs G T1 T2, m <> ty_precise ->
-    (forall x, x \notin L ->
-       subtyp m Gs (G & x ~ (typ_bnd T1)) (open_typ (in_ctx x) T1) (open_typ (in_ctx x) T2)) ->
-    subtyp m Gs G (typ_bnd T1) (typ_bnd T2).
+       subtyp ty_general sub_general (G & x ~ S2) (open_typ x T1) (open_typ x T2)) ->
+    subtyp ty_general m2 G (typ_all S1 T1) (typ_all S2 T2).
 
 Inductive wf_sto: ctx -> sto -> Prop :=
 | wf_sto_empty: wf_sto empty empty
@@ -358,7 +319,7 @@ Inductive wf_sto: ctx -> sto -> Prop :=
     wf_sto G s ->
     x # G ->
     x # s ->
-    ty_trm ty_precise G empty (trm_val v) T ->
+    ty_trm ty_precise sub_general G (trm_val v) T ->
     wf_sto (G & x ~ T) (s & x ~ v).
 
 (* ###################################################################### *)
@@ -400,7 +361,7 @@ Ltac gather_vars :=
   let A := gather_vars_with (fun x : vars      => x         ) in
   let B := gather_vars_with (fun x : var       => \{ x }    ) in
   let C := gather_vars_with (fun x : ctx       => (dom x) \u (fv_ctx_types x)) in
-  let D := gather_vars_with (fun x : sto       => dom x   \u (fv_sto_vals x)) in
+  let D := gather_vars_with (fun x : sto       => dom x     ) in
   let E := gather_vars_with (fun x : avar      => fv_avar  x) in
   let F := gather_vars_with (fun x : trm       => fv_trm   x) in
   let G := gather_vars_with (fun x : val       => fv_val   x) in
@@ -449,153 +410,29 @@ Qed.
 (** * Proofs *)
 
 (* ###################################################################### *)
-(** ** Well-formed store *)
-Lemma wf_sto_to_ok_s: forall s G,
-  wf_sto G s -> ok s.
-Proof. intros. induction H; jauto. Qed.
-
-Lemma wf_sto_to_ok_G: forall s G,
-  wf_sto G s -> ok G.
-Proof. intros. induction H; jauto. Qed.
-
-Hint Resolve wf_sto_to_ok_s wf_sto_to_ok_G.
-
-(* ###################################################################### *)
 (** ** Weakening *)
 
-Lemma ok_restricted_by: forall x G G',
-  ok G ->
-  restricted_by x G G' ->
-  ok G'.
-Proof.
-  introv Hok r. destruct r. subst.
-  eauto.
-Qed.
-
-Lemma binds_exists: forall {V} x (T:V) G,
-  binds x T G ->
-  ok G ->
-  exists G1 G2, G = G1 & (x ~ T) & G2.
-Proof.
-  introv Bi Hok. induction Hok.
-  - false. eapply binds_empty_inv. eassumption.
-  - apply binds_push_inv in Bi.
-    destruct Bi as [[Heqx Heqv] | [Neqx Bi]].
-    + subst. exists E. exists (@empty V). rewrite concat_empty_r. reflexivity.
-    + specialize (IHHok Bi). destruct IHHok as [G1 [G2 EqE]].
-      subst. exists G1. exists (G2 & x0 ~ v).
-      rewrite concat_assoc. reflexivity.
-Qed.
-
-Lemma concat_ok_eq: forall {V} G1 G2 G1' G2' x (T:V) (T':V),
-  G1 & x ~ T & G2 = G1' & x ~ T' & G2' ->
-  ok (G1 & x ~ T & G2) ->
-  G1 = G1' /\ G2 = G2' /\ T = T'.
-Proof.
-  introv Eq Hok.
-  assert (ok G1) as Hok1. {
-    apply ok_remove in Hok. eauto.
-  }
-  assert (ok G1') as Hok1'. {
-    rewrite Eq in Hok. apply ok_remove in Hok. eauto.
-  }
-  assert (ok G2) as Hok2. {
-    apply ok_remove in Hok. eauto.
-  }
-  assert (ok G2') as Hok2'. {
-    rewrite Eq in Hok. apply ok_remove in Hok. eauto.
-  }
-  assert (ok (G1' & x ~ T' & G2')) as Hok'. {
-    rewrite Eq in Hok. eauto.
-  }
-  generalize dependent G2'.
-  generalize dependent G1'.
-  induction Hok2; intros; inversion Hok2'; subst.
-  - rewrite concat_empty_r in Eq. rewrite concat_empty_r in Eq.
-    eapply eq_push_inv  in Eq. destruct Eq as [? [? Eq]]. eauto.
-  - rewrite concat_empty_r in Eq. rewrite concat_assoc in Eq.
-    eapply eq_push_inv in Eq. destruct Eq as [? [? Eq]]. subst.
-    eapply ok_middle_inv in Hok'. destruct Hok' as [? Contra].
-    eapply fresh_push_eq_inv in Contra. inversion Contra.
-  - rewrite concat_empty_r in Eq. rewrite concat_assoc in Eq.
-    eapply eq_push_inv in Eq. destruct Eq as [? [? Eq]]. subst.
-    rewrite concat_empty_r in Hok'. eapply ok_remove in Hok'.
-    assert (G1 & x ~ T & x ~ T' = G1 & x ~ T & (empty & x ~ T')) as A. {
-      rewrite concat_empty_l. reflexivity.
-    }
-    rewrite A in Hok'. eapply ok_middle_inv in Hok'. destruct Hok' as [_ Contra].
-    eapply fresh_push_eq_inv in Contra. inversion Contra.
-  - rewrite concat_assoc in Eq. rewrite concat_assoc in Eq.
-    eapply eq_push_inv in Eq. destruct Eq as [? [? Eq]]. subst.
-    assert (G1 = G1' /\ E = E0 /\ T = T') as A. {
-      eapply IHHok2; eauto.
-      rewrite concat_assoc in Hok. eauto.
-      rewrite concat_assoc in Hok'. eauto.
-    }
-    destruct A as [? [? ?]]. subst. split; eauto.
-Qed.
-
-Lemma weaken_restricted_by: forall x G' G1 G2 G3,
-  restricted_by x (G1 & G3) G' ->
-  ok (G1 & G2 & G3) ->                                 
-  restricted_by x (G1 & G2 & G3) G' \/
-  exists G3', G' = G1 & G3' /\ restricted_by x (G1 & G2 & G3) (G1 & G2 & G3').
-Proof.
-  introv r Hok. inversion r; subst.
-  assert (ok (G1 & G3)) as Hok13 by eauto.
-  destruct binds_concat_inv with (E1:=G1) (E2:=G3) (x:=x) (v:=T); eauto.
-  rewrite H. apply binds_middle_eq.
-  rewrite H in Hok13.
-  apply ok_middle_inv in Hok13. destruct Hok13. assumption.
-  right.
-  assert (exists G3a G3b, G3 = G3a & (x ~ T) & G3b) as E3. {
-    apply binds_exists; eauto.
-  }
-  destruct E3 as [G3a [G3b Eq3]]. subst.
-  assert (G1 & G3a = G0 /\ G3b = G4 /\ T = T) as A. {
-    eapply concat_ok_eq.
-    repeat rewrite concat_assoc in H. eapply H.
-    repeat rewrite concat_assoc in Hok13. eapply Hok13.
-  }
-  destruct A as [A1 [A2 ?]]. subst.
-  exists (G3a & x ~ T). split. rewrite concat_assoc. reflexivity.
-  repeat rewrite concat_assoc. apply lim_ctx with (G2:=G4). reflexivity.
-  left. destruct H0 as [NoBi3 Bi1].
-  assert (exists G1a G1b, G1 = G1a & (x ~ T) & G1b) as E1. {
-    apply binds_exists; eauto.
-  }
-  destruct E1 as [G1a [G1b Eq1]]. subst.
-  assert (G1a = G0 /\ G1b & G3 = G4 /\ T = T) as A. {
-    eapply concat_ok_eq.
-    repeat rewrite concat_assoc. eapply H.
-    repeat rewrite concat_assoc. eapply Hok13.
-  }
-  destruct A as [A1 [A2 ?]]. subst.
-  apply lim_ctx with (G2:=G1b & G2 & G3).
-  repeat rewrite concat_assoc. reflexivity.
-Qed.
-
 Lemma weaken_rules:
-  (forall m Gs G t T, ty_trm m Gs G t T -> forall G1 G2 G3,
+  (forall m1 m2 G t T, ty_trm m1 m2 G t T -> forall G1 G2 G3,
     G = G1 & G3 ->
     ok (G1 & G2 & G3) ->
-    ty_trm m Gs (G1 & G2 & G3) t T) /\
-  (forall Gs G d D, ty_def Gs G d D -> forall G1 G2 G3,
+    ty_trm m1 m2 (G1 & G2 & G3) t T) /\
+  (forall G d D, ty_def G d D -> forall G1 G2 G3,
     G = G1 & G3 ->
     ok (G1 & G2 & G3) ->
-    ty_def Gs (G1 & G2 & G3) d D) /\
-  (forall Gs G ds T, ty_defs Gs G ds T -> forall G1 G2 G3,
+    ty_def (G1 & G2 & G3) d D) /\
+  (forall G ds T, ty_defs G ds T -> forall G1 G2 G3,
     G = G1 & G3 ->
     ok (G1 & G2 & G3) ->
-    ty_defs Gs (G1 & G2 & G3) ds T) /\
-  (forall m Gs G T U, subtyp m Gs G T U -> forall G1 G2 G3,
+    ty_defs (G1 & G2 & G3) ds T) /\
+  (forall m1 m2 G T U, subtyp m1 m2 G T U -> forall G1 G2 G3,
     G = G1 & G3 ->
     ok (G1 & G2 & G3) ->
-    subtyp m Gs (G1 & G2 & G3) T U).
+    subtyp m1 m2 (G1 & G2 & G3) T U).
 Proof.
-  apply rules_mutind; try solve [eauto 4].
+  apply rules_mutind; try solve [eauto].
   + intros. subst.
-    eapply ty_var_c. eapply binds_weaken; eauto.
+    eapply ty_var. eapply binds_weaken; eauto.
   + intros. subst.
     apply_fresh ty_all_intro as z. eauto.
     assert (zL: z \notin L) by auto.
@@ -604,7 +441,7 @@ Proof.
     apply* H.
   + intros. subst.
     apply_fresh ty_new_intro as z; assert (zL: z \notin L) by auto.
-    - specialize (H z zL G1 G2 (G3 & z ~ open_typ (in_ctx z) T)).
+    - specialize (H z zL G1 G2 (G3 & z ~ open_typ z T)).
       repeat rewrite concat_assoc in H.
       apply* H.
   + intros. subst.
@@ -614,24 +451,6 @@ Proof.
     repeat rewrite concat_assoc in H0.
     apply* H0.
   + intros. subst.
-    inversion r; subst.
-    apply weaken_restricted_by with (G2:=G2) in r.
-    destruct r.
-    eapply subtyp_sel2_c. assumption. eassumption. eassumption.
-    destruct H2 as [G3' [Heq r]].
-    eapply subtyp_sel2_c. assumption. eapply r. eapply H. eapply Heq.
-    rewrite Heq in H0. eapply ok_restricted_by; eauto.
-    eauto.
-  + intros. subst.
-    inversion r; subst.
-    apply weaken_restricted_by with (G2:=G2) in r.
-    destruct r.
-    eapply subtyp_sel1_c. assumption. eassumption. eassumption.
-    destruct H2 as [G3' [Heq r]].
-    eapply subtyp_sel1_c. assumption. eapply r. eapply H. eapply Heq.
-    rewrite Heq in H0. eapply ok_restricted_by; eauto.
-    eauto.
-  + intros. subst.
     apply_fresh subtyp_all as z.
     eauto.
     eauto.
@@ -639,34 +458,12 @@ Proof.
     specialize (H0 z zL G1 G2 (G3 & z ~ S2)).
     repeat rewrite concat_assoc in H0.
     apply* H0.
-  + intros. subst.
-    apply_fresh subtyp_bnd as z.
-    assumption.
-    assert (zL: z \notin L) by auto.
-    specialize (H z zL G1 G2 (G3 & z ~ typ_bnd T1)).
-    repeat rewrite concat_assoc in H.
-    apply* H.
 Qed.
 
-Lemma weaken_ty_trm:  forall m Gs G1 G2 t T,
-    ty_trm m Gs G1 t T ->
+Lemma weaken_ty_trm:  forall m1 m2 G1 G2 t T,
+    ty_trm m1 m2 G1 t T ->
     ok (G1 & G2) ->
-    ty_trm m Gs (G1 & G2) t T.
-Proof.
-  intros.
-  assert (G1 & G2 = G1 & G2 & empty) as EqG. {
-    rewrite concat_empty_r.
-    reflexivity.
-  }
-  rewrite EqG. apply* weaken_rules.
-  rewrite concat_empty_r. reflexivity.
-  rewrite <- EqG. assumption.
-Qed.
-
-Lemma weaken_subtyp: forall m1 Gs G1 G2 S U,
-  subtyp m1 Gs G1 S U ->
-  ok (G1 & G2) ->
-  subtyp m1 Gs (G1 & G2) S U.
+    ty_trm m1 m2 (G1 & G2) t T.
 Proof.
   intros.
     assert (G1 & G2 = G1 & G2 & empty) as EqG. {
@@ -677,47 +474,37 @@ Proof.
   rewrite <- EqG. assumption.
 Qed.
 
-Lemma weaken_sto_rules:
-  (forall m Gs G t T, ty_trm m Gs G t T -> forall Gs',
-    ok (Gs & Gs') ->
-    ty_trm m (Gs & Gs') G t T) /\
-  (forall Gs G d D, ty_def Gs G d D -> forall Gs',
-    ok (Gs & Gs') ->
-    ty_def (Gs & Gs') G d D) /\
-  (forall Gs G ds T, ty_defs Gs G ds T -> forall Gs',
-    ok (Gs & Gs') ->
-    ty_defs (Gs & Gs') G ds T) /\
-  (forall m Gs G T U, subtyp m Gs G T U -> forall Gs',
-    ok (Gs & Gs') ->
-    subtyp m (Gs & Gs') G T U).
-Proof.
-  apply rules_mutind; eauto 4 using binds_concat_left_ok.
-Qed.
-
-Lemma weaken_sto_ty_trm:  forall m Gs Gs' G t T,
-    ty_trm m Gs G t T ->
-    ok (Gs & Gs') ->
-    ty_trm m (Gs & Gs') G t T.
+Lemma weaken_subtyp: forall m1 m2 G1 G2 S U,
+  subtyp m1 m2 G1 S U ->
+  ok (G1 & G2) ->
+  subtyp m1 m2 (G1 & G2) S U.
 Proof.
   intros.
-  apply* weaken_sto_rules.
-Qed.
-
-Lemma weaken_sto_subtyp:  forall m Gs Gs' G S U,
-    subtyp m Gs G S U ->
-    ok (Gs & Gs') ->
-    subtyp m (Gs & Gs') G S U.
-Proof.
-  intros.
-  apply* weaken_sto_rules.
+    assert (G1 & G2 = G1 & G2 & empty) as EqG. {
+    rewrite concat_empty_r. reflexivity.
+  }
+  rewrite EqG. apply* weaken_rules.
+  rewrite concat_empty_r. reflexivity.
+  rewrite <- EqG. assumption.
 Qed.
 
 (* ###################################################################### *)
+(** ** Well-formed store *)
+
+Lemma wf_sto_to_ok_s: forall s G,
+  wf_sto G s -> ok s.
+Proof. intros. induction H; jauto. Qed.
+
+Lemma wf_sto_to_ok_G: forall s G,
+  wf_sto G s -> ok G.
+Proof. intros. induction H; jauto. Qed.
+
+Hint Resolve wf_sto_to_ok_s wf_sto_to_ok_G.
 
 Lemma ctx_binds_to_sto_binds_raw: forall s G x T,
   wf_sto G s ->
   binds x T G ->
-  exists G1 G2 v, G = G1 & (x ~ T) & G2 /\ binds x v s /\ ty_trm ty_precise G1 empty (trm_val v) T.
+  exists G1 G2 v, G = G1 & (x ~ T) & G2 /\ binds x v s /\ ty_trm ty_precise sub_general G1 (trm_val v) T.
 Proof.
   introv Wf Bi. gen x T Bi. induction Wf; intros.
   + false* binds_empty_inv.
@@ -731,7 +518,7 @@ Qed.
 Lemma sto_binds_to_ctx_binds_raw: forall s G x v,
   wf_sto G s ->
   binds x v s ->
-  exists G1 G2 T, G = G1 & (x ~ T) & G2 /\ ty_trm ty_precise G1 empty (trm_val v) T.
+  exists G1 G2 T, G = G1 & (x ~ T) & G2 /\ ty_trm ty_precise sub_general G1 (trm_val v) T.
 Proof.
   introv Wf Bi. gen x v Bi. induction Wf; intros.
   + false* binds_empty_inv.
@@ -784,12 +571,11 @@ Proof.
     - auto.
 Qed.
 
-
-Lemma typing_implies_ctx_bound: forall m Gs G x T,
-  ty_trm m Gs G (trm_var (avar_c x)) T ->
+Lemma typing_implies_bound: forall m1 m2 G x T,
+  ty_trm m1 m2 G (trm_var (avar_f x)) T ->
   exists S, binds x S G.
 Proof.
-  intros. remember (trm_var (avar_c x)) as t.
+  intros. remember (trm_var (avar_f x)) as t.
   induction H;
     try solve [inversion Heqt];
     try solve [inversion Heqt; eapply IHty_trm; eauto];
@@ -797,42 +583,90 @@ Proof.
   - inversion Heqt. subst. exists T. assumption.
 Qed.
 
-Lemma typing_implies_sto_bound: forall m Gs G x T,
-  ty_trm m Gs G (trm_var (avar_s x)) T ->
-  exists T, binds x T Gs.
-Proof.
-  intros. remember (trm_var (avar_s x)) as t.
-  induction H;
-    try solve [inversion Heqt];
-    try solve [inversion Heqt; eapply IHty_trm; eauto];
-    try solve [inversion Heqt; eapply IHty_trm1; eauto].
-  - inversion Heqt. subst. exists T. assumption.
-Qed.
-
-Lemma typing_bvar_implies_false: forall m1 Gs G a T,
-  ty_trm m1 Gs G (trm_var (avar_b a)) T ->
+Lemma typing_bvar_implies_false: forall m1 m2 G a T,
+  ty_trm m1 m2 G (trm_var (avar_b a)) T ->
   False.
 Proof.
-  intros. remember (trm_var (avar_b a)) as t. induction H; try solve [inversion Heqt];
-  eapply IHty_trm; auto.
+  intros. remember (trm_var (avar_b a)) as t. induction H; try solve [inversion Heqt].
+  eapply IHty_trm. auto.
+Qed.
+
+(* ###################################################################### *)
+(** ** Extra Rec *)
+
+Lemma extra_bnd_rules:
+  (forall m1 m2 G t T, ty_trm m1 m2 G t T -> forall G1 G2 x S G',
+    G = G1 & (x ~ open_typ x S) & G2 ->
+    G' = G1 & (x ~ typ_bnd S) & G2 ->
+    ty_trm m1 m2 G' t T)
+/\ (forall G d D, ty_def G d D -> forall G1 G2 x S G',
+    G = G1 & (x ~ open_typ x S) & G2 ->
+    G' = G1 & (x ~ typ_bnd S) & G2 ->
+    ty_def G' d D)
+/\ (forall G ds T, ty_defs G ds T -> forall G1 G2 x S G',
+    G = G1 & (x ~ open_typ x S) & G2 ->
+    G' = G1 & (x ~ typ_bnd S) & G2 ->
+    ty_defs G' ds T)
+/\ (forall m1 m2 G T U, subtyp m1 m2 G T U -> forall G1 G2 x S G',
+    G = G1 & (x ~ open_typ x S) & G2 ->
+    G' = G1 & (x ~ typ_bnd S) & G2 ->
+    subtyp m1 m2 G' T U).
+Proof.
+  apply rules_mutind; intros; eauto.
+  - (* ty_var *)
+    subst. apply binds_middle_inv in b. destruct b as [Bi | [Bi | Bi]].
+    + apply ty_var. eauto.
+    + destruct Bi as [Bin [Eqx EqT ]]. subst.
+      apply ty_rec_elim. apply ty_var. eauto.
+    + destruct Bi as [Bin [Neqx Bi]]. apply ty_var. eauto.
+  - (* ty_all_intro *)
+    subst.
+    apply_fresh ty_all_intro as y; eauto.
+    assert (y \notin L) as FrL by eauto.
+    specialize (H y FrL).
+    specialize (H G1 (G2 & y ~ T) x S).
+    eapply H; eauto.
+    rewrite concat_assoc. reflexivity.
+    rewrite concat_assoc. reflexivity.
+  - (* ty_new_intro *)
+    subst.
+    apply_fresh ty_new_intro as y; eauto;
+    assert (y \notin L) as FrL by eauto.
+    specialize (H y FrL).
+    specialize (H G1 (G2 & y ~ open_typ y T) x S).
+    eapply H; eauto.
+    rewrite concat_assoc. reflexivity.
+    rewrite concat_assoc. reflexivity.
+  - (* ty_let *)
+    subst.
+    apply_fresh ty_let as y; eauto.
+    assert (y \notin L) as FrL by eauto.
+    specialize (H0 y FrL).
+    specialize (H0 G1 (G2 & y ~ T) x S).
+    eapply H0; eauto.
+    rewrite concat_assoc. reflexivity.
+    rewrite concat_assoc. reflexivity.
+  - (* subtyp_all *)
+    subst.
+    apply_fresh subtyp_all as y; eauto.
+    assert (y \notin L) as FrL by eauto.
+    specialize (H0 y FrL).
+    specialize (H0 G1 (G2 & y ~ S2) x S).
+    eapply H0; eauto.
+    rewrite concat_assoc. reflexivity.
+    rewrite concat_assoc. reflexivity.
 Qed.
 
 (* ###################################################################### *)
 (** ** Substitution *)
 
-Definition subst_fvar (z: var) (u: fvar) (v: fvar) : fvar :=
-  match v with
-  | in_sto x => in_sto x
-  | in_ctx x => (If x = z then u else in_ctx x)
-  end.
-
-Definition subst_avar (z: var) (u: fvar) (a: avar) : avar :=
+Definition subst_avar (z: var) (u: var) (a: avar) : avar :=
   match a with
   | avar_b i => avar_b i
-  | avar_f v => avar_f (subst_fvar z u v)
+  | avar_f x => (avar_f (If x = z then u else x))
   end.
 
-Fixpoint subst_typ (z: var) (u: fvar) (T: typ) { struct T } : typ :=
+Fixpoint subst_typ (z: var) (u: var) (T: typ) { struct T } : typ :=
   match T with
   | typ_top        => typ_top
   | typ_bot        => typ_bot
@@ -842,13 +676,13 @@ Fixpoint subst_typ (z: var) (u: fvar) (T: typ) { struct T } : typ :=
   | typ_bnd T      => typ_bnd (subst_typ z u T)
   | typ_all T U    => typ_all (subst_typ z u T) (subst_typ z u U)
   end
-with subst_dec (z: var) (u: fvar) (D: dec) { struct D } : dec :=
+with subst_dec (z: var) (u: var) (D: dec) { struct D } : dec :=
   match D with
   | dec_typ L T U => dec_typ L (subst_typ z u T) (subst_typ z u U)
   | dec_trm L U => dec_trm L (subst_typ z u U)
   end.
 
-Fixpoint subst_trm (z: var) (u: fvar) (t: trm) : trm :=
+Fixpoint subst_trm (z: var) (u: var) (t: trm) : trm :=
   match t with
   | trm_var x        => trm_var (subst_avar z u x)
   | trm_val v        => trm_val (subst_val z u v)
@@ -856,38 +690,31 @@ Fixpoint subst_trm (z: var) (u: fvar) (t: trm) : trm :=
   | trm_app x1 x2    => trm_app (subst_avar z u x1) (subst_avar z u x2)
   | trm_let t1 t2    => trm_let (subst_trm z u t1) (subst_trm z u t2)
   end
-with subst_val (z: var) (u: fvar) (v: val) : val :=
+with subst_val (z: var) (u: var) (v: val) : val :=
   match v with
   | val_new T ds     => val_new (subst_typ z u T) (subst_defs z u ds)
   | val_lambda T t   => val_lambda (subst_typ z u T) (subst_trm z u t)
   end
-with subst_def (z: var) (u: fvar) (d: def) : def :=
+with subst_def (z: var) (u: var) (d: def) : def :=
   match d with
   | def_typ L T => def_typ L (subst_typ z u T)
   | def_trm L t => def_trm L (subst_trm z u t)
   end
-with subst_defs (z: var) (u: fvar) (ds: defs) : defs :=
+with subst_defs (z: var) (u: var) (ds: defs) : defs :=
   match ds with
   | defs_nil => defs_nil
   | defs_cons rest d => defs_cons (subst_defs z u rest) (subst_def z u d)
   end.
 
-Definition subst_ctx (z: var) (u: fvar) (G: ctx) : ctx := map (subst_typ z u) G.
-Definition subst_sto (z: var) (u: fvar) (s: sto) : sto := map (subst_val z u) s.
+Definition subst_ctx (z: var) (u: var) (G: ctx) : ctx := map (subst_typ z u) G.
 
 (* ###################################################################### *)
 (** ** Lemmas for var-by-var substitution *)
 
-Lemma subst_fresh_fvar: forall x y,
-  (forall v: fvar, x \notin fv_fvar v -> subst_fvar x y v = v).
-Proof.
-  intros. unfold fv_fvar in *. destruct* v. simpl. case_var*. simpls. notin_false.
-Qed.
-
 Lemma subst_fresh_avar: forall x y,
   (forall a: avar, x \notin fv_avar a -> subst_avar x y a = a).
 Proof.
-  intros. destruct* a. simpl. f_equal. apply* subst_fresh_fvar.
+  intros. destruct* a. simpl. case_var*. simpls. notin_false.
 Qed.
 
 Lemma subst_fresh_typ_dec: forall x y,
@@ -897,8 +724,8 @@ Proof.
   intros x y. apply typ_mutind; intros; simpls; f_equal*. apply* subst_fresh_avar.
 Qed.
 
-Definition subst_fresh_typ x y := proj1 (subst_fresh_typ_dec x y).
-Definition subst_fresh_dec x y := proj2 (subst_fresh_typ_dec x y).
+Definition subst_fresh_typ(x y: var) := proj1 (subst_fresh_typ_dec x y).
+Definition subst_fresh_dec(x y: var) := proj2 (subst_fresh_typ_dec x y).
 
 Lemma subst_fresh_trm_val_def_defs: forall x y,
   (forall t : trm , x \notin fv_trm  t  -> subst_trm  x y t  = t ) /\
@@ -910,10 +737,10 @@ Proof.
     (apply* subst_fresh_avar || apply* subst_fresh_typ_dec).
 Qed.
 
-Definition subst_fresh_trm  x y := proj41 (subst_fresh_trm_val_def_defs x y).
-Definition subst_fresh_val  x y := proj42 (subst_fresh_trm_val_def_defs x y).
-Definition subst_fresh_def  x y := proj43 (subst_fresh_trm_val_def_defs x y).
-Definition subst_fresh_defs x y := proj44 (subst_fresh_trm_val_def_defs x y).
+Definition subst_fresh_trm (x y: var) := proj41 (subst_fresh_trm_val_def_defs x y).
+Definition subst_fresh_val (x y: var) := proj42 (subst_fresh_trm_val_def_defs x y).
+Definition subst_fresh_def (x y: var) := proj43 (subst_fresh_trm_val_def_defs x y).
+Definition subst_fresh_defs(x y: var) := proj44 (subst_fresh_trm_val_def_defs x y).
 
 Lemma invert_fv_ctx_types_push: forall x z T G,
   x \notin fv_ctx_types (G & z ~ T) -> x \notin fv_typ T /\ x \notin (fv_ctx_types G).
@@ -927,21 +754,6 @@ Proof.
   do 2 rewrite LibList.fold_right_cons in *.
   simpl in *.
   apply notin_union in N. exact N.
-Qed.
-
-Lemma fv_ctx_types_push: forall x z T G,
-  x \notin fv_typ T -> x \notin (fv_ctx_types G) ->
-  x \notin fv_ctx_types (G & z ~ T).
-Proof.
-  introv A B.
-  unfold fv_ctx_types in *.
-  unfold fv_in_values in *.
-  rewrite <- cons_to_push in *.
-  rewrite values_def in *.
-  unfold LibList.map in *.
-  do 2 rewrite LibList.fold_right_cons in *.
-  simpl in *.
-  apply notin_union. split; assumption.
 Qed.
 
 Lemma subst_fresh_ctx: forall x y G,
@@ -958,61 +770,16 @@ Proof.
     reflexivity.
 Qed.
 
-Lemma fv_ctx_types_binds: forall x z T G,
-  x \notin fv_ctx_types G -> binds z T G ->
-  x \notin fv_typ T.
-Proof.
-  intros.
-  unfold fv_ctx_types in *.
-  eapply fv_in_values_binds; eassumption.
-Qed.
-
-Lemma invert_fv_sto_vals_push: forall x z v s,
-  x \notin fv_sto_vals (s & z ~ v) -> x \notin fv_val v /\ x \notin (fv_sto_vals s).
-Proof.
-  introv N.
-  unfold fv_sto_vals in *.
-  unfold fv_in_values in *.
-  rewrite <- cons_to_push in *.
-  rewrite values_def in *.
-  unfold LibList.map in *.
-  do 2 rewrite LibList.fold_right_cons in *.
-  simpl in *.
-  apply notin_union in N. exact N.
-Qed.
-
-Lemma subst_fresh_sto: forall x y s,
-  x \notin fv_sto_vals s -> subst_sto x y s = s.
-Proof.
-  intros x y.
-  apply (env_ind (fun s => x \notin fv_sto_vals s -> subst_sto x y s = s)).
-  + intro N. unfold subst_sto. apply map_empty.
-  + intros G z T IH N.
-    apply invert_fv_sto_vals_push in N. destruct N as [N1 N2].
-    unfold subst_sto in *. rewrite map_push.
-    rewrite (IH N2).
-    rewrite subst_fresh_val.
-    reflexivity.
-    apply N1.
-Qed.
-
-Lemma fv_sto_vals_binds: forall x z v s,
-  x \notin fv_sto_vals s -> binds z v s ->
-  x \notin fv_val v.
-Proof.
-  intros.
-  unfold fv_sto_vals in *.
-  eapply fv_in_values_binds; eassumption.
-Qed.
+Definition subst_fvar(x y z: var): var := If z = x then y else z.
 
 Lemma subst_open_commute_avar: forall x y u,
   (forall a: avar, forall n: Datatypes.nat,
     subst_avar x y (open_rec_avar n u a)
-    = open_rec_avar n (subst_fvar x y u) (subst_avar x y a)).
+    = open_rec_avar n (subst_fvar x y u) (subst_avar  x y a)).
 Proof.
   intros. unfold subst_fvar, subst_avar, open_avar, open_rec_avar. destruct a.
   + repeat case_if; auto.
-  + reflexivity.
+  + case_var*.
 Qed.
 
 (* "open and then substitute" = "substitute and then open" *)
@@ -1079,7 +846,7 @@ Qed.
 (* "Introduce a substitution after open": Opening a term t with a var u is the
    same as opening t with x and then replacing x by u. *)
 Lemma subst_intro_trm: forall x u t, x \notin (fv_trm t) ->
-  open_trm u t = subst_trm x u (open_trm (in_ctx x) t).
+  open_trm u t = subst_trm x u (open_trm x t).
 Proof.
   introv Fr. unfold open_trm. rewrite* subst_open_commute_trm.
   destruct (@subst_fresh_trm_val_def_defs x u) as [Q _]. rewrite* (Q t).
@@ -1087,7 +854,7 @@ Proof.
 Qed.
 
 Lemma subst_intro_val: forall x u v, x \notin (fv_val v) ->
-  open_val u v = subst_val x u (open_val (in_ctx x) v).
+  open_val u v = subst_val x u (open_val x v).
 Proof.
   introv Fr. unfold open_trm. rewrite* subst_open_commute_val.
   destruct (@subst_fresh_trm_val_def_defs x u) as [_ [Q _]]. rewrite* (Q v).
@@ -1095,7 +862,7 @@ Proof.
 Qed.
 
 Lemma subst_intro_defs: forall x u ds, x \notin (fv_defs ds) ->
-  open_defs u ds = subst_defs x u (open_defs (in_ctx x) ds).
+  open_defs u ds = subst_defs x u (open_defs x ds).
 Proof.
   introv Fr. unfold open_trm. rewrite* subst_open_commute_defs.
   destruct (@subst_fresh_trm_val_def_defs x u) as [_ [_ [_ Q]]]. rewrite* (Q ds).
@@ -1103,7 +870,7 @@ Proof.
 Qed.
 
 Lemma subst_intro_typ: forall x u T, x \notin (fv_typ T) ->
-  open_typ u T = subst_typ x u (open_typ (in_ctx x) T).
+  open_typ u T = subst_typ x u (open_typ x T).
 Proof.
   introv Fr. unfold open_typ. rewrite* subst_open_commute_typ.
   destruct (@subst_fresh_typ_dec x u) as [Q _]. rewrite* (Q T).
@@ -1111,32 +878,24 @@ Proof.
 Qed.
 
 Lemma subst_intro_dec: forall x u D, x \notin (fv_dec D) ->
-  open_dec u D = subst_dec x u (open_dec (in_ctx x) D).
+  open_dec u D = subst_dec x u (open_dec x D).
 Proof.
   introv Fr. unfold open_trm. rewrite* subst_open_commute_dec.
   destruct (@subst_fresh_typ_dec x u) as [_ Q]. rewrite* (Q D).
   unfold subst_fvar. case_var*.
 Qed.
 
-Lemma subst_undo_fvar: forall x y,
-  (forall v, y \notin fv_fvar v -> (subst_fvar y (in_ctx x) (subst_fvar x (in_ctx y) v)) = v).
-Proof.
-  intros. unfold subst_fvar, subst_fvar; destruct v.
-  + reflexivity.
-  + unfold fv_fvar in H. assert (y <> v) by auto. repeat case_if; reflexivity.
-Qed.
-
 Lemma subst_undo_avar: forall x y,
-  (forall a, y \notin fv_avar a -> (subst_avar y (in_ctx x) (subst_avar x (in_ctx y) a)) = a).
+  (forall a, y \notin fv_avar a -> (subst_avar y x (subst_avar x y a)) = a).
 Proof.
-  intros. unfold subst_avar; destruct a.
+  intros. unfold subst_avar, subst_fvar, open_avar, open_rec_avar; destruct a.
   + reflexivity.
-  + f_equal. apply* subst_undo_fvar.
+  + unfold fv_avar in H. assert (y <> v) by auto. repeat case_if; reflexivity.
 Qed.
 
 Lemma subst_undo_typ_dec: forall x y,
-   (forall T , y \notin fv_typ  T  -> (subst_typ y (in_ctx x) (subst_typ  x (in_ctx y) T )) = T )
-/\ (forall D , y \notin fv_dec  D  -> (subst_dec y (in_ctx x) (subst_dec  x (in_ctx y) D )) = D ).
+   (forall T , y \notin fv_typ  T  -> (subst_typ  y x (subst_typ  x y T )) = T )
+/\ (forall D , y \notin fv_dec  D  -> (subst_dec  y x (subst_dec  x y D )) = D ).
 Proof.
   intros.
   apply typ_mutind; intros; simpl; unfold fv_typ, fv_dec in *; f_equal*.
@@ -1144,10 +903,10 @@ Proof.
 Qed.
 
 Lemma subst_undo_trm_val_def_defs: forall x y,
-   (forall t , y \notin fv_trm  t  -> (subst_trm  y (in_ctx x) (subst_trm  x (in_ctx y) t )) = t )
-/\ (forall v , y \notin fv_val  v  -> (subst_val  y (in_ctx x) (subst_val  x (in_ctx y) v )) = v )
-/\ (forall d , y \notin fv_def  d  -> (subst_def  y (in_ctx x) (subst_def  x (in_ctx y) d )) = d )
-/\ (forall ds, y \notin fv_defs ds -> (subst_defs y (in_ctx x) (subst_defs x (in_ctx y) ds)) = ds).
+   (forall t , y \notin fv_trm  t  -> (subst_trm  y x (subst_trm  x y t )) = t )
+/\ (forall v , y \notin fv_val  v  -> (subst_val  y x (subst_val  x y v )) = v )
+/\ (forall d , y \notin fv_def  d  -> (subst_def  y x (subst_def  x y d )) = d )
+/\ (forall ds, y \notin fv_defs ds -> (subst_defs y x (subst_defs x y ds)) = ds).
 Proof.
   intros.
   apply trm_mutind; intros; simpl; unfold fv_trm, fv_val, fv_def, fv_defs in *; f_equal*;
@@ -1155,31 +914,23 @@ Proof.
 Qed.
 
 Lemma subst_typ_undo: forall x y T,
-  y \notin fv_typ T -> (subst_typ y (in_ctx x) (subst_typ x (in_ctx y) T)) = T.
+  y \notin fv_typ T -> (subst_typ y x (subst_typ x y T)) = T.
 Proof.
   apply* subst_undo_typ_dec.
 Qed.
 
 Lemma subst_trm_undo: forall x y t,
-  y \notin fv_trm t -> (subst_trm y (in_ctx x) (subst_trm x (in_ctx y) t)) = t.
+  y \notin fv_trm t -> (subst_trm y x (subst_trm x y t)) = t.
 Proof.
   apply* subst_undo_trm_val_def_defs.
-Qed.
-
-Lemma subst_idempotent_fvar: forall x y,
-  (forall v, (subst_fvar x y (subst_fvar x y v)) = (subst_fvar x y v)).
-Proof.
-  intros. unfold subst_fvar; destruct v.
-  + reflexivity.
-  + case_if; eauto; destruct y; eauto; case_if; eauto.
 Qed.
 
 Lemma subst_idempotent_avar: forall x y,
   (forall a, (subst_avar x y (subst_avar x y a)) = (subst_avar x y a)).
 Proof.
-  intros. unfold subst_avar; destruct a.
+  intros. unfold subst_avar, subst_fvar, open_avar, open_rec_avar; destruct a.
   + reflexivity.
-  + f_equal. apply* subst_idempotent_fvar.
+  + repeat case_if; reflexivity.
 Qed.
 
 Lemma subst_idempotent_typ_dec: forall x y,
@@ -1237,16 +988,235 @@ Proof.
 Qed.
 
 (* ###################################################################### *)
+(** ** The substitution principle *)
+
+Lemma subst_rules: forall y S,
+  (forall m1 m2 G t T, ty_trm m1 m2 G t T -> forall G1 G2 x,
+    G = G1 & x ~ S & G2 ->
+    ok (G1 & x ~ S & G2) ->
+    x \notin fv_ctx_types G1 ->
+    ty_trm ty_general sub_general (G1 & (subst_ctx x y G2)) (trm_var (avar_f y)) (subst_typ x y S) ->
+    m1 = ty_general ->
+    m2 = sub_general ->
+    ty_trm m1 m2 (G1 & (subst_ctx x y G2)) (subst_trm x y t) (subst_typ x y T)) /\
+  (forall G d D, ty_def G d D -> forall G1 G2 x,
+    G = G1 & x ~ S & G2 ->
+    ok (G1 & x ~ S & G2) ->
+    x \notin fv_ctx_types G1 ->
+    ty_trm ty_general sub_general (G1 & (subst_ctx x y G2)) (trm_var (avar_f y)) (subst_typ x y S) ->
+    ty_def (G1 & (subst_ctx x y G2)) (subst_def x y d) (subst_dec x y D)) /\
+  (forall G ds T, ty_defs G ds T -> forall G1 G2 x,
+    G = G1 & x ~ S & G2 ->
+    ok (G1 & x ~ S & G2) ->
+    x \notin fv_ctx_types G1 ->
+    ty_trm ty_general sub_general (G1 & (subst_ctx x y G2)) (trm_var (avar_f y)) (subst_typ x y S) ->
+    ty_defs (G1 & (subst_ctx x y G2)) (subst_defs x y ds) (subst_typ x y T)) /\
+  (forall m1 m2 G T U, subtyp m1 m2 G T U -> forall G1 G2 x,
+    G = G1 & x ~ S & G2 ->
+    ok (G1 & x ~ S & G2) ->
+    x \notin fv_ctx_types G1 ->
+    ty_trm ty_general sub_general (G1 & (subst_ctx x y G2)) (trm_var (avar_f y)) (subst_typ x y S) ->
+    m1 = ty_general ->
+    m2 = sub_general ->
+    subtyp m1 m2 (G1 & (subst_ctx x y G2)) (subst_typ x y T) (subst_typ x y U)).
+Proof.
+  intros y S. apply rules_mutind; intros; subst.
+  - (* ty_var *)
+    simpl. case_if.
+    + apply binds_middle_eq_inv in b. subst. assumption. assumption.
+    + apply subst_fresh_ctx with (y:=y) in H1.
+      apply binds_subst in b.
+      apply ty_var. rewrite <- H1.
+      unfold subst_ctx. rewrite <- map_concat.
+      apply binds_map. assumption. assumption.
+  - (* ty_all_intro *)
+    simpl.
+    apply_fresh ty_all_intro as z; eauto.
+    assert (z \notin L) as FrL by eauto.
+    assert (subst_fvar x y z = z) as A. {
+      unfold subst_fvar. rewrite If_r. reflexivity. eauto.
+    }
+    rewrite <- A at 2. rewrite <- subst_open_commute_trm.
+    rewrite <- A at 3. rewrite <- subst_open_commute_typ.
+    assert (subst_ctx x y G2 & z ~ subst_typ x y T = subst_ctx x y (G2 & z ~ T)) as B. {
+      unfold subst_ctx. rewrite map_concat. rewrite map_single. reflexivity.
+    }
+    rewrite <- concat_assoc. rewrite B.
+    eapply H; eauto.
+    rewrite concat_assoc. reflexivity.
+    rewrite concat_assoc. apply ok_push. assumption. eauto.
+    rewrite <- B. rewrite concat_assoc. apply weaken_ty_trm. assumption.
+    apply ok_push. apply ok_concat_map. eauto. unfold subst_ctx. eauto.
+  - (* ty_all_elim *)
+    simpl. rewrite subst_open_commute_typ.
+    eapply ty_all_elim.
+    simpl in H.
+    apply H; eauto.
+    apply H0; eauto.
+  - (* ty_new_intro *)
+    simpl.
+    apply_fresh ty_new_intro as z; eauto.
+    assert (z \notin L) as FrL by eauto.
+    assert (subst_fvar x y z = z) as A. {
+      unfold subst_fvar. rewrite If_r. reflexivity. eauto.
+    }
+    rewrite <- A at 2. rewrite <- A at 3. rewrite <- A at 4.
+    rewrite <- subst_open_commute_typ. rewrite <- subst_open_commute_defs.
+    assert (subst_ctx x y G2 & z ~ subst_typ x y (open_typ z T) = subst_ctx x y (G2 & z ~ open_typ z T)) as B. {
+      unfold subst_ctx. rewrite map_concat. rewrite map_single. reflexivity.
+    }
+    rewrite <- concat_assoc. rewrite B.
+    apply H; eauto.
+    rewrite concat_assoc. reflexivity.
+    rewrite concat_assoc. apply ok_push. assumption. eauto.
+    rewrite <- B. rewrite concat_assoc. apply weaken_ty_trm. assumption.
+    apply ok_push. apply ok_concat_map. eauto. unfold subst_ctx. eauto.
+  - (* ty_new_elim *)
+    simpl. apply ty_new_elim.
+    apply H; eauto.
+  - (* ty_let *)
+    simpl.
+    apply_fresh ty_let as z; eauto.
+    assert (subst_ctx x y G2 & z ~ subst_typ x y T = subst_ctx x y (G2 & z ~ T)) as B. {
+      unfold subst_ctx. rewrite map_concat. rewrite map_single. reflexivity.
+    }
+    rewrite <- concat_assoc. rewrite B.
+    assert (subst_fvar x y z = z) as A. {
+      unfold subst_fvar. rewrite If_r. reflexivity. eauto.
+    }
+    rewrite <- A at 2. rewrite <- subst_open_commute_trm.
+    apply H0 with (x0:=z); eauto.
+    rewrite concat_assoc. reflexivity.
+    rewrite concat_assoc. apply ok_push. assumption. eauto.
+    rewrite <- B. rewrite concat_assoc. apply weaken_ty_trm. assumption.
+    apply ok_push. apply ok_concat_map. eauto. unfold subst_ctx. eauto.
+  - (* ty_rec_intro *)
+    simpl. apply ty_rec_intro.
+    assert (trm_var (avar_f (If x = x0 then y else x)) = subst_trm x0 y (trm_var (avar_f x))) as A. {
+      simpl. reflexivity.
+    }
+    rewrite A.
+    assert (open_typ (If x = x0 then y else x) (subst_typ x0 y T) = subst_typ x0 y (open_typ x T)) as B. {
+      rewrite subst_open_commute_typ. unfold subst_fvar. reflexivity.
+    }
+    rewrite B.
+    apply H; eauto.
+  - (* ty_rec_elim *)
+    simpl. rewrite subst_open_commute_typ.
+    apply ty_rec_elim.
+    apply H; eauto.
+  - (* ty_and_intro *)
+    simpl.
+    assert (trm_var (avar_f (If x = x0 then y else x)) = subst_trm x0 y (trm_var (avar_f x))) as A. {
+      simpl. reflexivity.
+    }
+    rewrite A.
+    apply ty_and_intro; eauto.
+  - (* ty_sub *)
+    eapply ty_sub; eauto.
+    intro Contra. inversion Contra.
+  - (* ty_def_typ *)
+    simpl. apply ty_def_typ; eauto.
+  - (* ty_def_trm *)
+    simpl. apply ty_def_trm; eauto.
+  - (* ty_defs_one *)
+    simpl. apply ty_defs_one; eauto.
+  - (* ty_defs_cons *)
+    simpl. apply ty_defs_cons; eauto.
+    rewrite <- subst_label_of_def.
+    apply subst_defs_hasnt. assumption.
+  - (* subtyp_top *)
+    apply subtyp_top.
+  - (* subtyp_bot *)
+    apply subtyp_bot.
+  - (* subtyp_refl *)
+    apply subtyp_refl.
+  - (* subtyp_trans *)
+    eapply subtyp_trans; eauto.
+  - (* subtyp_and11 *)
+    eapply subtyp_and11; eauto.
+  - (* subtyp_and12 *)
+    eapply subtyp_and12; eauto.
+  - (* subtyp_and2 *)
+    eapply subtyp_and2; eauto.
+  - (* subtyp_fld *)
+    eapply subtyp_fld; eauto.
+  - (* subtyp_typ *)
+    eapply subtyp_typ; eauto.
+  - (* subtyp_sel2 *)
+    eapply subtyp_sel2; eauto.
+    eapply H; eauto.
+  - (* subtyp_sel1 *)
+    eapply subtyp_sel1; eauto.
+    eapply H; eauto.
+  - (* subtyp_sel2_tight *) inversion H5.
+  - (* subtyp_sel1_tight *) inversion H5.
+  - (* subtyp_all *)
+    simpl. apply_fresh subtyp_all as z; eauto.
+    assert (z \notin L) as FrL by eauto.
+    assert (subst_fvar x y z = z) as A. {
+      unfold subst_fvar. rewrite If_r. reflexivity. eauto.
+    }
+    rewrite <- A at 2. rewrite <- A at 3.
+    rewrite <- subst_open_commute_typ. rewrite <- subst_open_commute_typ.
+    assert (subst_ctx x y G2 & z ~ subst_typ x y S2 = subst_ctx x y (G2 & z ~ S2)) as B. {
+      unfold subst_ctx. rewrite map_concat. rewrite map_single. reflexivity.
+    }
+    rewrite <- concat_assoc. rewrite B.
+    apply H0; eauto.
+    rewrite concat_assoc. reflexivity.
+    rewrite concat_assoc. apply ok_push. assumption. eauto.
+    rewrite <- B. rewrite concat_assoc. apply weaken_ty_trm. assumption.
+    apply ok_push. apply ok_concat_map. eauto. unfold subst_ctx. eauto.
+Qed.
+
+Lemma subst_ty_trm: forall y S G x t T,
+    ty_trm ty_general sub_general (G & x ~ S) t T -> 
+    ok (G & x ~ S) ->
+    x \notin fv_ctx_types G ->
+    ty_trm ty_general sub_general G (trm_var (avar_f y)) (subst_typ x y S) ->
+    ty_trm ty_general sub_general G (subst_trm x y t) (subst_typ x y T).
+Proof.
+  intros.
+  apply (proj51 (subst_rules y S)) with (G1:=G) (G2:=empty) (x:=x) in H.
+  unfold subst_ctx in H. rewrite map_empty in H. rewrite concat_empty_r in H.
+  apply H.
+  rewrite concat_empty_r. reflexivity.
+  rewrite concat_empty_r. assumption.
+  assumption.
+  unfold subst_ctx. rewrite map_empty. rewrite concat_empty_r. assumption.
+  reflexivity.
+  reflexivity.
+Qed.
+
+Lemma subst_ty_defs: forall y S G x ds T,
+    ty_defs (G & x ~ S) ds T ->
+    ok (G & x ~ S) ->
+    x \notin fv_ctx_types G ->
+    ty_trm ty_general sub_general G (trm_var (avar_f y)) (subst_typ x y S) ->
+    ty_defs G (subst_defs x y ds) (subst_typ x y T).
+Proof.
+  intros.
+  apply (proj53 (subst_rules y S)) with (G1:=G) (G2:=empty) (x:=x) in H.
+  unfold subst_ctx in H. rewrite map_empty in H. rewrite concat_empty_r in H.
+  apply H.
+  rewrite concat_empty_r. reflexivity.
+  rewrite concat_empty_r. assumption.
+  assumption.
+  unfold subst_ctx. rewrite map_empty. rewrite concat_empty_r. assumption.
+Qed.
+
+(* ###################################################################### *)
 (** ** Some Lemmas *)
 
-Lemma corresponding_types: forall Gs s x T,
-  wf_sto Gs s ->
-  binds x T Gs ->
+Lemma corresponding_types: forall G s x T,
+  wf_sto G s ->
+  binds x T G ->
   ((exists S U t, binds x (val_lambda S t) s /\
-                  ty_trm ty_precise Gs empty (trm_val (val_lambda S t)) (typ_all S U) /\
+                  ty_trm ty_precise sub_general G (trm_val (val_lambda S t)) (typ_all S U) /\
                   T = typ_all S U) \/
    (exists S ds, binds x (val_new S ds) s /\
-                 ty_trm ty_precise Gs empty (trm_val (val_new S ds)) (typ_bnd S) /\
+                 ty_trm ty_precise sub_general G (trm_val (val_new S ds)) (typ_bnd S) /\
                  T = typ_bnd S)).
 Proof.
   introv H Bi. induction H.
@@ -1255,16 +1225,14 @@ Proof.
     + inversions Bi. inversion H2; subst.
       * left. exists T0. exists U. exists t.
         split. auto. split.
-        eapply weaken_sto_ty_trm. assumption.
-        apply ok_push. eapply wf_sto_to_ok_G. eassumption. assumption.
+        apply weaken_ty_trm. assumption. apply ok_push. eapply wf_sto_to_ok_G. eassumption. assumption.
         reflexivity.
       * right. exists T0. exists ds.
         split. auto. split.
-        eapply weaken_sto_ty_trm. assumption.
-        apply ok_push. eapply wf_sto_to_ok_G. eassumption. assumption.
+        apply weaken_ty_trm. assumption. apply ok_push. eapply wf_sto_to_ok_G. eassumption. assumption.
         reflexivity.
       * assert (exists x, trm_val v = trm_var (avar_f x)) as A. {
-          apply H3. discriminate.
+          apply H3. reflexivity.
         }
         destruct A as [? A]. inversion A.
     + specialize (IHwf_sto Bi).
@@ -1272,69 +1240,74 @@ Proof.
       * destruct IH as [S [U [t [IH1 [IH2 IH3]]]]].
         left. exists S. exists U. exists t.
         split. assumption. split.
-        eapply weaken_sto_ty_trm. assumption.
-        apply ok_push. eapply wf_sto_to_ok_G. eassumption. assumption.
+        apply weaken_ty_trm. assumption. apply ok_push. eapply wf_sto_to_ok_G. eassumption. assumption.
         assumption.
       * destruct IH as [S [ds [IH1 [IH2 IH3]]]].
         right. exists S. exists ds.
         split. assumption. split.
-        eapply weaken_sto_ty_trm. assumption.
-        apply ok_push. eapply wf_sto_to_ok_G. eassumption. assumption.
+        apply weaken_ty_trm. assumption. apply ok_push. eapply wf_sto_to_ok_G. eassumption. assumption.
         assumption.
 Qed.
 
-Lemma unique_rec_subtyping: forall Gs G S T,
-  subtyp ty_precise Gs G (typ_bnd S) T ->
+Lemma unique_rec_subtyping: forall G S T,
+  subtyp ty_precise sub_general G (typ_bnd S) T ->
   T = typ_bnd S.
 Proof.
   introv Hsub.
   remember (typ_bnd S) as T'.
-  remember ty_precise as m.
-  induction Hsub; try solve [subst; false].
-  - specialize (IHHsub1 HeqT' Heqm). subst.
+  remember ty_precise as m1.
+  remember sub_general as m2.
+  induction Hsub; try solve [inversion Heqm1].
+  - specialize (IHHsub1 HeqT' Heqm1 Heqm2). subst.
     apply IHHsub2; reflexivity.
+  - inversion HeqT'.
+  - inversion HeqT'.
 Qed.
 
-Lemma unique_all_subtyping: forall G Gs S U T,
-  subtyp ty_precise G Gs (typ_all S U) T ->
+Lemma unique_all_subtyping: forall G S U T,
+  subtyp ty_precise sub_general G (typ_all S U) T ->
   T = typ_all S U.
 Proof.
   introv Hsub.
   remember (typ_all S U) as T'.
-  remember ty_precise as m.
-  induction Hsub; try solve [subst; false].
-  - specialize (IHHsub1 HeqT' Heqm). subst.
+  remember ty_precise as m1.
+  remember sub_general as m2.
+  induction Hsub; try solve [inversion Heqm1].
+  - specialize (IHHsub1 HeqT' Heqm1 Heqm2). subst.
     apply IHHsub2; reflexivity.
+  - inversion HeqT'.
+  - inversion HeqT'.
 Qed.
 
-Lemma unique_lambda_typing: forall G Gs x S U T,
+Lemma unique_lambda_typing: forall G x S U T,
   binds x (typ_all S U) G ->
-  ty_trm ty_precise G Gs (trm_var (avar_s x)) T ->
+  ty_trm ty_precise sub_general G (trm_var (avar_f x)) T ->
   T = typ_all S U.
 Proof.
   introv Bi Hty.
-  remember (trm_var (avar_s x)) as t.
-  remember ty_precise as m.
-  induction Hty; try solve [subst; false].
+  remember (trm_var (avar_f x)) as t.
+  remember ty_precise as m1.
+  remember sub_general as m2.
+  induction Hty; try solve [inversion Heqt; inversion Heqm1].
   - inversions Heqt.
     unfold binds in Bi. unfold binds in H.
     rewrite H in Bi. inversion Bi.
     reflexivity.
-  - specialize (IHHty Bi Heqt Heqm).
+  - specialize (IHHty Bi Heqt Heqm1 Heqm2).
     inversion IHHty.
-  - specialize (IHHty Bi Heqt Heqm).
-    rewrite IHHty in H0. rewrite Heqm in H0.
+  - specialize (IHHty Bi Heqt Heqm1 Heqm2).
+    rewrite IHHty in H0. rewrite Heqm1 in H0. rewrite Heqm2 in H0.
     apply unique_all_subtyping in H0.
     apply H0.
 Qed.
 
-Lemma lambda_not_rcd: forall G Gs x S U A T1 T2,
+Lemma lambda_not_rcd: forall G x S U A T,
   binds x (typ_all S U) G ->
-  ty_trm ty_precise G Gs (trm_var (avar_s x)) (typ_rcd (dec_typ A T1 T2)) ->
+  ty_trm ty_precise sub_general G (trm_var (avar_f x)) (typ_rcd (dec_typ A T T)) ->
   False.
 Proof.
   introv Bi Hty.
-  assert (typ_rcd (dec_typ A T1 T2) = typ_all S U) as Contra. {
+  assert (typ_rcd (dec_typ A T T) = typ_all S U) as Contra. {
     eapply unique_lambda_typing; eassumption.
   }
   inversion Contra.
@@ -1386,13 +1359,12 @@ Proof.
     rewrite <- open_dec_preserves_label. assumption.
 Qed.
 
-Lemma open_eq_avar: forall v x i a1 a2,
-  x = var_of v ->
+Lemma open_eq_avar: forall x i a1 a2,
   x \notin fv_avar a1 -> x \notin fv_avar a2 ->
-  open_rec_avar i v a1 = open_rec_avar i v a2 ->
+  open_rec_avar i x a1 = open_rec_avar i x a2 ->
   a1 = a2.
 Proof.
-  introv Eq Fr1 Fr2 H. induction a1; induction a2; simpl in H; inversion H.
+  introv Fr1 Fr2 H. induction a1; induction a2; simpl in H; inversion H.
   - case_if; case_if.
     + reflexivity.
     + inversion H. subst. reflexivity.
@@ -1405,18 +1377,17 @@ Proof.
   - subst. reflexivity.
 Qed.
 
-Lemma open_eq_typ_dec: forall v x,
-  x = var_of v ->
+Lemma open_eq_typ_dec: forall x,
   (forall T1, x \notin fv_typ T1 ->
    forall T2, x \notin fv_typ T2 ->
-   forall i, open_rec_typ i v T1 = open_rec_typ i v T2 ->
+   forall i, open_rec_typ i x T1 = open_rec_typ i x T2 ->
    T1 = T2) /\
   (forall D1, x \notin fv_dec D1 ->
    forall D2, x \notin fv_dec D2 ->
-   forall i, open_rec_dec i v D1 = open_rec_dec i v D2 ->
+   forall i, open_rec_dec i x D1 = open_rec_dec i x D2 ->
    D1 = D2).
 Proof.
-  introv Eq. apply typ_mutind; intros.
+  intros. apply typ_mutind; intros.
   - simpl in H1. induction T2; simpl in H1; inversion H1.
     reflexivity.
   - simpl in H1. induction T2; simpl in H1; inversion H1.
@@ -1447,22 +1418,21 @@ Proof.
     eapply H; eauto.
 Qed.
 
-Lemma open_eq_typ: forall v x i T1 T2,
-  x = var_of v ->
+Lemma open_eq_typ: forall x i T1 T2,
   x \notin fv_typ T1 -> x \notin fv_typ T2 ->
-  open_rec_typ i v T1 = open_rec_typ i v T2 ->
+  open_rec_typ i x T1 = open_rec_typ i x T2 ->
   T1 = T2.
 Proof.
-  introv Eq Fr1 Fr2 Heq.
-  destruct (open_eq_typ_dec v Eq) as [HT HD].
+  introv Fr1 Fr2 Heq.
+  destruct (open_eq_typ_dec x) as [HT HD].
   eapply HT; eauto.
 Qed.
 
-Lemma open_record_dec_rev: forall v D,
-  (var_of v) \notin fv_dec D ->
-  record_dec (open_dec v D) -> record_dec D.
+Lemma open_record_dec_rev: forall D x,
+  x \notin fv_dec D ->
+  record_dec (open_dec x D) -> record_dec D.
 Proof.
-  introv Fr H. remember (open_dec v D) as DX.
+  introv Fr H. remember (open_dec x D) as DX.
   generalize dependent D.
   inversion H; intros.
   - destruct D; unfold open_dec in HeqDX; simpl in HeqDX; inversion HeqDX.
@@ -1474,11 +1444,11 @@ Proof.
     subst. constructor.
 Qed.
 
-Lemma open_record_typ_rev: forall v T ls,
-   (var_of v) \notin fv_typ T ->
-  record_typ (open_typ v T) ls -> record_typ T ls.
+Lemma open_record_typ_rev: forall T x ls,
+   x \notin fv_typ T ->
+  record_typ (open_typ x T) ls -> record_typ T ls.
 Proof.
-  introv Fr H. remember (open_typ v T) as TX.
+  introv Fr H. remember (open_typ x T) as TX.
   generalize dependent T.
   induction H; intros.
   - destruct T; unfold open_typ in HeqTX; simpl in HeqTX; inversion HeqTX.
@@ -1498,28 +1468,28 @@ Proof.
     rewrite <- open_dec_preserves_label in H2. apply H2.
 Qed.
 
-Lemma open_record_type: forall v T,
-  record_type T -> record_type (open_typ v T).
+Lemma open_record_type: forall T x,
+  record_type T -> record_type (open_typ x T).
 Proof.
   intros. destruct H as [ls H]. exists ls. eapply open_record_typ.
   eassumption.
 Qed.
 
-Lemma open_record_type_rev: forall v T,
-  (var_of v) \notin fv_typ T ->
-  record_type (open_typ v T) -> record_type T.
+Lemma open_record_type_rev: forall T x,
+  x \notin fv_typ T ->
+  record_type (open_typ x T) -> record_type T.
 Proof.
   introv Fr H. destruct H as [ls H]. exists ls. eapply open_record_typ_rev; eauto.
 Qed.
 
-Lemma label_same_typing: forall s G d D,
-  ty_def s G d D -> label_of_def d = label_of_dec D.
+Lemma label_same_typing: forall G d D,
+  ty_def G d D -> label_of_def d = label_of_dec D.
 Proof.
   intros. inversion H; subst; simpl; reflexivity.
 Qed.
 
-Lemma record_defs_typing_rec: forall s G ds S,
-  ty_defs s G ds S ->
+Lemma record_defs_typing_rec: forall G ds S,
+  ty_defs G ds S ->
   exists ls, record_typ S ls /\ forall l, l \notin ls <-> defs_hasnt ds l.
 Proof.
   intros. induction H.
@@ -1562,8 +1532,8 @@ Proof.
         apply notin_singleton. eauto.
 Qed.
 
-Lemma record_defs_typing: forall s G ds S,
-  ty_defs s G ds S ->
+Lemma record_defs_typing: forall G ds S,
+  ty_defs G ds S ->
   record_type S.
 Proof.
   intros.
@@ -1573,18 +1543,18 @@ Proof.
   exists ls. apply A1.
 Qed.
 
-Lemma record_new_typing: forall s G S ds,
-  ty_trm ty_precise s G (trm_val (val_new S ds)) (typ_bnd S) ->
+Lemma record_new_typing: forall G S ds,
+  ty_trm ty_precise sub_general G (trm_val (val_new S ds)) (typ_bnd S) ->
   record_type S.
 Proof.
   intros.
   inversion H; subst.
   + pick_fresh x.
-    apply open_record_type_rev with (v:= in_ctx x).
-    unfold var_of. eauto.
+    apply open_record_type_rev with (x:=x).
+    eauto.
     eapply record_defs_typing. eapply H4. eauto.
   + assert (exists x, trm_val (val_new S ds) = trm_var (avar_f x)) as Contra. {
-      apply H0; eauto. discriminate.
+      apply H0; eauto.
     }
     destruct Contra as [? Contra]. inversion Contra.
 Qed.
@@ -1658,13 +1628,12 @@ Proof.
     + apply rs_pick. apply IHrecord_sub. assumption.
 Qed.
 
-Lemma record_subtyping: forall s G T T',
-  subtyp ty_precise s G T T' ->
+Lemma record_subtyping: forall G T T',
+  subtyp ty_precise sub_general G T T' ->
   record_type T ->
   record_sub T T'.
 Proof.
-  introv Hsub Hr. generalize dependent Hr.
-  dependent induction Hsub; try solve [false].
+  introv Hsub Hr. generalize dependent Hr. dependent induction Hsub.
   - intros HS.
     apply record_sub_trans with (T2:=T).
     apply IHHsub1. apply HS.
@@ -1676,24 +1645,6 @@ Proof.
   - intros Htype. destruct Htype as [ls Htyp].
     inversion Htyp; subst.
     eapply rs_dropl. apply rs_refl.
-Qed.
-
-Lemma record_subtyping_inv: forall Gs G T T',
-  record_sub T T' ->
-  subtyp ty_general Gs G T T'.
-Proof.
-  introv Hsub.
-  dependent induction Hsub; try solve [false].
-  - apply subtyp_refl. discriminate.
-  - apply subtyp_and12.
-  - apply subtyp_trans with (T:=T).
-    apply subtyp_and11.
-    apply IHHsub.
-  - apply subtyp_and2. discriminate.
-    eapply subtyp_trans with (T:=T).
-    apply subtyp_and11.
-    apply IHHsub.
-    apply subtyp_and12.
 Qed.
 
 Lemma record_typ_sub_label_in: forall T D ls,
@@ -1730,48 +1681,35 @@ Proof.
   - eapply IHHtyp; eassumption.
 Qed.
 
-Lemma rcd_typ_eq: forall T A T1 T2,
-  record_type T ->
-  record_sub T (typ_rcd (dec_typ A T1 T2)) ->
-  T1 = T2.
-Proof.
-  introv Htype Hsub.
-  generalize dependent T2. generalize dependent T1. generalize dependent A.
-  destruct Htype as [ls Htyp].
-  induction Htyp; intros; inversion Hsub; subst; eauto;
-  try solve [inversion H; subst; reflexivity].
-Qed.
-
-Lemma record_type_sub_not_rec: forall S T v,
-  record_sub (open_typ v S) (typ_bnd T) ->
+Lemma record_type_sub_not_rec: forall S T x,
+  record_sub (open_typ x S) (typ_bnd T) ->
   record_type S ->
   False.
 Proof.
-  introv Hsub Htype. remember (open_typ v S) as Sx.
-  apply open_record_type with (v:=v) in Htype.
+  introv Hsub Htype. remember (open_typ x S) as Sx.
+  apply open_record_type with (x:=x) in Htype.
   rewrite <- HeqSx in Htype. clear HeqSx.
   destruct Htype as [ls Htyp]. induction Htyp.
   - inversion Hsub.
   - inversion Hsub; subst. apply IHHtyp. assumption.
 Qed.
 
-Lemma shape_new_typing: forall Gs G x S T,
-  binds x (typ_bnd S) Gs ->
+Lemma shape_new_typing: forall G x S T,
+  binds x (typ_bnd S) G ->
   record_type S ->
-  ty_trm ty_precise Gs G (trm_var (avar_s x)) T ->
-  T = typ_bnd S \/ record_sub (open_typ (in_sto x) S) T.
+  ty_trm ty_precise sub_general G (trm_var (avar_f x)) T ->
+  T = typ_bnd S \/ record_sub (open_typ x S) T.
 Proof.
-  introv Bi HS Hx.
-  dependent induction Hx; try solve [false].
+  introv Bi HS Hx. dependent induction Hx.
   - unfold binds in H. unfold binds in Bi. rewrite H in Bi. inversion Bi.
     left. reflexivity.
-  - assert (typ_bnd T = typ_bnd S \/ record_sub (open_typ (in_sto x) S) (typ_bnd T)) as A. {
+  - assert (typ_bnd T = typ_bnd S \/ record_sub (open_typ x S) (typ_bnd T)) as A. {
       eapply IHHx; eauto.
     }
     destruct A as [A | A].
     + inversion A. right. apply rs_refl.
     + apply record_type_sub_not_rec in A. inversion A. assumption.
-  - assert (T = typ_bnd S \/ record_sub (open_typ (in_sto x) S) T) as A. {
+  - assert (T = typ_bnd S \/ record_sub (open_typ x S) T) as A. {
       eapply IHHx; eauto.
     }
     destruct A as [A | A].
@@ -1782,15 +1720,15 @@ Proof.
       eapply open_record_type. assumption.
 Qed.
 
-Lemma unique_tight_bounds: forall Gs s x T1 T2 A,
-  wf_sto Gs s ->
-  ty_trm ty_precise Gs empty (trm_var (avar_s x)) (typ_rcd (dec_typ A T1 T1)) ->
-  ty_trm ty_precise Gs empty (trm_var (avar_s x)) (typ_rcd (dec_typ A T2 T2)) ->
+Lemma unique_tight_bounds: forall G s x T1 T2 A,
+  wf_sto G s ->
+  ty_trm ty_precise sub_general G (trm_var (avar_f x)) (typ_rcd (dec_typ A T1 T1)) ->
+  ty_trm ty_precise sub_general G (trm_var (avar_f x)) (typ_rcd (dec_typ A T2 T2)) ->
   T1 = T2.
 Proof.
   introv Hwf Hty1 Hty2.
-  assert (exists T, binds x T Gs) as Bi. {
-    eapply typing_implies_sto_bound. eassumption.
+  assert (exists T, binds x T G) as Bi. {
+    eapply typing_implies_bound. eassumption.
   }
   destruct Bi as [T Bi].
   destruct (corresponding_types Hwf Bi).
@@ -1806,7 +1744,7 @@ Proof.
     inversion Contra1.
     destruct (shape_new_typing Bi Htype Hty2) as [Contra2 | A2].
     inversion Contra2.
-    assert (record_type (open_typ (in_sto x) S)) as HXtype. {
+    assert (record_type (open_typ x S)) as HXtype. {
       apply open_record_type. assumption.
     }
     eapply unique_rcd_typ.
@@ -1815,92 +1753,79 @@ Proof.
     eassumption.
 Qed.
 
-Lemma tight_bounds_eq: forall Gs s x T1 T2 A,
-  wf_sto Gs s ->
-  ty_trm ty_precise Gs empty (trm_var (avar_s x)) (typ_rcd (dec_typ A T1 T2)) ->
-  T1 = T2.
-Proof.
-  introv Hwf Hty.
-  assert (exists T, binds x T Gs) as Bi. {
-    eapply typing_implies_sto_bound. eassumption.
-  }
-  destruct Bi as [T Bi].
-  destruct (corresponding_types Hwf Bi).
-  - destruct H as [S [U [t [Bis [Ht EqT]]]]].
-    false.
-    eapply lambda_not_rcd.
-    subst. eassumption. eassumption.
-  - destruct H as [S [ds [Bis [Ht EqT]]]]. subst.
-    assert (record_type S) as Htype. {
-      eapply record_new_typing. eassumption.
-    }
-    destruct (shape_new_typing Bi Htype Hty) as [Contra1 | A1].
-    inversion Contra1.
-    assert (record_type (open_typ (in_sto x) S)) as HXtype. {
-      apply open_record_type. assumption.
-    }
-    eapply rcd_typ_eq.
-    apply HXtype.
-    eassumption.
-Qed.
-
 Lemma precise_to_general:
-  (forall m Gs G t T,
-     ty_trm m Gs G t T ->
-     m = ty_precise ->
-     ty_trm ty_general Gs G t T) /\
-  (forall m Gs G S U,
-     subtyp m Gs G S U ->
-     m = ty_precise ->
-     subtyp ty_general Gs G S U).
+  (forall m1 m2 G t T,
+     ty_trm m1 m2 G t T ->
+     m1 = ty_precise ->
+     m2 = sub_general ->
+     ty_trm ty_general sub_general G t T) /\
+  (forall m1 m2 G S U,
+     subtyp m1 m2 G S U ->
+     m1 = ty_precise ->
+     m2 = sub_general ->
+     subtyp ty_general sub_general G S U).
 Proof.
-  apply ts_mutind; intros; subst; eauto; try solve [false].
-  eapply ty_sub; eauto.
+  apply ts_mutind; intros; subst; eauto.
 Qed.
 
-Lemma precise_to_general_typing: forall Gs G t T,
-  ty_trm ty_precise Gs G t T ->
-  ty_trm ty_general Gs G t T.
+Lemma precise_to_general_typing: forall G t T,
+  ty_trm ty_precise sub_general G t T ->
+  ty_trm ty_general sub_general G t T.
 Proof.
   intros. apply* precise_to_general.
 Qed.
 
 Lemma tight_to_general:
-  (forall m Gs G t T,
-     ty_trm m Gs G t T -> forall n,
-     m = ty_tight n ->
-     ty_trm ty_general Gs G t T) /\
-  (forall m Gs G S U,
-     subtyp m Gs G S U -> forall n,
-     m = ty_tight n ->
-     subtyp ty_general Gs G S U).
+  (forall m1 m2 G t T,
+     ty_trm m1 m2 G t T ->
+     m1 = ty_general ->
+     m2 = sub_tight ->
+     ty_trm ty_general sub_general G t T) /\
+  (forall m1 m2 G S U,
+     subtyp m1 m2 G S U ->
+     m1 = ty_general ->
+     m2 = sub_tight ->
+     subtyp ty_general sub_general G S U).
 Proof.
-  apply ts_mutind; intros; subst; eauto;
-  try solve [econstructor; eauto; try discriminate; try reflexivity].
-  eapply subtyp_and2; eauto; discriminate.
-  eapply subtyp_fld; eauto; discriminate.
-  eapply subtyp_typ; eauto; discriminate.
-  eapply subtyp_sel2_c; eauto; discriminate.
-  eapply subtyp_sel1_c; eauto; discriminate.
-
-  - destruct o as [[Contra ?] | [? ?]]. inversion Contra. subst.
-    eapply subtyp_sel2_s; eauto. discriminate.
-    eapply precise_to_general_typing. eassumption.
-
-  - destruct o as [[Contra ?] | [? ?]]. inversion Contra. subst.
-    eapply subtyp_sel1_s; eauto. discriminate.
-    eapply precise_to_general_typing. eassumption.
-
-  - apply_fresh subtyp_all as z; eauto; try discriminate.
-
-  - apply_fresh subtyp_bnd as z; eauto; try discriminate.
+  apply ts_mutind; intros; subst; eauto.
+  - apply precise_to_general in t; eauto.
+  - apply precise_to_general in t; eauto.
 Qed.
 
-Lemma tight_to_general_subtyping: forall n Gs G S U,
-  subtyp (ty_tight n) Gs G S U ->
-  subtyp ty_general Gs G S U.
+Lemma tight_to_general_typing: forall G t T,
+  ty_trm ty_general sub_tight G t T ->
+  ty_trm ty_general sub_general G t T.
 Proof.
   intros. apply* tight_to_general.
+Qed.
+
+Lemma tight_to_general_subtyping: forall G S U,
+  subtyp ty_general sub_tight G S U ->
+  subtyp ty_general sub_general G S U.
+Proof.
+  intros. apply* tight_to_general.
+Qed.
+
+Lemma precise_to_tight:
+  (forall m1 m2 G t T,
+     ty_trm m1 m2 G t T ->
+     m1 = ty_precise ->
+     m2 = sub_general ->
+     ty_trm ty_general sub_tight G t T) /\
+  (forall m1 m2 G S U,
+     subtyp m1 m2 G S U ->
+     m1 = ty_precise ->
+     m2 = sub_general ->
+     subtyp ty_general sub_tight G S U).
+Proof.
+  apply ts_mutind; intros; subst; eauto; inversion H0.
+Qed.
+
+Lemma precise_to_tight_typing: forall G t T,
+  ty_trm ty_precise sub_general G t T ->
+  ty_trm ty_general sub_tight G t T.
+Proof.
+  intros. apply* precise_to_tight.
 Qed.
 
 Lemma sto_binds_to_ctx_binds: forall G s x v,
@@ -1933,7 +1858,7 @@ Qed.
 Lemma record_type_new: forall G s x T ds,
   wf_sto G s ->
   binds x (val_new T ds) s ->
-  record_type (open_typ (in_sto x) T).
+  record_type (open_typ x T).
 Proof.
   introv Hwf Bis.
   destruct (sto_binds_to_ctx_binds Hwf Bis) as [S Bi].
@@ -1949,246 +1874,181 @@ Qed.
 (* ###################################################################### *)
 (** ** Narrowing *)
 
-Inductive subenv(Gs: ctx): ctx -> ctx -> Prop :=
-| se_refl: forall G, subenv Gs G G
-| se_push: forall G1 G2 T1 T2 x,
-  subenv Gs G1 G2 ->
-  subtyp ty_general Gs (G1 & (x ~ T1)) T1 T2 ->
-  subenv Gs (G1 & (x ~ T1)) (G2 & (x ~ T2)).
+Definition subenv(G1 G2: ctx) :=
+  forall x T2, binds x T2 G2 ->
+    binds x T2 G1 \/
+    exists T1,
+      binds x T1 G1 /\ subtyp ty_general sub_general G1 T1 T2.
 
-Lemma subenv_last: forall Gs G x S U,
-  subtyp ty_general Gs G S U ->
+Lemma subenv_push: forall G G' x T,
+  subenv G' G ->
+  ok (G' & x ~ T) ->
+  subenv (G' & x ~ T) (G & x ~ T).
+Proof.
+  intros.
+  unfold subenv. intros xb Tb Bi. apply binds_push_inv in Bi.
+  destruct Bi as [Bi | Bi].
+  + destruct Bi as [Bi1 Bi2]. subst.
+    left. eauto.
+  + destruct Bi as [Bi1 Bi2].
+    unfold subenv in H. specialize (H xb Tb Bi2). destruct H as [Bi' | Bi'].
+    * left. eauto.
+    * right. destruct Bi' as [T' [Bi1' Bi2']].
+      exists T'. split. eauto. apply weaken_subtyp. assumption. eauto.
+Qed.
+
+Lemma subenv_last: forall G x S U,
+  subtyp ty_general sub_general G S U ->
   ok (G & x ~ S) ->
-  subenv Gs (G & x ~ S) (G & x ~ U).
+  subenv (G & x ~ S) (G & x ~ U).
 Proof.
-  intros.
-  eapply se_push.
-  eapply se_refl.
-  apply weaken_subtyp; eauto.
-Qed.
-
-Lemma subenv_last_only: forall Gs x S U,
-  subtyp ty_general Gs empty S U ->
-  subenv Gs (x ~ S) (x ~ U).
-Proof.
-  intros.
-  assert ((@empty typ) & (x ~ S) = (x ~ S)) as A. {
-    rewrite concat_empty_l. reflexivity.
-  }
-  assert ((@empty typ) & (x ~ U) = (x ~ U)) as B. {
-    rewrite concat_empty_l. reflexivity.
-  }
-  rewrite <- A. rewrite <- B.
-  eapply subenv_last; eauto.
-Qed.
-
-Lemma notin_subenv: forall Gs G' G,
-  subenv Gs G' G -> forall x,
-  x # G' ->
-  x # G.
-Proof.
-  introv SE. dependent induction SE; introv N; eauto.
-Qed.
-
-Lemma ok_subenv: forall Gs G' G,
-  subenv Gs G' G ->
-  ok G' ->
-  ok G.
-Proof.
-  introv SE. dependent induction SE; introv Hok.
-  - assumption.
-  - apply ok_push_inv in Hok. destruct Hok as [Hok ?].
-    apply ok_push. apply IHSE. assumption.
-    eapply notin_subenv; eauto.
-Qed.
-
-Lemma restricted_by_same: forall y T G,
-  ok (G & y ~ T) -> forall x G',
-  x <> y ->
-  restricted_by x (G & y ~ T) G' ->
-  restricted_by x G G'.
-Proof.
-  introv Hok N r. inversion r; subst.
-  assert (ok G2) as Hok2. {
-    rewrite H in Hok. eauto.
-  }
-  assert (exists G2A G2B, G2 = G2A & G2B /\ G = G1 & x ~ T0 & G2A) as A. {
-    induction Hok2.
-    + rewrite concat_empty_r in H. apply eq_push_inv in H. destruct H as [? [? ?]]. subst.
-      false.
-    + rewrite concat_assoc in H. apply eq_push_inv in H. destruct H as [? [? ?]]. subst.
-      exists E (x0 ~ v). split; eauto.
-  }
-  destruct A as [G2A [G2B [Eq2 Eq]]].
-  subst.
-  apply lim_ctx with (G2:=G2A).
-  reflexivity.
-Qed.
-
-Lemma restricted_by_skip: forall x y T G G',
-  x <> y ->
-  restricted_by x G G' ->
-  restricted_by x (G & y ~ T) G'.
-Proof.
-  introv N r. inversion r; subst.
-  apply lim_ctx with (G2:=(G2 & y ~ T)).
-  rewrite concat_assoc. reflexivity.
-Qed.
-
-Lemma narrow_restricted_by: forall Gs G0 G,
-  ok G0 ->
-  subenv Gs G0 G -> forall x G',
-  restricted_by x G G' ->
-  exists G0', subenv Gs G0' G' /\ restricted_by x G0 G0'.
-Proof.
-  introv Hok SE. eapply ok_subenv in Hok; eauto.
-  dependent induction SE; intros.
-  - exists G'. split. apply se_refl. assumption.
-  - destruct (classicT (x0 = x)) as [Eq | Ne].
-    + subst. inversion H0; subst.
-      assert (G2 = G0 /\ empty = G3 /\ T2 = T) as A. {
-        eapply concat_ok_eq.
-        rewrite concat_empty_r. eapply H1.
-        rewrite concat_empty_r.
-        eauto.
-      }
-      destruct A as [? [? ?]]. subst.
-      exists (G1 & x ~ T1). split; eauto.
-      eapply se_push; eauto.
-      apply lim_ctx with (G2:=empty). rewrite concat_empty_r. reflexivity.
-    + assert (exists G0', subenv Gs G0' G' /\ restricted_by x0 G1 G0') as A. {
-        eapply IHSE; eauto.
-        eapply restricted_by_same; eauto.
-      }
-      destruct A as [G0' [A1 A2]].
-      exists G0'. split; eauto.
-      eapply restricted_by_skip.
-      eauto. eauto.
+  intros. unfold subenv. intros y T Bi.
+  apply binds_push_inv in Bi. destruct Bi as [Bi | Bi].
+  - destruct Bi. subst. right. exists S. split; eauto.
+    apply weaken_subtyp; eauto.
+  - destruct Bi. left. eauto.
 Qed.
 
 Lemma narrow_rules:
-  (forall m Gs G t T, ty_trm m Gs G t T -> forall G',
-    m = ty_general ->
+  (forall m1 m2 G t T, ty_trm m1 m2 G t T -> forall G',
+    m1 = ty_general ->
+    m2 = sub_general ->
     ok G' ->
-    subenv Gs G' G ->
-    ty_trm m Gs G' t T)
-/\ (forall Gs G d D, ty_def Gs G d D -> forall G',
+    subenv G' G ->
+    ty_trm m1 m2 G' t T)
+/\ (forall G d D, ty_def G d D -> forall G',
     ok G' ->
-    subenv Gs G' G ->
-    ty_def Gs G' d D)
-/\ (forall Gs G ds T, ty_defs Gs G ds T -> forall G',
+    subenv G' G ->
+    ty_def G' d D)
+/\ (forall G ds T, ty_defs G ds T -> forall G',
     ok G' ->
-    subenv Gs G' G ->
-    ty_defs Gs G' ds T)
-/\ (forall m Gs G S U, subtyp m Gs G S U -> forall G',
-    m = ty_general ->
+    subenv G' G ->
+    ty_defs G' ds T)
+/\ (forall m1 m2 G S U, subtyp m1 m2 G S U -> forall G',
+    m1 = ty_general ->
+    m2 = sub_general ->
     ok G' ->
-    subenv Gs G' G ->
-    subtyp m Gs G' S U).
+    subenv G' G ->
+    subtyp m1 m2 G' S U).
 Proof.
-  apply rules_mutind; intros; eauto 4; try solve [false].
+  apply rules_mutind; intros; eauto.
   - (* ty_var *)
-    subst.
-    generalize dependent T. dependent induction H1.
+    subst. unfold subenv in H2. specialize (H2 x T b).
+    destruct H2.
     + eauto.
-    + introv Bi.
-      destruct (classicT (x = x0)) as [Eq | Ne].
-      * subst. eapply binds_push_eq_inv in Bi. subst.
-        eapply ty_sub; eauto 4.
-        intros Contra. false.
-      * assert (ty_trm ty_general Gs G1 (trm_var (avar_c x)) T) as A. {
-          eapply IHsubenv; eauto.
-          eapply binds_push_neq_inv. eassumption. assumption.
-        }
-        eapply weaken_ty_trm. apply A. assumption.
+    + destruct H as [T' [Bi Hsub]].
+      eapply ty_sub; eauto.
   - (* ty_all_intro *)
     subst.
     apply_fresh ty_all_intro as y; eauto.
-    eapply H; eauto.
-    eapply se_push; eauto.
-    apply subtyp_refl. discriminate.
+    eapply H; eauto. apply subenv_push; eauto.
   - (* ty_new_intro *)
     subst.
     apply_fresh ty_new_intro as y; eauto.
-    apply H; eauto.
-    eapply se_push; eauto.
-    apply subtyp_refl. discriminate.
+    apply H; eauto. apply subenv_push; eauto.
   - (* ty_let *)
     subst.
     apply_fresh ty_let as y; eauto.
-    apply H0 with (x:=y); eauto.
-    eapply se_push; eauto.
-    apply subtyp_refl. discriminate.
-  - (* subtyp_sel2_c *) subst.
-    assert (exists G0', subenv Gs G0' G' /\ restricted_by x G'0 G0') as B. {
-      apply narrow_restricted_by with (Gs:=Gs) (G:=G) (G0:=G'0); auto.
-    }
-    destruct B as [G0' [SE' r']].
-    eapply subtyp_sel2_c.
-    discriminate.
-    eapply r'.
-    eapply H; eauto.
-    eapply ok_restricted_by; eauto.
-  - (* subtyp_sel1_c *) subst.
-    assert (exists G0', subenv Gs G0' G' /\ restricted_by x G'0 G0') as B. {
-      apply narrow_restricted_by with (Gs:=Gs) (G:=G) (G0:=G'0); auto.
-    }
-    destruct B as [G0' [SE' r']].
-    eapply subtyp_sel1_c.
-    discriminate.
-    eapply r'.
-    eapply H; eauto.
-    eapply ok_restricted_by; eauto.
-  - (* subtyp_sel2_s *) subst.
-    destruct o as [[? ?] | [Contra ?]]. subst.
-    eapply subtyp_sel2_s.
-    discriminate.
-    left. split; reflexivity.
-    eapply H; eauto.
-    false.
-  - (* subtyp_sel1_s *) subst.
-    destruct o as [[? ?] | [Contra ?]]. subst.
-    eapply subtyp_sel1_s.
-    discriminate.
-    left. split; reflexivity.
-    eapply H; eauto.
-    false.
+    apply H0 with (x:=y); eauto. apply subenv_push; eauto.
+  - inversion H1 (* sub_tight *).
+  - inversion H1 (* sub_tight *).
   - (* subtyp_all *)
     subst.
-    apply_fresh subtyp_all as y; eauto 4.
-    apply H0; eauto. eapply se_push; eauto.
-  - (* subtyp_bnd *)
-    subst.
-    apply_fresh subtyp_bnd as y; eauto 4.
-    apply H; eauto. eapply se_push; eauto.
+    apply_fresh subtyp_all as y; eauto.
+    apply H0; eauto. apply subenv_push; eauto.
 Qed.
 
-Lemma narrow_typing: forall Gs G G' t T,
-  ty_trm ty_general Gs G t T ->
-  subenv Gs G' G -> ok G' ->
-  ty_trm ty_general Gs G' t T.
+Lemma narrow_typing: forall G G' t T,
+  ty_trm ty_general sub_general G t T ->
+  subenv G' G -> ok G' ->
+  ty_trm ty_general sub_general G' t T.
 Proof.
   intros. apply* narrow_rules.
 Qed.
 
-Lemma narrow_subtyping: forall Gs G G' S U,
-  subtyp ty_general Gs G S U ->
-  subenv Gs G' G -> ok G' ->
-  subtyp ty_general Gs G' S U.
+Lemma narrow_subtyping: forall G G' S U,
+  subtyp ty_general sub_general G S U ->
+  subenv G' G -> ok G' ->
+  subtyp ty_general sub_general G' S U.
 Proof.
   intros. apply* narrow_rules.
 Qed.
 
 (* ###################################################################### *)
-(** * misc *)
+(** * Has member *)
 
-Lemma val_new_typing: forall Gs s x T ds,
-  wf_sto Gs s ->
+Inductive has_member: ctx -> var -> typ -> typ_label -> typ -> typ -> Prop :=
+| has_any : forall G x T A S U,
+  ty_trm ty_general sub_tight G (trm_var (avar_f x)) T ->
+  has_member_rules G x T A S U ->
+  has_member G x T A S U
+with has_member_rules: ctx -> var -> typ -> typ_label -> typ -> typ -> Prop :=
+| has_refl : forall G x A S U,
+  has_member_rules G x (typ_rcd (dec_typ A S U)) A S U
+| has_and1 : forall G x T1 T2 A S U,
+  has_member G x T1 A S U ->
+  has_member_rules G x (typ_and T1 T2) A S U
+| has_and2 : forall G x T1 T2 A S U,
+  has_member G x T2 A S U ->
+  has_member_rules G x (typ_and T1 T2) A S U
+| has_bnd : forall G x T A S U,
+  has_member G x (open_typ x T) A S U ->
+  has_member_rules G x (typ_bnd T) A S U
+| has_sel : forall G x y B T' A S U,
+  ty_trm ty_precise sub_general G (trm_var (avar_f y)) (typ_rcd (dec_typ B T' T')) ->
+  has_member G x T' A S U ->
+  has_member_rules G x (typ_sel (avar_f y) B) A S U
+| has_bot  : forall G x A S U,
+  has_member_rules G x typ_bot A S U
+.
+
+Scheme has_mut := Induction for has_member Sort Prop
+with hasr_mut := Induction for has_member_rules Sort Prop.
+Combined Scheme has_mutind from has_mut, hasr_mut.
+
+Lemma has_member_rules_inv: forall G x T A S U, has_member_rules G x T A S U ->
+  (T = typ_rcd (dec_typ A S U)) \/
+  (exists T1 T2, T = typ_and T1 T2 /\
+    (has_member G x T1 A S U \/
+     has_member G x T2 A S U)) \/
+  (exists T', T = typ_bnd T' /\
+    has_member G x (open_typ x T') A S U) \/
+  (exists y B T', T = typ_sel (avar_f y) B /\
+    ty_trm ty_precise sub_general G (trm_var (avar_f y)) (typ_rcd (dec_typ B T' T')) /\
+    has_member G x T' A S U) \/
+  (T = typ_bot).
+Proof.
+  intros. inversion H; subst.
+  - left. eauto.
+  - right. left. exists T1 T2. eauto.
+  - right. left. exists T1 T2. eauto.
+  - right. right. left. exists T0. eauto.
+  - right. right. right. left. exists y B T'. eauto.
+  - right. right. right. right. reflexivity.
+Qed.
+
+Lemma has_member_inv: forall G x T A S U, has_member G x T A S U ->
+  (T = typ_rcd (dec_typ A S U)) \/
+  (exists T1 T2, T = typ_and T1 T2 /\
+    (has_member G x T1 A S U \/
+     has_member G x T2 A S U)) \/
+  (exists T', T = typ_bnd T' /\
+    has_member G x (open_typ x T') A S U) \/
+  (exists y B T', T = typ_sel (avar_f y) B /\
+    ty_trm ty_precise sub_general G (trm_var (avar_f y)) (typ_rcd (dec_typ B T' T')) /\
+    has_member G x T' A S U) \/
+  (T = typ_bot).
+Proof.
+  intros. inversion H; subst. apply has_member_rules_inv in H1. apply H1.
+Qed.
+
+Lemma val_new_typing: forall G s x T ds,
+  wf_sto G s ->
   binds x (val_new T ds) s ->
-  ty_trm ty_precise Gs empty (trm_val (val_new T ds)) (typ_bnd T).
+  ty_trm ty_precise sub_general G (trm_val (val_new T ds)) (typ_bnd T).
 Proof.
   introv Hwf Bis.
-  assert (exists T, binds x T Gs) as Bi. {
+  assert (exists T, binds x T G) as Bi. {
     eapply sto_binds_to_ctx_binds; eauto.
   }
   destruct Bi as [T0 Bi].
@@ -2200,6 +2060,7 @@ Proof.
     inversion Bis. subst.
     assumption.
 Qed.
+
 
 Lemma rcd_typ_eq_bounds: forall T A S U,
   record_type T ->
@@ -2214,87 +2075,222 @@ Proof.
   - apply IHHtyp with (A:=A); eauto.
 Qed.
 
-Lemma exists_bound_restricted_by: forall x T G,
-  binds x T G ->
-  exists G', restricted_by x G G'.
+Lemma has_member_rcd_typ_sub_mut:
+  (forall G x T A S U,
+    has_member G x T A S U ->
+    record_type T ->
+    record_sub T (typ_rcd (dec_typ A S U))) /\
+  (forall G x T A S U,
+    has_member_rules G x T A S U ->
+    record_type T ->
+    record_sub T (typ_rcd (dec_typ A S U))).
 Proof.
-  intros x T.
-  apply (env_ind (fun G => binds x T G -> exists G', restricted_by x G G')).
-  - intro Bi. false. eapply binds_empty_inv; eauto.
-  - introv IH Bi.
-    apply binds_push_inv in Bi. destruct Bi as [[? ?] | [Neq Bi]].
-    + subst. eexists. apply lim_ctx with (G2:=empty).
-      rewrite concat_empty_r. reflexivity.
-    + specialize (IH Bi). destruct IH as [G' IH].
-      exists G'. inversion IH; subst. eapply lim_ctx with (G2:=G2 & x0 ~ v).
-      rewrite concat_assoc. reflexivity.
+  apply has_mutind; intros.
+  - apply H; eauto.
+  - apply rs_refl.
+  - inversion H0; subst. inversion H1; subst. apply rs_drop.
+    apply H; eauto.
+    exists ls. assumption.
+  - inversion H0; subst. inversion H1; subst. inversion h; subst. inversion H3; subst.
+    eapply rs_dropl. eapply rs_refl.
+  - inversion H0. inversion H1.
+  - inversion H0. inversion H1.
+  - destruct H as [ls H]. inversion H.
 Qed.
 
-Lemma precise_fresh_subtyp: forall Gs S U,
-  subtyp ty_precise Gs empty S U -> forall y,
-    y \notin fv_ctx_types Gs ->
-    y \notin fv_typ S ->
-    y \notin fv_typ U.
+Lemma has_member_tightness: forall G s x T ds A S U,
+  wf_sto G s ->
+  binds x (val_new T ds) s ->
+  has_member G x (typ_bnd T) A S U ->
+  S = U.
 Proof.
-  introv Hsub. dependent induction Hsub; intros; eauto;
-  try solve [simpl in H0; apply notin_union_r in H0; destruct H0; assumption];
-  try solve [false].             
-Qed.
-
-Lemma fresh_fv_typ: forall x y,
-  y <> x ->
-  (forall T, y \notin fv_typ T -> forall i,
-    y \notin fv_typ (open_rec_typ i (in_sto x) T)) /\
-  (forall d, y \notin fv_dec d -> forall i,
-    y \notin fv_dec (open_rec_dec i (in_sto x) d)).
-Proof.
-  intros. apply typ_mutind; intros; simpl; eauto; try solve [
-    simpl in H2; eapply notin_union_r in H2; destruct H2;
-    apply notin_union_l; eauto].
-  - simpl. unfold open_rec_avar. destruct a.
-    case_if.
-    + simpl. unfold fv_fvar. simpl. apply notin_singleton. assumption.
-    + simpl. eauto.
-    + simpl. simpl in H0. assumption.
-Qed.
-
-Lemma precise_fresh_ty_trm: forall Gs x T,
-  ty_trm ty_precise Gs empty (trm_var (avar_s x)) T -> forall y,
-    y \notin fv_ctx_types Gs -> y # Gs ->
-    y \notin fv_typ T.
-Proof.
-  introv Hty. dependent induction Hty; intros; eauto; try solve [subst; false].
-  - eapply fv_ctx_types_binds; eauto.
-  - destruct (typing_implies_sto_bound Hty) as [Tx Bi].
-    assert (x <> y) as A. {
-      destruct (classicT (x = y)) as [Eq | Ne].
-      + subst. false. eapply binds_fresh_inv; eauto.
-      + assumption.
-    }
-    assert (y \notin fv_typ (typ_bnd T)) as B. {
-      eapply IHHty; eauto.
-      unfold avar_s. reflexivity.
-    }
-    eapply fresh_fv_typ; eauto.
-  - eapply precise_fresh_subtyp; eauto.
-Qed.
-
-Lemma restricted_by_first: forall x T G2 G',
-  ok (x ~ T & G2) ->
-  restricted_by x (x ~ T & G2) G' ->
-  G' = x ~ T.
-Proof.
-  introv Hok r. inversion r; subst.
-  lets Hok': (ok_restricted_by Hok r).
-  assert (empty = G1 /\ G2 = G0 /\ T = T0) as A. {
-    eapply concat_ok_eq.
-    rewrite concat_empty_l. eapply H.
-    rewrite concat_empty_l. eapply Hok.
+  introv Hwf Bis Hmem.
+  assert (record_type T) as Htype. {
+    eapply record_new_typing. eapply val_new_typing; eauto.
   }
-  destruct A as [A1 [A2 AT]]. subst.
-  rewrite concat_empty_l. reflexivity.
+  assert (record_type (open_typ x T)) as Htypex. {
+    apply open_record_type. assumption.
+  }
+  assert (has_member G x (open_typ x T) A S U) as Hmemx. {
+    inversion Hmem; subst. inversion H0; subst. assumption.
+  }
+  assert (record_sub (open_typ x T) (typ_rcd (dec_typ A S U))) as Hsub. {
+    destruct has_member_rcd_typ_sub_mut as [HL _].
+    eapply HL; eauto.
+  }
+  eapply rcd_typ_eq_bounds. eapply Htypex. eapply Hsub.
 Qed.
 
+Lemma has_member_covariance: forall G s T1 T2 x A S2 U2,
+  wf_sto G s ->
+  subtyp ty_general sub_tight G T1 T2 ->
+  ty_trm ty_general sub_tight G (trm_var (avar_f x)) T1 ->
+  has_member G x T2 A S2 U2 ->
+  exists S1 U1, has_member G x T1 A S1 U1 /\
+                subtyp ty_general sub_tight G S2 S1 /\
+                subtyp ty_general sub_tight G U1 U2.
+Proof.
+  introv Hwf Hsub Hty Hmem.
+  generalize dependent U2.
+  generalize dependent S2.
+  dependent induction Hsub; subst; intros.
+  - (* top *)
+    inversion Hmem; subst. inversion H0.
+  - (* bot *)
+    exists S2 U2. split.
+    apply has_any. assumption. apply has_bot.
+    split; apply subtyp_refl.
+  - (* refl *)
+    exists S2 U2. eauto.
+  - (* trans *)
+    assert (ty_trm ty_general sub_tight G (trm_var (avar_f x)) T) as HS. {
+      eapply ty_sub. intros Hp. subst. eexists; eauto.
+      eapply Hty.
+      eassumption.
+    }
+    specialize (IHHsub2 Hwf HS S2 U2 Hmem).
+    destruct IHHsub2 as [S3 [U3 [Hmem3 [Hsub31 Hsub32]]]].
+    specialize (IHHsub1 Hwf Hty S3 U3 Hmem3).
+    destruct IHHsub1 as [S1 [U1 [Hmem1 [Hsub11 Hsub12]]]].
+    exists S1 U1. split. apply Hmem1. split; eauto.
+  - (* and11 *)
+    exists S2 U2. split.
+    inversion Hmem; subst. apply has_any. assumption. eapply has_and1. assumption.
+    split; eauto.
+  - (* and12 *)
+    exists S2 U2. split.
+    inversion Hmem; subst. apply has_any. assumption. eapply has_and2. assumption.
+    split; eauto.
+  - (* and2 *)
+    apply has_member_inv in Hmem.
+    repeat destruct Hmem as [Hmem|Hmem].
+    + inversion Hmem.
+    + destruct Hmem as [T1 [T2 [Heq [Hmem | Hmem]]]]; inversions Heq.
+      * specialize (IHHsub1 Hwf Hty S2 U2 Hmem). apply IHHsub1.
+      * specialize (IHHsub2 Hwf Hty S2 U2 Hmem). apply IHHsub2.
+    + destruct Hmem as [T1' [Heq _]]. inversion Heq.
+    + destruct Hmem as [y [B [T' [Heq _]]]]. inversion Heq.
+    + inversion Hmem.
+  - (* fld *)
+    inversion Hmem; subst. inversion H0; subst.
+  - (* typ *)
+    apply has_member_inv in Hmem.
+    repeat destruct Hmem as [Hmem|Hmem].
+    + inversions Hmem.
+      exists S1 T1. split.
+      apply has_any. assumption. apply has_refl.
+      split; assumption.
+    + destruct Hmem as [T1' [T2' [Heq _]]]. inversion Heq.
+    + destruct Hmem as [T1' [Heq _]]. inversion Heq.
+    + destruct Hmem as [y [B [T' [Heq _]]]]. inversion Heq.
+    + inversion Hmem.
+  - (* sel2 *)
+    apply has_member_inv in Hmem.
+    repeat destruct Hmem as [Hmem|Hmem].
+    + inversion Hmem.
+    + destruct Hmem as [T1' [T2' [Heq _]]]. inversion Heq.
+    + destruct Hmem as [T1' [Heq _]]. inversion Heq.
+    + destruct Hmem as [y [B [T' [Heq [Htyb Hmem]]]]]. inversions Heq.
+      assert (T' = T) as HeqT. {
+        eapply unique_tight_bounds; eassumption.
+      }
+      subst. eauto.
+    + inversion Hmem.
+  - (* sel1 *)
+    exists S2 U2. split.
+    eapply has_any. assumption. eapply has_sel. eassumption. eassumption.
+    eauto.
+  - (* all *)
+    inversion Hmem; subst. inversion H2; subst.
+Qed.
+
+Lemma has_member_monotonicity: forall G s x T0 ds T A S U,
+  wf_sto G s ->
+  binds x (val_new T0 ds) s ->
+  has_member G x T A S U ->
+  exists T1, has_member G x (typ_bnd T0) A T1 T1 /\
+             subtyp ty_general sub_tight G S T1 /\
+             subtyp ty_general sub_tight G T1 U.
+Proof.
+  introv Hwf Bis Hmem. inversion Hmem; subst.
+  generalize dependent U. generalize dependent S.
+  dependent induction H; intros.
+  - (* var *)
+    destruct (corresponding_types Hwf H).
+    destruct H1 as [S0 [U0 [t [Bis' _]]]]. unfold binds in Bis'. unfold binds in Bis. rewrite Bis' in Bis. inversion Bis.
+    destruct H1 as [S0 [ds0 [Bis' [Hty Heq]]]]. unfold binds in Bis'. unfold binds in Bis. rewrite Bis in Bis'. inversions Bis'.
+    assert (S = U). {
+      eapply has_member_tightness. eassumption. eassumption.
+      eapply has_any.
+      eapply ty_var. eassumption.
+      eassumption.
+    }
+    subst.
+    exists U. eauto.
+  - (* rec_intro *)
+    apply has_member_inv in Hmem.
+    repeat destruct Hmem as [Hmem|Hmem].
+    + inversion Hmem.
+    + destruct Hmem as [T1' [T2' [Heq _]]]. inversion Heq.
+    + destruct Hmem as [T1' [Heq _]]. inversions Heq.
+      apply IHty_trm; eauto.
+      inversions H0. assumption.
+      inversions H0. inversions H4. assumption.
+    + destruct Hmem as [y [B [T' [Heq [Htyb Hmem]]]]]. inversion Heq.
+    + inversion Hmem.
+  - (* rec_elim *)
+    apply IHty_trm; eauto.
+    apply has_any. assumption. apply has_bnd. assumption.
+    apply has_bnd. assumption.
+  - (* and_intro *)
+    apply has_member_inv in Hmem.
+    repeat destruct Hmem as [Hmem|Hmem].
+    + inversion Hmem.
+    + destruct Hmem as [T1' [T2' [Heq [Hmem | Hmem]]]];
+      inversions Heq; inversions H1; inversions H9.
+      apply IHty_trm1; eauto.
+      apply IHty_trm2; eauto. apply has_any; assumption.
+      apply IHty_trm1; eauto. apply has_any; assumption.
+      apply IHty_trm2; eauto.
+    + destruct Hmem as [T1' [Heq _]]. inversion Heq.
+    + destruct Hmem as [y [B [T' [Heq [Htyb Hmem]]]]]. inversion Heq.
+    + inversion Hmem.
+  - (* sub *)
+    destruct (has_member_covariance Hwf H1 H0 Hmem) as [S' [U' [Hmem' [Hsub1' Hsub2']]]].
+    inversion Hmem'; subst.
+    specialize (IHty_trm Hwf Bis S' U' Hmem' H4).
+    destruct IHty_trm as [T1 [Hmem1 [Hsub1 Hsub2]]].
+    exists T1. eauto.
+Qed.
+
+(* ###################################################################### *)
+(** * Tight bound completeness *)
+
+Lemma has_member_rcd_typ_sub2_mut:
+  (forall G x T A S U,
+    has_member G x T A S U ->
+    record_type T ->
+    T = (typ_rcd (dec_typ A S U)) \/ subtyp ty_precise sub_general G T (typ_rcd (dec_typ A S U)))  /\
+  (forall G x T A S U,
+    has_member_rules G x T A S U ->
+    record_type T ->
+    T = (typ_rcd (dec_typ A S U)) \/ subtyp ty_precise sub_general G T (typ_rcd (dec_typ A S U))).
+Proof.
+  apply has_mutind; intros.
+  - apply H; eauto.
+  - left. reflexivity.
+  - inversion H0; subst. inversion H1; subst.
+    assert (record_type T1) as Htyp1. { exists ls. assumption. }
+    specialize (H Htyp1). destruct H as [H | H].
+    + subst. right. apply subtyp_and11.
+    + right.
+      eapply subtyp_trans. eapply subtyp_and11. apply H.
+  - inversion H0; subst. inversion H1; subst. inversion h; subst. inversion H3; subst.
+    right. eapply subtyp_and12.
+  - inversion H0. inversion H1.
+  - inversion H0. inversion H1.
+  - destruct H as [ls H]. inversion H.
+Qed.
 
 Lemma wf_sto_val_new_in_G: forall G s x T ds,
   wf_sto G s ->
@@ -2314,300 +2310,78 @@ Proof.
     assumption.
 Qed.
 
-Lemma all_intro_inversion: forall Gs G S t U,
-  ty_trm ty_precise Gs G (trm_val (val_lambda S t)) U ->
+(* If G ~ s, s |- x = new(x: T)d, and G |-# x: {A: S..U} then G |-# x.A <: U and G |-# S <: x.A. *)
+Lemma tight_bound_completeness: forall G s x T ds A S U,
+  wf_sto G s ->
+  binds x (val_new T ds) s ->
+  ty_trm ty_general sub_tight G (trm_var (avar_f x)) (typ_rcd (dec_typ A S U)) ->
+  subtyp ty_general sub_tight G (typ_sel (avar_f x) A) U /\
+  subtyp ty_general sub_tight G S (typ_sel (avar_f x) A).
+Proof.
+  introv Hwf Bis Hty.
+  assert (has_member G x (typ_rcd (dec_typ A S U)) A S U) as Hmem. {
+    apply has_any. assumption. apply has_refl.
+  }
+  apply has_member_monotonicity with (s:=s) (ds:=ds) (T0:=T) in Hmem.
+  destruct Hmem as [T1 [Hmem [Hsub1 Hsub2]]].
+  assert (has_member G x (open_typ x T) A T1 T1) as Hmemx. {
+    apply has_member_inv in Hmem.
+    repeat destruct Hmem as [Hmem|Hmem].
+    + inversion Hmem.
+    + destruct Hmem as [T1' [T2' [Heq _]]]. inversion Heq.
+    + destruct Hmem as [T1' [Heq Hmem]]. inversions Heq. assumption.
+    + destruct Hmem as [y [B [T' [Heq [Htyb Hmem]]]]]. inversion Heq.
+    + inversion Hmem.
+  }
+  assert (record_type T) as Htype. {
+    eapply record_new_typing. eapply val_new_typing; eauto.
+  }
+  assert (record_type (open_typ x T)) as Htypex. {
+    apply open_record_type. assumption.
+  }
+  assert (open_typ x T = (typ_rcd (dec_typ A T1 T1)) \/ subtyp ty_precise sub_general G (open_typ x T) (typ_rcd (dec_typ A T1 T1))) as Hsub. {
+    destruct has_member_rcd_typ_sub2_mut as [HE _].
+    eapply HE; eauto.
+  }
+  assert (ty_trm ty_precise sub_general G (trm_var (avar_f x)) (open_typ x T)) as Htypx. {
+    eapply ty_rec_elim.
+    eapply ty_var.
+    eapply wf_sto_val_new_in_G; eauto.
+  }
+  assert (ty_trm ty_precise sub_general G (trm_var (avar_f x)) (typ_rcd (dec_typ A T1 T1))) as Htyp. {
+    destruct Hsub as [Heq | Hsub].
+    - rewrite Heq in Htypx. apply Htypx.
+    - eapply ty_sub.
+      intro. eexists. reflexivity.
+      eapply Htypx. eapply Hsub.
+  }
+  split.
+  eapply subtyp_trans. eapply subtyp_sel1_tight. eapply Htyp. eapply Hsub2.
+  eapply subtyp_trans. eapply Hsub1. eapply subtyp_sel2_tight. eapply Htyp.
+  eapply Hwf. eapply Bis.
+Qed.
+
+(* ###################################################################### *)
+(** * Misc Inversions *)
+
+Lemma all_intro_inversion: forall G S t U,
+  ty_trm ty_precise sub_general G (trm_val (val_lambda S t)) U ->
   exists T, U = typ_all S T.
 Proof.
   intros. dependent induction H.
   - eexists. reflexivity.
-  - assert (ty_precise <> ty_general) as Neqm by discriminate.
-    specialize (H Neqm). destruct H. inversion H.
+  - assert (ty_precise = ty_precise) as Heqm1 by reflexivity.
+    specialize (H Heqm1). destruct H. inversion H.
 Qed.
 
-Lemma new_intro_inversion: forall Gs G T ds U,
-  ty_trm ty_precise Gs G (trm_val (val_new T ds)) U ->
+Lemma new_intro_inversion: forall G T ds U,
+  ty_trm ty_precise sub_general G (trm_val (val_new T ds)) U ->
   U = typ_bnd T /\ record_type T.
 Proof.
   intros. inversion H; subst.
   - apply record_new_typing in H. split; eauto.
-  - assert (ty_precise <> ty_general) as Neqm by discriminate.
-    specialize (H0 Neqm). destruct H0. inversion H0.
-Qed.
-
-(* ###################################################################### *)
-(** ** The substitution principle *)
-
-Lemma subst_rules: forall y S,
-   (forall m Gs G t T, ty_trm m Gs G t T -> forall s G2 x,
-    wf_sto Gs s ->
-    G = x ~ S & G2 ->
-    ok (x ~ S & G2) ->
-    x \notin fv_ctx_types Gs -> x # Gs ->
-    ty_trm ty_general Gs empty (trm_var (avar_s y)) (subst_typ x (in_sto y) S) ->
-    m = ty_general ->
-    ty_trm m Gs (subst_ctx x (in_sto y) G2) (subst_trm x (in_sto y) t) (subst_typ x (in_sto y) T)) /\
-  (forall Gs G d D, ty_def Gs G d D -> forall s G2 x,
-    wf_sto Gs s ->
-    G = x ~ S & G2 ->
-    ok (x ~ S & G2) ->
-    x \notin fv_ctx_types Gs -> x # Gs ->
-    ty_trm ty_general Gs empty (trm_var (avar_s y)) (subst_typ x (in_sto y) S) ->
-    ty_def Gs (subst_ctx x (in_sto y) G2) (subst_def x (in_sto y) d) (subst_dec x (in_sto y) D)) /\
-  (forall Gs G ds T, ty_defs Gs G ds T -> forall s G2 x,
-    wf_sto Gs s ->
-    G = x ~ S & G2 ->
-    ok (x ~ S & G2) ->
-    x \notin fv_ctx_types Gs -> x # Gs ->
-    ty_trm ty_general Gs empty (trm_var (avar_s y)) (subst_typ x (in_sto y) S) ->
-    ty_defs Gs (subst_ctx x (in_sto y) G2) (subst_defs x (in_sto y) ds) (subst_typ x (in_sto y) T)) /\
-  (forall m Gs G T U, subtyp m Gs G T U -> forall s G2 x,
-    wf_sto Gs s ->
-    G = x ~ S & G2 ->
-    ok (x ~ S & G2) ->
-    x \notin fv_ctx_types Gs -> x # Gs ->
-    ty_trm ty_general Gs empty (trm_var (avar_s y)) (subst_typ x (in_sto y) S) ->
-    m = ty_general ->
-    subtyp m Gs (subst_ctx x (in_sto y) G2) (subst_typ x (in_sto y) T) (subst_typ x (in_sto y) U)).
-Proof.
-  intros y S. apply rules_mutind; intros; subst G; try subst m; try solve [false].
-  - (* ty_var_s *)
-    simpl.
-    assert (subst_typ x0 (in_sto y) T = T) as A. {
-      apply subst_fresh_typ.
-      eapply fv_ctx_types_binds with (G:=Gs); eauto.
-    }
-    rewrite A.
-    apply ty_var_s with (T:=T); eauto.
-  - (* ty_var_c *)
-    simpl. case_if.
-    + assert (T = S) as A. {
-        rewrite <- concat_empty_l in b. rewrite concat_assoc in b.
-        apply binds_middle_eq_inv in b. subst. reflexivity.
-        rewrite concat_empty_l. assumption.
-      }
-      subst.
-      assert ((subst_ctx x0 (in_sto y) G2)=empty & (subst_ctx x0 (in_sto y) G2)) as B. {
-        rewrite concat_empty_l. reflexivity.
-      }
-      rewrite B. apply weaken_ty_trm; eauto. rewrite concat_empty_l.
-      apply ok_map. eauto.
-    + rewrite <- concat_empty_l in b. rewrite concat_assoc in b.
-      apply binds_subst in b. rewrite concat_empty_l in b.
-      apply ty_var_c.
-      apply binds_map. assumption. assumption.
-  - (* ty_all_intro *)
-    simpl.
-    apply_fresh ty_all_intro as z; eauto.
-    assert (z \notin L) as FrL by eauto.
-    assert (subst_fvar x (in_sto y) (in_ctx z) = (in_ctx z)) as A. {
-      unfold subst_fvar. rewrite If_r. reflexivity. eauto.
-    }
-    rewrite <- A.
-    rewrite <- subst_open_commute_trm. rewrite <- subst_open_commute_typ.
-    assert (subst_ctx x (in_sto y) G2 & z ~ subst_typ x (in_sto y) T = subst_ctx x (in_sto y) (G2 & z ~ T)) as B. {
-      unfold subst_ctx. rewrite map_concat. rewrite map_single. reflexivity.
-    }
-    rewrite B.
-    eapply H; eauto.
-    rewrite concat_assoc. reflexivity.
-    rewrite concat_assoc. apply ok_push. assumption. eauto.
-  - (* ty_all_elim *)
-    simpl. rewrite subst_open_commute_typ.
-    eapply ty_all_elim.
-    eapply H; eauto.
-    eapply H0; eauto.
-  - (* ty_new_intro *)
-    simpl.
-    apply_fresh ty_new_intro as z; eauto.
-    assert (z \notin L) as FrL by eauto.
-    assert (subst_fvar x (in_sto y) (in_ctx z) = (in_ctx z)) as A. {
-      unfold subst_fvar. rewrite If_r. reflexivity. eauto.
-    }
-    rewrite <- A.
-    rewrite <- subst_open_commute_typ. rewrite <- subst_open_commute_defs.
-    assert (subst_ctx x (in_sto y) G2 & z ~ subst_typ x (in_sto y) (open_typ (in_ctx z) T) = subst_ctx x (in_sto y) (G2 & z ~ open_typ (in_ctx z) T)) as B. {
-      unfold subst_ctx. rewrite map_concat. rewrite map_single. reflexivity.
-    }
-    rewrite B.
-    eapply H; eauto.
-    rewrite concat_assoc. reflexivity.
-    rewrite concat_assoc. apply ok_push. assumption. eauto.
-  - (* ty_new_elim *)
-    simpl. apply ty_new_elim.
-    eapply H; eauto.
-  - (* ty_let *)
-    simpl.
-    apply_fresh ty_let as z; eauto.
-    assert (subst_ctx x (in_sto y) G2 & z ~ subst_typ x (in_sto y) T = subst_ctx x (in_sto y) (G2 & z ~ T)) as B. {
-      unfold subst_ctx. rewrite map_concat. rewrite map_single. reflexivity.
-    }
-    rewrite B.
-    assert (subst_fvar x (in_sto y) (in_ctx z) = (in_ctx z)) as A. {
-      unfold subst_fvar. rewrite If_r. reflexivity. eauto.
-    }
-    rewrite <- A. rewrite <- subst_open_commute_trm.
-    eapply H0 with (x0:=z); eauto.
-    rewrite concat_assoc. reflexivity.
-    rewrite concat_assoc. apply ok_push. assumption. eauto.
-  - (* ty_rec_intro *)
-    simpl. apply ty_rec_intro.
-    rewrite <- subst_open_commute_typ.
-    eapply H; eauto.
-  - (* ty_rec_elim *)
-    simpl. rewrite subst_open_commute_typ.
-    apply ty_rec_elim.
-    eapply H; eauto.
-  - (* ty_and_intro *)
-    simpl.
-    apply ty_and_intro; eauto.
-  - (* ty_sub *)
-    eapply ty_sub; eauto 4.
-    intro Contra. false.
-  - (* ty_def_typ *)
-    simpl. apply ty_def_typ; eauto.
-  - (* ty_def_trm *)
-    simpl. apply ty_def_trm; eauto.
-  - (* ty_defs_one *)
-    simpl. apply ty_defs_one; eauto.
-  - (* ty_defs_cons *)
-    simpl. apply ty_defs_cons; eauto.
-    rewrite <- subst_label_of_def.
-    apply subst_defs_hasnt. assumption.
-  - (* subtyp_top *)
-    apply subtyp_top. discriminate.
-  - (* subtyp_bot *)
-    apply subtyp_bot. discriminate.
-  - (* subtyp_refl *)
-    apply subtyp_refl. discriminate.
-  - (* subtyp_trans *)
-    eapply subtyp_trans; eauto 4.
-    eapply subtyp_refl. discriminate.
-  - (* subtyp_and11 *)
-    eapply subtyp_and11; eauto.
-  - (* subtyp_and12 *)
-    eapply subtyp_and12; eauto.
-  - (* subtyp_and2 *)
-    eapply subtyp_and2; eauto 4.
-  - (* subtyp_fld *)
-    eapply subtyp_fld; eauto.
-  - (* subtyp_typ *)
-    eapply subtyp_typ; eauto 4.
-  - (* subtyp_sel2_c *)
-    simpl.
-    case_if.
-    + assert (G' = x0 ~ S) as B. {
-        eapply restricted_by_first; eauto.
-      }
-      subst.
-      assert (ty_trm ty_general Gs (subst_ctx x0 (in_sto y) empty)
-        (subst_trm x0 (in_sto y) (trm_var (avar_c x0)))
-        (subst_typ x0 (in_sto y) (typ_rcd (dec_typ A S0 T)))) as Hg. {
-        eapply H; eauto.
-        rewrite concat_empty_r. reflexivity.
-        rewrite concat_empty_r. eauto.
-      }
-      simpl in Hg. rewrite If_l in Hg.
-      unfold subst_ctx in Hg. rewrite map_empty in Hg.
-      assert (avar_f (in_sto y) = (avar_s y)) as C by eauto.
-      rewrite C in Hg.
-      eapply subtyp_sel2_s.
-      discriminate. left. split; reflexivity.
-      assert (subst_ctx x0 (in_sto y) G2 = empty & subst_ctx x0 (in_sto y) G2) as D. {
-        rewrite concat_empty_l. reflexivity.
-      }
-      rewrite D. eapply weaken_ty_trm. eapply Hg.
-      rewrite concat_empty_l. unfold subst_ctx. eauto.
-      reflexivity.
-    + assert (exists GA2 GB2, G2 = GA2 & GB2 /\ G' = x0 ~ S & GA2) as B. {
-        admit.
-      }
-      destruct B as [GA2 [GB2 [Heq2 Heq']]]. subst.
-      eapply subtyp_sel2_c.
-      discriminate.
-      instantiate (1:=(subst_ctx x0 (in_sto y) GA2)). admit.
-      specialize (H s GA2 x0). simpl in H. rewrite If_r in H.
-      eapply H; eauto.
-      rewrite concat_assoc in H2. eauto.
-      assumption.
-  - (* subtyp_sel1 *)
-    admit.
-  - (* subtyp_sel2_tight *)
-    destruct o as [[? ?] | [Contra ?]]. subst.
-    simpl. eapply subtyp_sel2_s; eauto.
-    simpl in H. eapply H; eauto 4.
-    false.
-(*
-    lets B: (precise_fresh_ty_trm t H3 H4); eauto.
-    simpl in B. apply notin_union_r in B. destruct B as [B ?].
-    assert (subst_typ x0 (in_sto y) T = T) as C. {
-      apply subst_fresh_typ.
-      assumption.
-    }
-    rewrite C. assumption.
-*)
-  - (* subtyp_sel1_tight *)
-    destruct o as [[? ?] | [Contra ?]]. subst.
-    simpl. eapply subtyp_sel1_s; eauto.
-    simpl in H. eapply H; eauto 4.
-    false.
-  - (* subtyp_all *)
-    simpl. apply_fresh subtyp_all as z; eauto.
-    assert (z \notin L) as FrL by eauto.
-    assert (subst_fvar x (in_sto y) (in_ctx z) = (in_ctx z)) as A. {
-      unfold subst_fvar. rewrite If_r. reflexivity. eauto.
-    }
-    rewrite <- A.
-    rewrite <- subst_open_commute_typ. rewrite <- subst_open_commute_typ.
-    assert (subst_ctx x (in_sto y) G2 & z ~ subst_typ x (in_sto y) S2 = subst_ctx x (in_sto y) (G2 & z ~ S2)) as B. {
-      unfold subst_ctx. rewrite map_concat. rewrite map_single. reflexivity.
-    }
-    rewrite B.
-    eapply H0; eauto.
-    rewrite concat_assoc. reflexivity.
-    rewrite concat_assoc. apply ok_push. assumption. eauto.
-  - (* subtyp_bnd *)
-    simpl. apply_fresh subtyp_bnd as z; eauto 4.
-    assert (z \notin L) as FrL by eauto.
-    assert (subst_fvar x (in_sto y) (in_ctx z) = (in_ctx z)) as A. {
-      unfold subst_fvar. rewrite If_r. reflexivity. eauto.
-    }
-    rewrite <- A.
-    rewrite <- subst_open_commute_typ. rewrite <- subst_open_commute_typ.
-    assert (subst_ctx x (in_sto y) G2 & z ~ typ_bnd (subst_typ x (in_sto y) T1) = subst_ctx x (in_sto y) (G2 & z ~ (typ_bnd T1))) as B. {
-      unfold subst_ctx. rewrite map_concat. rewrite map_single.
-      simpl. reflexivity.
-    }
-    rewrite B.
-    eapply H; eauto using concat_assoc.
-    rewrite concat_assoc. apply ok_push; eauto.
-Qed.
-
-Lemma subst_ty_trm: forall y S s Gs x t T,
-    wf_sto Gs s ->
-    ty_trm ty_general Gs (x ~ S) t T -> 
-    x \notin fv_ctx_types Gs -> x # Gs ->
-    ty_trm ty_general Gs empty (trm_var (avar_s y)) (subst_typ x (in_sto y) S) ->
-    ty_trm ty_general Gs empty (subst_trm x (in_sto y) t) (subst_typ x (in_sto y) T).
-Proof.
-  intros.
-  apply (proj51 (subst_rules y S)) with (s:=s) (G2:=empty) (x:=x) in H0; eauto 4.
-  unfold subst_ctx in H0. rewrite map_empty in H0. assumption.
-  rewrite concat_empty_r. reflexivity.
-  rewrite concat_empty_r. rewrite <- concat_empty_l. eapply ok_push; eauto.
-Qed.
-
-Lemma subst_ty_defs: forall y S s Gs x ds T,
-    wf_sto Gs s ->
-    ty_defs Gs (x ~ S) ds T ->
-    x \notin fv_ctx_types Gs -> x # Gs ->
-    ty_trm ty_general Gs empty (trm_var (avar_s y)) (subst_typ x (in_sto y) S) ->
-    ty_defs Gs empty (subst_defs x (in_sto y) ds) (subst_typ x (in_sto y) T).
-Proof.
-  intros.
-  apply (proj53 (subst_rules y S)) with (s:=s) (G2:=empty) (x:=x) in H0; eauto 4.
-  unfold subst_ctx in H0. rewrite map_empty in H0. assumption.
-  rewrite concat_empty_r. reflexivity.
-  rewrite concat_empty_r. rewrite <- concat_empty_l. eapply ok_push; eauto.
+  - assert (ty_precise = ty_precise) as Heqm1 by reflexivity.
+    specialize (H0 Heqm1). destruct H0. inversion H0.
 Qed.
 
 (* ###################################################################### *)
@@ -2627,55 +2401,55 @@ If S in SS and G |-! y: {A: S..S} then y.A in SS.
 If S in SS then rec(x: S) in SS.
 *)
 
-Inductive possible_types: nat -> ctx -> var -> val -> typ -> Prop :=
-| pt_top : forall n G x v,
-  possible_types n G x v typ_top
-| pt_new : forall n G x T ds,
-  possible_types n G x (val_new T ds) (open_typ (in_sto x) T)
-| pt_rcd_trm : forall n G x T ds a t T',
-  defs_has (open_defs (in_sto x) ds) (def_trm a t) ->
-  ty_trm ty_general G empty t T' ->
-  possible_types n G x (val_new T ds) (typ_rcd (dec_trm a T'))
-| pt_rcd_typ : forall n G x T ds A T' S U,
-  defs_has (open_defs (in_sto x) ds) (def_typ A T') ->
-  subtyp ty_general G empty S T' ->
-  subtyp ty_general G empty T' U ->
-  possible_types n G x (val_new T ds) (typ_rcd (dec_typ A S U))
-| pt_lambda : forall L n G x S t T S' T',
+Inductive possible_types: ctx -> var -> val -> typ -> Prop :=
+| pt_top : forall G x v,
+  possible_types G x v typ_top
+| pt_new : forall G x T ds,
+  possible_types G x (val_new T ds) (open_typ x T)
+| pt_rcd_trm : forall G x T ds a t T',
+  defs_has (open_defs x ds) (def_trm a t) ->
+  ty_trm ty_general sub_general G t T' ->
+  possible_types G x (val_new T ds) (typ_rcd (dec_trm a T'))
+| pt_rcd_typ : forall G x T ds A T' S U,
+  defs_has (open_defs x ds) (def_typ A T') ->
+  subtyp ty_general sub_general G S T' ->
+  subtyp ty_general sub_general G T' U ->
+  possible_types G x (val_new T ds) (typ_rcd (dec_typ A S U))
+| pt_lambda : forall L G x S t T S' T',
   (forall y, y \notin L ->
-   ty_trm ty_general G (y ~ S) (open_trm (in_ctx y) t) (open_typ (in_ctx y) T)) ->
-  subtyp ty_general G empty S' S ->
+   ty_trm ty_general sub_general (G & y ~ S) (open_trm y t) (open_typ y T)) ->
+  subtyp ty_general sub_general G S' S ->
   (forall y, y \notin L ->
-   subtyp ty_general G (y ~ S') (open_typ (in_ctx y) T) (open_typ (in_ctx y) T')) ->
-  possible_types n G x (val_lambda S t) (typ_all S' T')
-| pt_and : forall n n1 n2 G x v S1 S2,
-  possible_types n1 G x v S1 ->
-  possible_types n2 G x v S2 ->
-  possible_types (n+(max n1 n2)) G x v (typ_and S1 S2)
-| pt_sel : forall n n1 G x v y A S,
-  possible_types n1 G x v S ->
-  ty_trm ty_precise G empty (trm_var y) (typ_rcd (dec_typ A S S)) ->
-  possible_types (n+n1) G x v (typ_sel y A)
-| pt_bnd : forall n n1 G x v S S',
-  possible_types n1 G x v S ->
-  S = open_typ (in_sto x) S' ->
-  possible_types (n+n1+1) G x v (typ_bnd S')
+   subtyp ty_general sub_general (G & y ~ S') (open_typ y T) (open_typ y T')) ->
+  possible_types G x (val_lambda S t) (typ_all S' T')
+| pt_and : forall G x v S1 S2,
+  possible_types G x v S1 ->
+  possible_types G x v S2 ->
+  possible_types G x v (typ_and S1 S2)
+| pt_sel : forall G x v y A S,
+  possible_types G x v S ->
+  ty_trm ty_precise sub_general G (trm_var y) (typ_rcd (dec_typ A S S)) ->
+  possible_types G x v (typ_sel y A)
+| pt_bnd : forall G x v S S',
+  possible_types G x v S ->
+  S = open_typ x S' ->
+  possible_types G x v (typ_bnd S')
 .
 
-Lemma var_new_typing: forall Gs G s x T ds,
-  wf_sto Gs s ->
+Lemma var_new_typing: forall G s x T ds,
+  wf_sto G s ->
   binds x (val_new T ds) s ->
-  ty_trm ty_general Gs G (trm_var (avar_s x)) (open_typ (in_sto x) T).
+  ty_trm ty_general sub_general G (trm_var (avar_f x)) (open_typ x T).
 Proof.
   intros.
-  apply ty_rec_elim. apply ty_var_s. eapply wf_sto_val_new_in_G; eauto.
+  apply ty_rec_elim. apply ty_var. eapply wf_sto_val_new_in_G; eauto.
 Qed.
 
-Lemma ty_defs_has: forall Gs G ds T d,
-  ty_defs Gs G ds T ->
+Lemma ty_defs_has: forall G ds T d,
+  ty_defs G ds T ->
   defs_has ds d ->
   record_type T ->
-  exists D, ty_def Gs G d D /\ record_sub T (typ_rcd D).
+  exists D, ty_def G d D /\ record_sub T (typ_rcd D).
 Proof.
   introv Hdefs Hhas Htype. generalize dependent d. generalize dependent ds.
   inversion Htype; subst. induction H; intros.
@@ -2687,7 +2461,7 @@ Proof.
     + inversions Hhas.
       exists D. split. inversions Hdefs; subst. assumption.
       eapply rs_dropl. eapply rs_refl.
-    + assert (exists D0, ty_def Gs G d D0 /\ record_sub T (typ_rcd D0)) as A. {
+    + assert (exists D0, ty_def G d D0 /\ record_sub T (typ_rcd D0)) as A. {
         eapply IHrecord_typ; eauto.
         exists ls. eassumption.
       }
@@ -2695,35 +2469,34 @@ Proof.
       exists D0. split. apply A1. apply rs_drop. apply A2.
 Qed.
 
-Lemma new_ty_defs: forall Gs s x T ds,
-  wf_sto Gs s ->
+Lemma new_ty_defs: forall G s x T ds,
+  wf_sto G s ->
   binds x (val_new T ds) s ->
-  ty_defs Gs empty (open_defs (in_sto x) ds) (open_typ (in_sto x) T).
+  ty_defs G (open_defs x ds) (open_typ x T).
 Proof.
   introv Hwf Bis.
   lets Htyv: (val_new_typing Hwf Bis).
   inversion Htyv; subst.
   pick_fresh y. assert (y \notin L) as FrL by auto. specialize (H3 y FrL).
   rewrite subst_intro_defs with (x:=y). rewrite subst_intro_typ with (x:=y).
-  rewrite concat_empty_l in H3.
-  eapply subst_ty_defs; eauto.
+  eapply subst_ty_defs. eapply H3.
+  apply ok_push. eapply wf_sto_to_ok_G. eassumption. eauto. eauto.
   rewrite <- subst_intro_typ with (x:=y).
-  eapply ty_rec_elim. apply ty_var_s. eapply wf_sto_val_new_in_G; eauto.
+  eapply ty_rec_elim. apply ty_var. eapply wf_sto_val_new_in_G; eauto.
   eauto. eauto. eauto.
-  assert (ty_precise <> ty_general) as Neqm by discriminate.
-  specialize (H Neqm). destruct H as [? Contra]. inversion Contra.
+  assert (ty_precise = ty_precise) as Heqm1 by reflexivity.
+  specialize (H Heqm1). destruct H as [? Contra]. inversion Contra.
 Qed.
 
-Lemma pt_piece_rcd: forall n Gs s x T ds d D,
-  wf_sto Gs s ->
+Lemma pt_piece_rcd: forall G s x T ds d D,
+  wf_sto G s ->
   binds x (val_new T ds) s ->
-  defs_has (open_defs (in_sto x) ds) d ->
-  ty_def Gs empty d D ->
-  possible_types n Gs x (val_new T ds) (typ_rcd D).
+  defs_has (open_defs x ds) d ->
+  ty_def G d D ->
+  possible_types G x (val_new T ds) (typ_rcd D).
 Proof.
   introv Hwf Bis Hhas Hdef.
-  inversion Hdef; subst; econstructor; eauto;
-  eapply subtyp_refl; discriminate.
+  inversion Hdef; subst; econstructor; eauto.
 Qed.
 
 Inductive record_has: typ -> dec -> Prop :=
@@ -2750,10 +2523,10 @@ Proof.
     + apply IHds; eauto.
 Qed.
 
-Lemma record_has_ty_defs: forall Gs G T ds D,
-  ty_defs Gs G ds T ->
+Lemma record_has_ty_defs: forall G T ds D,
+  ty_defs G ds T ->
   record_has T D ->
-  exists d, defs_has ds d /\ ty_def Gs G d D.
+  exists d, defs_has ds d /\ ty_def G d D.
 Proof.
   introv Hdefs Hhas. induction Hdefs.
   - inversion Hhas; subst. exists d. split.
@@ -2770,11 +2543,11 @@ Proof.
       assumption.
 Qed.
 
-Lemma pt_rcd_has_piece: forall n Gs s x T ds D,
-  wf_sto Gs s ->
+Lemma pt_rcd_has_piece: forall G s x T ds D,
+  wf_sto G s ->
   binds x (val_new T ds) s ->
-  record_has (open_typ (in_sto x) T) D ->
-  possible_types n Gs x (val_new T ds) (typ_rcd D).
+  record_has (open_typ x T) D ->
+  possible_types G x (val_new T ds) (typ_rcd D).
 Proof.
   introv Hwf Bis Hhas.
   lets Hdefs: (new_ty_defs Hwf Bis).
@@ -2782,33 +2555,33 @@ Proof.
   eapply pt_piece_rcd; eauto.
 Qed.
 
-Lemma pt_rcd_trm_inversion: forall n Gs s x v a T,
-  wf_sto Gs s ->
+Lemma pt_rcd_trm_inversion: forall G s x v a T,
+  wf_sto G s ->
   binds x v s ->
-  possible_types n Gs x v (typ_rcd (dec_trm a T)) ->
+  possible_types G x v (typ_rcd (dec_trm a T)) ->
   exists S ds t,
     v = val_new S ds /\
-    defs_has (open_defs (in_sto x) ds) (def_trm a t) /\
-    ty_trm ty_general Gs empty t T.
+    defs_has (open_defs x ds) (def_trm a t) /\
+    ty_trm ty_general sub_general G t T.
 Proof.
   introv Hwf Bis Hp. inversion Hp; subst.
-  - induction T0; simpl in H4; try solve [inversion H4].
-    induction d; simpl in H4; try solve [inversion H4].
-    unfold open_typ in H4. simpl in H4. inversions H4.
+  - induction T0; simpl in H3; try solve [inversion H3].
+    induction d; simpl in H3; try solve [inversion H3].
+    unfold open_typ in H3. simpl in H3. inversions H3.
     lets Hty: (val_new_typing Hwf Bis). inversion Hty; subst.
     pick_fresh y. assert (y \notin L) as FrL by auto. specialize (H3 y FrL).
     unfold open_typ in H3. simpl in H3. inversion H3; subst.
     destruct ds; simpl in H; try solve [inversion H].
     destruct ds; simpl in H; try solve [inversion H].
     unfold open_defs in H. simpl in H. inversions H.
-    destruct d0; simpl in H4; inversion H4; subst.
-    assert (ty_trm ty_general Gs empty (open_trm (in_sto x) t1) (open_typ (in_sto x) t0)) as A. {
+    destruct d0; simpl in H2; inversion H2; subst.
+    inversion H2; subst.
+    assert (ty_trm ty_general sub_general G (open_trm x t1) (open_typ x t0)) as A. {
       rewrite subst_intro_typ with (x:=y). rewrite subst_intro_trm with (x:=y).
-      rewrite concat_empty_l in H2.
-      eapply subst_ty_trm; eauto.
+      eapply subst_ty_trm. eapply H4.
+      apply ok_push. eapply wf_sto_to_ok_G. eassumption. eauto. eauto. eauto.
       simpl. rewrite <- subst_intro_typ with (x:=y).
-      lets Htyv: (var_new_typing (@empty typ) Hwf Bis).
-      unfold open_typ in Htyv. simpl in Htyv.
+      lets Htyv: (var_new_typing Hwf Bis). unfold open_typ in Htyv. simpl in Htyv.
       unfold open_typ. apply Htyv.
       eauto.
       apply notin_union_r1 in Fr. apply notin_union_r2 in Fr.
@@ -2819,51 +2592,52 @@ Proof.
     unfold open_defs. simpl. unfold defs_has. simpl.
     rewrite If_l. reflexivity. reflexivity.
     eapply A.
-    assert (ty_precise <> ty_general) as Neqm by discriminate.
-    specialize (H Neqm). destruct H. inversion H.
+    assert (ty_precise = ty_precise) as Heqm1 by reflexivity.
+    specialize (H Heqm1). destruct H. inversion H.
   - repeat eexists. eassumption. assumption.
 Qed.
 
-Lemma pt_rcd_typ_inversion: forall n Gs s x v A S U,
-  wf_sto Gs s ->
+Lemma pt_rcd_typ_inversion: forall G s x v A S U,
+  wf_sto G s ->
   binds x v s ->
-  possible_types n Gs x v (typ_rcd (dec_typ A S U)) ->
+  possible_types G x v (typ_rcd (dec_typ A S U)) ->
   exists T ds T',
     v = val_new T ds /\
-    defs_has (open_defs (in_sto x) ds) (def_typ A T') /\
-    subtyp ty_general Gs empty S T' /\
-    subtyp ty_general Gs empty T' U.
+    defs_has (open_defs x ds) (def_typ A T') /\
+    subtyp ty_general sub_general G S T' /\
+    subtyp ty_general sub_general G T' U.
 Proof.
   introv Hwf Bis Hp. inversion Hp; subst.
-  - induction T; simpl in H4; try solve [inversion H4].
-    induction d; simpl in H4; try solve [inversion H4].
-    unfold open_typ in H4. simpl in H4. inversions H4.
+  - induction T; simpl in H3; try solve [inversion H3].
+    induction d; simpl in H3; try solve [inversion H3].
+    unfold open_typ in H3. simpl in H3. inversions H3.
     lets Hty: (val_new_typing Hwf Bis). inversion Hty; subst.
     pick_fresh y. assert (y \notin L) as FrL by auto. specialize (H3 y FrL).
     unfold open_typ in H3. simpl in H3. inversion H3; subst.
     destruct ds; simpl in H; try solve [inversion H].
     destruct ds; simpl in H; try solve [inversion H].
     unfold open_defs in H. simpl in H. inversions H.
-    destruct d0; simpl in H4; inversion H4; subst.
+    destruct d0; simpl in H2; inversion H2; subst.
+    inversion H2; subst.
     assert (t2 = t0). {
-      apply open_eq_typ with (v:=(in_ctx y)) (x:=y) (i:=0); eauto.
+      eapply open_eq_typ; eauto.
       apply notin_union_r1 in Fr. apply notin_union_r1 in Fr.
       apply notin_union_r2 in Fr.
-      unfold fv_defs in Fr. eauto.
+      unfold fv_defs in Fr. eauto. eauto.
     }
     assert (t2 = t1). {
-      apply open_eq_typ with (v:=(in_ctx y)) (x:=y) (i:=0); eauto.
+      eapply open_eq_typ; eauto.
       apply notin_union_r1 in Fr. apply notin_union_r1 in Fr.
       apply notin_union_r2 in Fr.
-      unfold fv_defs in Fr. eauto.
+      unfold fv_defs in Fr. eauto. eauto.
     }
-    subst. subst.
+    subst. subst. clear H5. clear H8.
     repeat eexists.
     unfold open_defs. simpl. unfold defs_has. simpl.
     rewrite If_l. reflexivity. reflexivity.
-    eapply subtyp_refl. discriminate. eapply subtyp_refl. discriminate.
-    assert (ty_precise <> ty_general) as Neqm by discriminate.
-    specialize (H Neqm). destruct H. inversion H.
+    eapply subtyp_refl. eapply subtyp_refl.
+    assert (ty_precise = ty_precise) as Heqm1 by reflexivity.
+    specialize (H Heqm1). destruct H. inversion H.
   - repeat eexists. eassumption. eassumption. eassumption.
 Qed.
 
@@ -2893,38 +2667,32 @@ Proof.
     + apply rh_and. apply IHHsub. assumption.
 Qed.
 
-Lemma pt_record_sub_has: forall n G x v T1 T2,
-  (forall D, record_has T1 D -> possible_types n G x v (typ_rcd D)) ->
+Lemma pt_record_sub_has: forall G x v T1 T2,
+  (forall D, record_has T1 D -> possible_types G x v (typ_rcd D)) ->
   record_sub T1 T2 ->
-  (forall D, record_has T2 D -> possible_types n G x v (typ_rcd D)).
+  (forall D, record_has T2 D -> possible_types G x v (typ_rcd D)).
 Proof.
   introv HP Hsub. intros D Hhas. apply HP; eauto using record_sub_has.
 Qed.
 
-Lemma max_and: forall n, 0+(max n n)=n.
-Proof.
-  intros. rewrite Max.max_idempotent. omega.
-Qed.
-
-Lemma pt_has_record: forall n G x v T,
-  (forall D, record_has T D -> possible_types n G x v (typ_rcd D)) ->
+Lemma pt_has_record: forall G x v T,
+  (forall D, record_has T D -> possible_types G x v (typ_rcd D)) ->
   record_type T ->
-  possible_types n G x v T.
+  possible_types G x v T.
 Proof.
   introv HP Htype. destruct Htype as [ls Htyp]. induction Htyp.
   - apply HP; eauto. apply rh_one.
-  - rewrite <- (max_and n).
-    apply pt_and.
+  - apply pt_and.
     + apply IHHtyp; eauto.
       intros D0 HH0. apply HP; eauto. apply rh_and; eauto.
     + apply HP; eauto. apply rh_andl.
 Qed.
 
-Lemma pt_has_sub: forall n G x v T U,
-  (forall D, record_has T D -> possible_types n G x v (typ_rcd D)) ->
+Lemma pt_has_sub: forall G x v T U,
+  (forall D, record_has T D -> possible_types G x v (typ_rcd D)) ->
   record_type T ->
   record_sub T U ->
-  possible_types n G x v U.
+  possible_types G x v U.
 Proof.
   introv HP Htype Hsub. induction Hsub.
   - apply pt_has_record; eauto.
@@ -2933,8 +2701,7 @@ Proof.
     apply rs_drop. apply rs_refl.
     eapply record_type_sub_closed; eauto.
     apply rs_drop. apply rs_refl.
-  - rewrite <- (max_and n).
-    apply pt_and.
+  - apply pt_and.
     + apply IHHsub; eauto. eapply pt_record_sub_has; eauto.
       apply rs_drop. apply rs_refl.
       eapply record_type_sub_closed; eauto.
@@ -2942,73 +2709,34 @@ Proof.
     + apply HP; eauto. apply rh_andl.
 Qed.
 
-Lemma possible_types_closure_record: forall n Gs s x T ds U,
-  wf_sto Gs s ->
+Lemma possible_types_closure_record: forall G s x T ds U,
+  wf_sto G s ->
   binds x (val_new T ds) s ->
-  record_sub (open_typ (in_sto x) T) U ->
-  possible_types n Gs x (val_new T ds) U.
+  record_sub (open_typ x T) U ->
+  possible_types G x (val_new T ds) U.
 Proof.
   introv Hwf Bis Hsub.
-  apply pt_has_sub with (T:=open_typ (in_sto x) T).
+  apply pt_has_sub with (T:=open_typ x T).
   intros D Hhas. eapply pt_rcd_has_piece; eauto.
   apply open_record_type. eapply record_new_typing; eauto. eapply val_new_typing; eauto.
   assumption.
 Qed.
 
-Lemma pt_monotonic: forall n Gs x v T,
-  possible_types n Gs x v T -> forall n', n <= n' ->
-  possible_types n' Gs x v T.
-Proof.
-  Hint Constructors possible_types.
-  introv Hp. inversion Hp; subst; eauto; introv LE.
-  + assert (exists n0', n' = n0' + (n0 + max n1 n2) /\ 0 <= n0') as Eq'. {
-      apply NPeano.Nat.le_exists_sub. apply LE.
-    }
-    destruct Eq' as [n0' [Eq' ?]].
-    repeat rewrite Plus.plus_assoc in Eq'.
-    subst.
-    eapply pt_and; eauto.
-  + assert (exists n0', n' = n0' + (n0 + n1) /\ 0 <= n0') as Eq'. {
-      apply NPeano.Nat.le_exists_sub. apply LE.
-    }
-    destruct Eq' as [n0' [Eq' ?]].
-    repeat rewrite Plus.plus_assoc in Eq'.
-    subst.
-    eapply pt_sel; eauto.
-  + assert (exists n0', n' = n0' + (n0 + n1 + 1) /\ 0 <= n0') as Eq'. {
-      apply NPeano.Nat.le_exists_sub. apply LE.
-    }
-    destruct Eq' as [n0' [Eq' ?]].
-    repeat rewrite Plus.plus_assoc in Eq'.
-    subst.
-    eapply pt_bnd; eauto.
-Qed.
-
-Lemma pt_monotonic0: forall n Gs x v T,
-  possible_types 0 Gs x v T ->
-  possible_types n Gs x v T.
-Proof.
-  intros. eapply pt_monotonic; eauto. omega.
-Qed.
-
-Lemma pt_and_inversion: forall n Gs s x v T1 T2,
-  wf_sto Gs s ->
+Lemma pt_and_inversion: forall G s x v T1 T2,
+  wf_sto G s ->
   binds x v s ->
-  possible_types n Gs x v (typ_and T1 T2) ->
-  possible_types n Gs x v T1 /\ possible_types n Gs x v T2.
+  possible_types G x v (typ_and T1 T2) ->
+  possible_types G x v T1 /\ possible_types G x v T2.
 Proof.
   introv Hwf Bis Hp. dependent induction Hp.
-  - assert (record_type (open_typ (in_sto x0) T)) as Htype. {
+  - assert (record_type (open_typ x0 T)) as Htype. {
       eapply open_record_type.
       eapply record_new_typing. eapply val_new_typing; eauto.
     }
     destruct (record_sub_and Htype x) as [Hsub1 Hsub2].
     split;
     eapply possible_types_closure_record; eauto.
-  - lets M1: (Max.le_max_l n1 n2).
-    lets M2: (Max.le_max_r n1 n2).
-    split;
-    eapply pt_monotonic; eauto; try omega.
+  - split; assumption.
 Qed.
 
 (*
@@ -3021,20 +2749,18 @@ Let SS = Ts(G, x, v). We first show SS is closed wrt G |-# _ <: _.
 Assume T0 in SS and G |- T0 <: U0.s We show U0 in SS by an induction on subtyping derivations of G |-# T0 <: U0.
 *)
 
-Lemma possible_types_closure_tight_zero: forall n Gs s x v T0 U0,
-  wf_sto Gs s ->
+Lemma possible_types_closure_tight: forall G s x v T0 U0,
+  wf_sto G s ->
   binds x v s ->
-  possible_types 0 Gs x v T0 ->
-  subtyp (ty_tight n) Gs empty T0 U0 ->
-  possible_types 0 Gs x v U0.
+  possible_types G x v T0 ->
+  subtyp ty_general sub_tight G T0 U0 ->
+  possible_types G x v U0.
 Proof.
-  introv Hwf Bis HT0 Hsub; dependent induction Hsub;
-  assert (@empty typ ~= @empty typ) as HE by reflexivity.
-
+  introv Hwf Bis HT0 Hsub. dependent induction Hsub.
   - (* Top *) apply pt_top.
   - (* Bot *) inversion HT0; subst.
-    lets Htype: (open_record_type (in_sto x) (record_new_typing (val_new_typing Hwf Bis))).
-    destruct Htype as [ls Htyp]. rewrite H5 in Htyp. inversion Htyp.
+    lets Htype: (open_record_type x (record_new_typing (val_new_typing Hwf Bis))).
+    destruct Htype as [ls Htyp]. rewrite H3 in Htyp. inversion Htyp.
   - (* Refl-<: *) assumption.
   - (* Trans-<: *)
     apply IHHsub2; try assumption.
@@ -3048,7 +2774,6 @@ Proof.
     destruct HT0 as [HT HU].
     assumption.
   - (* <:-And *)
-    rewrite <- (max_and 0).
     apply pt_and. apply IHHsub1; assumption. apply IHHsub2; assumption.
   - (* Fld-<:-Fld *)
     apply pt_rcd_trm_inversion with (s:=s) in HT0; eauto.
@@ -3057,9 +2782,9 @@ Proof.
     eapply pt_rcd_trm.
     eassumption.
     apply ty_sub with (T:=T).
-    intro Contra. false.
+    intro Contra. inversion Contra.
     assumption.
-    eapply tight_to_general_subtyping. eassumption.
+    apply tight_to_general_subtyping. assumption.
   - (* Typ-<:-Typ *)
     apply pt_rcd_typ_inversion with (s:=s) in HT0; eauto.
     destruct HT0 as [T [ds [T' [Heq [Hhas [Hsub1' Hsub2']]]]]].
@@ -3068,60 +2793,34 @@ Proof.
     eassumption.
     eapply subtyp_trans. eapply tight_to_general_subtyping. eassumption. eassumption.
     eapply subtyp_trans. eassumption. eapply tight_to_general_subtyping. eassumption.
-  - (* <:-Sel *)
-    inversion H0; subst. false. eapply empty_middle_inv. eassumption.
-  - (* Sel-<: *)
-    inversion H0; subst. false. eapply empty_middle_inv. eassumption.
-  - (* <:-Sel sto *)
-    destruct H0 as [[Contra ?] | [? ?]]. inversion Contra. subst.
-    assert (S = T) as B. {
-      eapply tight_bounds_eq; eauto.
-    }
-    subst.
-    rewrite <- (LibNat.plus_zero_l 0).
+  - (* <:-Sel-tight *)
     eapply pt_sel. eassumption. assumption.
-  - (* Sel-<: sto *)
-    destruct H0 as [[Contra ?] | [? ?]]. inversion Contra. subst.
+  - (* Sel-<:-tight *)
     inversion HT0; subst.
-    assert (record_type (open_typ (in_sto x) T0)) as B. {
+    assert (record_type (open_typ x T0)) as B. {
       eapply record_type_new; eassumption.
     }
-    rewrite H7 in B. destruct B as [? B]. inversion B.
-    assert (S = T) as B. {
-      eapply tight_bounds_eq; eauto.
-    }
-    subst.
-    assert (S0 = T) as B. {
+    rewrite H4 in B. destruct B as [? B]. inversion B.
+    assert (T = S) as B. {
       eapply unique_tight_bounds; eauto.
     }
-    subst.
-    eapply pt_monotonic; eauto; try omega.
+    subst. assumption.
   - (* All-<:-All *)
     inversion HT0; subst.
-    assert (record_type (open_typ (in_sto x) T)) as B. {
+    assert (record_type (open_typ x T)) as B. {
       eapply record_type_new; eassumption.
     }
-    rewrite H7 in B. destruct B as [? B]. inversion B.
+    rewrite H5 in B. destruct B as [? B]. inversion B.
     apply_fresh pt_lambda as y.
-    eapply H4; eauto.
-    eapply subtyp_trans. eassumption. eassumption.
-    assert (y ~ S2 = empty & (y ~ S2)) as C. {
-      rewrite concat_empty_l. eauto.
-    }
+    eapply H3; eauto.
+    eapply subtyp_trans. eapply tight_to_general_subtyping. eassumption. eassumption.
     eapply subtyp_trans.
-    eapply narrow_subtyping. eapply H10; eauto.
-    eapply subenv_last_only. eapply Hsub.
-    rewrite <- concat_empty_l. eapply ok_push; eauto.
-    rewrite C. eauto.
-  - (* Rec-<:-Rec *)
-    inversion HT0; subst.
-    assert (record_type (open_typ (in_sto x) T)) as B. {
-      eapply record_type_new; eassumption.
-    }
-    rewrite H7 in B. destruct B as [? B]. inversion B.
-    omega.
+    eapply narrow_subtyping. eapply H8; eauto.
+    eapply subenv_last. eapply tight_to_general_subtyping. eapply Hsub.
+    eapply ok_push. eapply wf_sto_to_ok_G. eassumption. eauto.
+    eapply ok_push. eapply wf_sto_to_ok_G. eassumption. eauto.
+    eapply H; eauto.
 Qed.
-
 
 (*
 Lemma (Possible types completeness for values)
@@ -3129,44 +2828,23 @@ Lemma (Possible types completeness for values)
 If `G ~ s` and `x = v in s` and  `G |-! v: T` then `T in Ts(G, x, v)`.
  *)
 
-Lemma possible_types_completeness_for_values: forall Gs s x v T,
-  wf_sto Gs s ->
+Lemma possible_types_completeness_for_values: forall G s x v T,
+  wf_sto G s ->
   binds x v s ->
-  ty_trm ty_precise Gs empty (trm_val v) T ->
-  possible_types 1 Gs x v T.
+  ty_trm ty_precise sub_general G (trm_val v) T ->
+  possible_types G x v T.
 Proof.
   introv Hwf Bis Hty. destruct v as [S ds | S t].
   - apply new_intro_inversion in Hty. destruct Hty as [Heq Htype]. subst.
-    assert (0+0+1=1) as B by omega. rewrite <- B.
     eapply pt_bnd. eapply pt_new. reflexivity.
   - remember Hty as Hty'. clear HeqHty'. inversion Hty'; subst.
     + apply all_intro_inversion in Hty. destruct Hty as [T' Heq]. subst.
       apply_fresh pt_lambda as y.
-      assert (y ~ S = empty & y ~ S) as A. {
-        rewrite concat_empty_l. reflexivity.
-      }
-      rewrite A. eapply H5; eauto.
-      apply subtyp_refl. discriminate.
-      apply subtyp_refl. discriminate.
-    + assert (ty_precise <> ty_general) as Neqm by discriminate.
-      specialize (H Neqm). destruct H. inversion H.
-Qed.
-
-Lemma bound__precise: forall Gs s x v T,
-  wf_sto Gs s ->
-  binds x v s ->
-  binds x T Gs ->
-  ty_trm ty_precise Gs empty (trm_val v) T.
-Proof.
-  introv Hwf Bis Bi.
-  assert (ty_trm ty_precise Gs empty (trm_val v) T) as A. {
-    destruct (ctx_binds_to_sto_binds_raw Hwf Bi) as [? [? [? [? [Bis' ?]]]]]; eauto.
-    unfold binds in *. rewrite Bis' in *. inversions Bis.
-    rewrite <- concat_assoc.
-    eapply weaken_sto_ty_trm. assumption.
-    rewrite concat_assoc. eapply wf_sto_to_ok_G. eassumption.
-  }
-  apply A.
+      eapply H5; eauto.
+      apply subtyp_refl.
+      apply subtyp_refl.
+    + assert (ty_precise = ty_precise) as Heqm1 by reflexivity.
+      specialize (H Heqm1). destruct H. inversion H.
 Qed.
 
 (*
@@ -3180,243 +2858,130 @@ If `G ~ s` and `G |- x: T` then, for some value `v`,
 `s(x) = v` and `T in Ts(G, x, v)`.
 *)
 
-Ltac inv_eq :=
-  match goal with
-  | H: _ = _ |- _ => unfold avar_s in H; inversions H
-  end.
-
-Lemma possible_types_closure_tight_rules: forall l,
-  (forall m Gs G t T, ty_trm m Gs G t T -> forall n s x v, n < l ->
-   G = empty ->
-   m = ty_tight n ->
-   wf_sto Gs s ->
-   binds x v s ->
-   t = trm_var (avar_s x) ->
-   possible_types (S n) Gs x v T
-  ) /\
-  (forall m Gs G T U, subtyp m Gs G T U -> forall n s x v, n < l  ->
-   G = empty ->
-   m = ty_tight n ->
-   wf_sto Gs s ->
-   binds x v s ->
-   possible_types (S n) Gs x v T ->
-   possible_types (S n) Gs x v U).
-Proof.
-  intros l. induction l. split; introv H LE; omega.
-  apply ts_mutind; intros; subst; eauto 4; try solve [false].
-  - inv_eq.
-    eapply pt_monotonic. eapply possible_types_completeness_for_values; eauto.
-    eapply bound__precise; eauto.
-    omega.
-  - inv_eq. inv_eq.
-    assert (0+(S n)+1=S (S n)) as A by omega. rewrite <- A.
-    eapply pt_bnd. eapply H; eauto.
-    omega. reflexivity.
-  - inv_eq.
-    assert (possible_types (S n) Gs x0 v (typ_bnd T)) as Hp. {
-      eapply H; eauto.
-    }
-    inversion Hp; subst.
-    + lets Htype: (record_type_new H3 H4). rewrite H8 in Htype. inversion Htype. inversion H1.
-    + eapply pt_monotonic. eassumption. omega.
-  - assert (possible_types (S n0) Gs x0 v T) as Hp1 by solve [eapply H; eauto].
-    assert (possible_types (S n0) Gs x0 v U) as Hp2 by solve [eapply H0; eauto].
-    rewrite <- (max_and (S n0)). apply pt_and; assumption.
-  - inv_eq. apply pt_monotonic with (n:=S n1). eapply H; eauto. omega. omega.
-
-  - (* Bot *) inversion H4; subst.
-    lets Htype: (open_record_type (in_sto x) (record_new_typing (val_new_typing H2 H3))).
-    destruct Htype as [ls Htyp]. rewrite H8 in Htyp. inversion Htyp.
-  - (* And-<: *)
-    eapply pt_and_inversion in H4; eauto.
-    destruct H4 as [HT HU].
-    assumption.
-  - (* And-<: *)
-    eapply pt_and_inversion in H4; eauto.
-    destruct H4 as [HT HU].
-    assumption.
-  - (* <:-And *)
-    rewrite <- (max_and (Datatypes.S n0)).
-    apply pt_and; eauto.
-  - (* Fld-<:-Fld *)
-    eapply pt_rcd_trm_inversion in H5; eauto.
-    destruct H5 as [S [ds [t [Heq [Hhas Hty]]]]].
-    subst.
-    eapply pt_rcd_trm.
-    eassumption.
-    apply ty_sub with (T:=T).
-    intro Contra. false.
-    assumption.
-    eapply tight_to_general_subtyping. eauto.
-  - (* Typ-<:-Typ *)
-    eapply pt_rcd_typ_inversion in H6; eauto.
-    destruct H6 as [T [ds [T' [Heq [Hhas [Hsub1' Hsub2']]]]]].
-    subst.
-    eapply pt_rcd_typ.
-    eassumption.
-    eapply subtyp_trans. eapply tight_to_general_subtyping. eassumption. eassumption.
-    eapply subtyp_trans. eassumption. eapply tight_to_general_subtyping. eassumption.
-  - (* <:-Sel *)
-    inversion r; subst. false. eapply empty_middle_inv. eassumption.
-  - (* Sel-<: *)
-    inversion r; subst. false. eapply empty_middle_inv. eassumption.
-  - (* <:-Sel sto *)
-    destruct o as [[Contra ?] | [? ?]]. inversion Contra. subst.
-    assert (S = T) as B. {
-      eapply tight_bounds_eq; eauto.
-    }
-    subst.
-    rewrite <- (LibNat.plus_zero_l (S n0)).
-    eapply pt_sel. eassumption. assumption.
-  - (* Sel-<: sto *)
-    destruct o as [[Contra ?] | [? ?]]. inversion Contra. subst.
-    inversion H5; subst.
-    assert (record_type (open_typ (in_sto x0) T0)) as B. {
-      eapply record_type_new; eassumption.
-    }
-    rewrite H10 in B. destruct B as [? B]. inversion B.
-    assert (S = T) as B. {
-      eapply tight_bounds_eq; eauto.
-    }
-    subst.
-    assert (S0 = T) as B. {
-      eapply unique_tight_bounds; eauto.
-    }
-    subst.
-    eapply pt_monotonic; eauto; try omega.
-  - (* All-<:-All *)
-    inversion H6; subst.
-    assert (record_type (open_typ (in_sto x) T)) as B. {
-      eapply record_type_new; eassumption.
-    }
-    rewrite H10 in B. destruct B as [? B]. inversion B.
-    apply_fresh pt_lambda as y.
-    eapply H7; eauto.
-    eapply subtyp_trans. eassumption. eassumption.
-    assert (y ~ S2 = empty & (y ~ S2)) as C. {
-      rewrite concat_empty_l. eauto.
-    }
-    eapply subtyp_trans.
-    eapply narrow_subtyping. eapply H13; eauto.
-    eapply subenv_last_only. eauto.
-    rewrite <- concat_empty_l. eapply ok_push; eauto.
-    rewrite C. eauto.
-  - (* Rec-<:-Rec *)
-    inversion H5; subst.
-    assert (record_type (open_typ (in_sto x) T)) as B. {
-      eapply record_type_new; eassumption.
-    }
-    rewrite H9 in B. destruct B as [? B]. inversion B.
-    pick_fresh z. assert (z \notin L) as FrL by auto.
-    specialize (s z FrL).
-    assert (n1 + n2 = n0) as C. {
-      omega.
-    }
-    assert (subtyp (ty_tight (pred n0)) Gs empty (open_typ (in_sto x) T1) (open_typ (in_sto x) T2)) as Hsub by admit.
-    assert (possible_types n0 Gs x v (open_typ (in_sto x) T2)) as Hp. {
-      destruct n0.
-      + assert (n2=0) by omega. subst.
-        eapply possible_types_closure_tight_zero with (n:=0) (T0:=(open_typ (in_sto x) T1)); try eassumption.
-      + eapply (proj2 IHl). eapply Hsub. omega. reflexivity. simpl. reflexivity.
-        eassumption. eassumption. eapply pt_monotonic. eassumption. omega.
-    }
-    rewrite C. rewrite <- (LibNat.plus_zero_l n0).
-    eapply pt_bnd. eapply Hp. reflexivity.
-Qed.
-
-Lemma possible_types_closure_tight: forall n Gs s x v T0 U0,
-  wf_sto Gs s ->
-  binds x v s ->
-  possible_types (S n) Gs x v T0 ->
-  subtyp (ty_tight n) Gs empty T0 U0 ->
-  possible_types (S n) Gs x v U0.
-Proof.
-  introv Hwf Bis Hpt Hsub.
-  eapply possible_types_closure_tight_rules.
-  eapply Hsub.
-  reflexivity. reflexivity.
-  eapply Hwf.
-  eapply Bis.
-  eapply Hpt.
-Qed.
-
-Lemma possible_types_completeness_tight: forall Gs s x T,
-  wf_sto Gs s ->
-  ty_trm ty_tight Gs empty (trm_var (avar_s x)) T ->
-  exists v, binds x v s /\ exists n, possible_types n Gs x v T.
+Lemma possible_types_completeness_tight: forall G s x T,
+  wf_sto G s ->
+  ty_trm ty_general sub_tight G (trm_var (avar_f x)) T ->
+  exists v, binds x v s /\ possible_types G x v T.
 Proof.
   introv Hwf H. dependent induction H.
-  - assert (exists v, binds x v s /\ ty_trm ty_precise Gs empty (trm_val v) T) as A. {
+  - assert (exists v, binds x v s /\ ty_trm ty_precise sub_general G (trm_val v) T) as A. {
       destruct (ctx_binds_to_sto_binds_raw Hwf H) as [G1 [? [v [? [Bi Hty]]]]].
       exists v. split. apply Bi. subst. rewrite <- concat_assoc.
-      eapply weaken_sto_ty_trm. assumption.
-      rewrite concat_assoc. eapply wf_sto_to_ok_G. eassumption.
+      eapply weaken_ty_trm. assumption. rewrite concat_assoc.
+      eapply wf_sto_to_ok_G. eassumption.
     }
     destruct A as [v [Bis Hty]].
-    exists v. split. apply Bis.
-    exists 1. eapply possible_types_completeness_for_values; eauto.
-  - specialize (IHty_trm x Hwf).
+    exists v. split. apply Bis. eapply possible_types_completeness_for_values; eauto.
+  - specialize (IHty_trm Hwf).
     destruct IHty_trm as [v [Bis Hp]].
-    eauto. eauto.
-    exists v. split. assumption.
-    destruct Hp as [n1 Hp].
-    exists (0+n1+1). eapply pt_bnd. eapply Hp. reflexivity.
-  - specialize (IHty_trm x Hwf).
-    destruct IHty_trm as [v [Bis Hp]]; eauto.
-    exists v. split. assumption.
-    destruct Hp as [n1 Hp].
-    inversion Hp; subst.
-    + lets Htype: (record_type_new Hwf Bis). rewrite H5 in Htype. inversion Htype. inversion H0.
-    + eexists. eassumption.
-  - specialize (IHty_trm1 x Hwf). destruct IHty_trm1 as [v [Bis1 Hp1]]; eauto.
-    specialize (IHty_trm2 x Hwf). destruct IHty_trm2 as [v' [Bis2 Hp2]]; eauto.
+    exists v. split. assumption. eapply pt_bnd. eapply Hp. reflexivity.
+  - specialize (IHty_trm Hwf).
+    destruct IHty_trm as [v [Bis Hp]].
+    exists v. split. assumption. inversion Hp; subst.
+    + lets Htype: (record_type_new Hwf Bis). rewrite H4 in Htype. inversion Htype. inversion H0.
+    + assumption.
+  - specialize (IHty_trm1 Hwf). destruct IHty_trm1 as [v [Bis1 Hp1]].
+    specialize (IHty_trm2 Hwf). destruct IHty_trm2 as [v' [Bis2 Hp2]].
     unfold binds in Bis1. unfold binds in Bis2. rewrite Bis2 in Bis1. inversions Bis1.
-    exists v. split. eauto.
-    destruct Hp1 as [n1 Hp1]. destruct Hp2 as [n2 Hp2].
-    exists (0+max n1 n2). apply pt_and; assumption.
-  - specialize (IHty_trm x Hwf). destruct IHty_trm as [v [Bis Hp]]; eauto.
-    exists v. split. apply Bis.
-    destruct Hp as [n1 Hp].
-    exists n1. eapply possible_types_closure_tight; eauto.
+    exists v. split. eauto. apply pt_and; assumption.
+  - specialize (IHty_trm Hwf). destruct IHty_trm as [v [Bis Hp]].
+    exists v. split. apply Bis. eapply possible_types_closure_tight; eauto.
 Qed.
 
-Lemma tight_ty_rcd_typ__new: forall Gs s x A S U,
-  wf_sto Gs s ->
-  ty_trm ty_tight Gs empty (trm_var (avar_s x)) (typ_rcd (dec_typ A S U)) ->
+Lemma tight_ty_rcd_typ__new: forall G s x A S U,
+  wf_sto G s ->
+  ty_trm ty_general sub_tight G (trm_var (avar_f x)) (typ_rcd (dec_typ A S U)) ->
   exists T ds, binds x (val_new T ds) s.
 Proof.
   introv Hwf Hty.
   destruct (possible_types_completeness_tight Hwf Hty) as [v [Bis Hpt]].
-  destruct Hpt as [n1 Hpt].
   inversion Hpt; subst; repeat eexists; eauto.
 Qed.
 
-Lemma possible_types_closure: forall n Gs s x v S T,
-  wf_sto Gs s ->
+
+Lemma general_to_tight: forall G0 s0,
+  wf_sto G0 s0 ->
+  (forall m1 m2 G t T,
+     ty_trm m1 m2 G t T ->
+     G = G0 ->
+     m1 = ty_general ->
+     m2 = sub_general ->
+     ty_trm ty_general sub_tight G t T) /\
+  (forall m1 m2 G S U,
+     subtyp m1 m2 G S U ->
+     G = G0 ->
+     m1 = ty_general ->
+     m2 = sub_general ->
+     subtyp ty_general sub_tight G S U).
+Proof.
+  intros G0 s0 Hwf.
+  apply ts_mutind; intros; subst; eauto.
+  - assert (exists S ds, binds x (val_new S ds) s0) as Bis. {
+      eapply tight_ty_rcd_typ__new; eauto.
+    }
+    destruct Bis as [? [? Bis]].
+    eapply proj2. eapply tight_bound_completeness; eauto.
+  - assert (exists S ds, binds x (val_new S ds) s0) as Bis. {
+      eapply tight_ty_rcd_typ__new; eauto.
+    }
+    destruct Bis as [? [? Bis]].
+    eapply proj1. eapply tight_bound_completeness; eauto.
+Qed.
+
+Lemma general_to_tight_subtyping: forall G s S U,
+   wf_sto G s ->
+  subtyp ty_general sub_general G S U ->
+  subtyp ty_general sub_tight G S U.
+Proof.
+  intros. apply* general_to_tight.
+Qed.
+
+Lemma possible_types_closure: forall G s x v S T,
+  wf_sto G s ->
   binds x v s ->
-  possible_types n Gs x v S ->
-  subtyp ty_general Gs empty S T ->
-  possible_types n Gs x v T.
+  possible_types G x v S ->
+  subtyp ty_general sub_general G S T ->
+  possible_types G x v T.
 Proof.
   intros. eapply possible_types_closure_tight; eauto.
-  admit.
+  eapply general_to_tight_subtyping; eauto.
 Qed.
 
-Lemma possible_types_completeness: forall Gs s x T,
-  wf_sto Gs s ->
-  ty_trm ty_general Gs empty (trm_var (avar_s x)) T ->
-  exists v, binds x v s /\ exists n, possible_types n Gs x v T.
+Lemma possible_types_completeness: forall G s x T,
+  wf_sto G s ->
+  ty_trm ty_general sub_general G (trm_var (avar_f x)) T ->
+  exists v, binds x v s /\ possible_types G x v T.
 Proof.
-  intros.
-  eapply possible_types_completeness_tight; eauto.
-  admit.
+  introv Hwf H. dependent induction H.
+  - assert (exists v, binds x v s /\ ty_trm ty_precise sub_general G (trm_val v) T) as A. {
+      destruct (ctx_binds_to_sto_binds_raw Hwf H) as [G1 [? [v [? [Bi Hty]]]]].
+      exists v. split. apply Bi. subst. rewrite <- concat_assoc.
+      eapply weaken_ty_trm. assumption. rewrite concat_assoc.
+      eapply wf_sto_to_ok_G. eassumption.
+    }
+    destruct A as [v [Bis Hty]].
+    exists v. split. apply Bis. eapply possible_types_completeness_for_values; eauto.
+  - specialize (IHty_trm Hwf).
+    destruct IHty_trm as [v [Bis Hp]].
+    exists v. split. assumption. eapply pt_bnd. eapply Hp. reflexivity.
+  - specialize (IHty_trm Hwf).
+    destruct IHty_trm as [v [Bis Hp]].
+    exists v. split. assumption. inversion Hp; subst.
+    + lets Htype: (record_type_new Hwf Bis). rewrite H4 in Htype. inversion Htype. inversion H0.
+    + assumption.
+  - specialize (IHty_trm1 Hwf). destruct IHty_trm1 as [v [Bis1 Hp1]].
+    specialize (IHty_trm2 Hwf). destruct IHty_trm2 as [v' [Bis2 Hp2]].
+    unfold binds in Bis1. unfold binds in Bis2. rewrite Bis2 in Bis1. inversions Bis1.
+    exists v. split. eauto. apply pt_and; assumption.
+  - specialize (IHty_trm Hwf). destruct IHty_trm as [v [Bis Hp]].
+    exists v. split. apply Bis. eapply possible_types_closure; eauto.
 Qed.
 
-Lemma possible_types_lemma: forall Gs s x v T,
-  wf_sto Gs s ->
+Lemma possible_types_lemma: forall G s x v T,
+  wf_sto G s ->
   binds x v s ->
-  ty_trm ty_general Gs empty (trm_var (avar_s x)) T ->
-  exists n, possible_types n Gs x v T.
+  ty_trm ty_general sub_general G (trm_var (avar_f x)) T ->
+  possible_types G x v T.
 Proof.
   introv Hwf Bis Hty.
   lets A: (possible_types_completeness Hwf Hty).
@@ -3425,49 +2990,49 @@ Proof.
   assumption.
 Qed.
 
-Lemma ctx_binds_to_sto_binds_typing: forall Gs s x T,
-  wf_sto Gs s ->
-  binds x T Gs ->
-  exists v, binds x v s /\ ty_trm ty_precise Gs empty (trm_val v) T.
+Lemma ctx_binds_to_sto_binds_typing: forall G s x T,
+  wf_sto G s ->
+  binds x T G ->
+  exists v, binds x v s /\ ty_trm ty_precise sub_general G (trm_val v) T.
 Proof.
   introv Hwf Bi.
   lets A: (ctx_binds_to_sto_binds_raw Hwf Bi).
   destruct A as [G1 [G2 [v [HeqG [Bis Hty]]]]].
   exists v. split; eauto.
   subst. rewrite <- concat_assoc.
-  inversion Hwf; subst.
-  apply binds_empty_inv in Bis. inversion Bis.
-  eapply weaken_sto_ty_trm. assumption.
-  rewrite concat_assoc. eapply wf_sto_to_ok_G. eassumption.
+  apply weaken_ty_trm; eauto.
+  rewrite concat_assoc.
+  eapply wf_sto_to_ok_G; eauto.
 Qed.
 
 (*
 Lemma (Canonical forms 1)
 If G ~ s and G |- x: all(x: T)U then s(x) = lambda(x: T')t where G |- T <: T' and G, x: T |- t: U.
  *)
-Lemma canonical_forms_1: forall Gs s x T U,
-  wf_sto Gs s ->
-  ty_trm ty_general Gs empty (trm_var (avar_s x)) (typ_all T U) ->
-  (exists L T' t, binds x (val_lambda T' t) s /\ subtyp ty_general Gs empty T T' /\
-  (forall y, y \notin L -> ty_trm ty_general Gs (y ~ T) (open_trm (in_ctx y) t) (open_typ (in_ctx y) U))).
+Lemma canonical_forms_1: forall G s x T U,
+  wf_sto G s ->
+  ty_trm ty_general sub_general G (trm_var (avar_f x)) (typ_all T U) ->
+  (exists L T' t, binds x (val_lambda T' t) s /\ subtyp ty_general sub_general G T T' /\
+  (forall y, y \notin L -> ty_trm ty_general sub_general (G & y ~ T) (open_trm y t) (open_typ y U))).
 Proof.
   introv Hwf Hty.
-  lets Bi: (typing_implies_sto_bound Hty). destruct Bi as [S Bi].
+  lets Bi: (typing_implies_bound Hty). destruct Bi as [S Bi].
   lets A: (ctx_binds_to_sto_binds_typing Hwf Bi). destruct A as [v [Bis Htyv]].
-  lets Hp: (possible_types_lemma Hwf Bis Hty). destruct Hp as [n1 Hp].
+  lets Hp: (possible_types_lemma Hwf Bis Hty).
   inversion Hp; subst.
-  - lets Htype: (record_type_new Hwf Bis). rewrite H4 in Htype.
+  - lets Htype: (record_type_new Hwf Bis). rewrite H3 in Htype.
     destruct Htype as [ls Htyp]. inversion Htyp.
-  - pick_fresh y. exists (dom Gs \u L). exists S0. exists t.
+  - pick_fresh y. exists (dom G \u L). exists S0. exists t.
     split. apply Bis. split. assumption.
     intros y0 Fr0.
     eapply ty_sub.
-    intros Contra. false.
+    intros Contra. inversion Contra.
     eapply narrow_typing.
     eapply H1; eauto.
-    apply subenv_last_only. apply H6.
-    rewrite <- concat_empty_l. apply ok_push; eauto.
-    eapply H7; eauto.
+    apply subenv_last. apply H5.
+    apply ok_push. eapply wf_sto_to_ok_G; eauto. eauto.
+    apply ok_push. eapply wf_sto_to_ok_G; eauto. eauto.
+    eapply H6; eauto.
 Qed.
 
 (*
@@ -3476,15 +3041,15 @@ Lemma (Canonical forms 2)
 If G ~ s and G |- x: {a: T} then s(x) = new(x: S)d for some type S, definition d such that G |- d: S and d contains a definition {a = t} where G |- t: T.
 
 *)
-Lemma canonical_forms_2: forall Gs s x a T,
-  wf_sto Gs s ->
-  ty_trm ty_general Gs empty (trm_var (avar_s x)) (typ_rcd (dec_trm a T)) ->
-  (exists S ds t, binds x (val_new S ds) s /\ ty_defs Gs empty (open_defs (in_sto x) ds) (open_typ (in_sto x) S) /\ defs_has (open_defs (in_sto x) ds) (def_trm a t) /\ ty_trm ty_general Gs empty t T).
+Lemma canonical_forms_2: forall G s x a T,
+  wf_sto G s ->
+  ty_trm ty_general sub_general G (trm_var (avar_f x)) (typ_rcd (dec_trm a T)) ->
+  (exists S ds t, binds x (val_new S ds) s /\ ty_defs G (open_defs x ds) (open_typ x S) /\ defs_has (open_defs x ds) (def_trm a t) /\ ty_trm ty_general sub_general G t T).
 Proof.
   introv Hwf Hty.
-  lets Bi: (typing_implies_sto_bound Hty). destruct Bi as [S Bi].
+  lets Bi: (typing_implies_bound Hty). destruct Bi as [S Bi].
   lets A: (ctx_binds_to_sto_binds_typing Hwf Bi). destruct A as [v [Bis Htyv]].
-  lets Hp: (possible_types_lemma Hwf Bis Hty). destruct Hp as [n1 Hp].
+  lets Hp: (possible_types_lemma Hwf Bis Hty).
   apply pt_rcd_trm_inversion with (s:=s) in Hp; eauto.
   destruct Hp as [S' [ds [t' [Heq [Hdefs Htyd]]]]].
   subst.
@@ -3496,32 +3061,24 @@ Qed.
 (* ###################################################################### *)
 (** * Misc *)
 
-Lemma var_typing_implies_avar_f: forall Gs G a T,
-  ty_trm ty_general Gs G (trm_var a) T ->
+Lemma var_typing_implies_avar_f: forall G a T,
+  ty_trm ty_general sub_general G (trm_var a) T ->
   exists x, a = avar_f x.
 Proof.
   intros. dependent induction H; try solve [eexists; reflexivity].
   apply IHty_trm.
 Qed.
 
-Lemma var_typing_implies_avar_s: forall Gs v T,
-  ty_trm ty_general Gs empty (trm_var (avar_f v)) T ->
-  avar_f v = avar_s (var_of v).
-Proof.
-  intros. dependent induction H; eauto.
-  false. apply* binds_empty_inv.
-Qed.
-
-Lemma val_typing: forall Gs G v T,
-  ty_trm ty_general Gs G (trm_val v) T ->
-  exists T', ty_trm ty_precise Gs G (trm_val v) T' /\
-             subtyp ty_general Gs G T' T.
+Lemma val_typing: forall G v T,
+  ty_trm ty_general sub_general G (trm_val v) T ->
+  exists T', ty_trm ty_precise sub_general G (trm_val v) T' /\
+             subtyp ty_general sub_general G T' T.
 Proof.
   intros. dependent induction H.
   - exists (typ_all T U). split.
-    apply ty_all_intro with (L:=L); eauto. apply subtyp_refl. discriminate.
+    apply ty_all_intro with (L:=L); eauto. apply subtyp_refl.
   - exists (typ_bnd T). split.
-    apply ty_new_intro with (L:=L); eauto. apply subtyp_refl. discriminate.
+    apply ty_new_intro with (L:=L); eauto. apply subtyp_refl.
   - destruct IHty_trm as [T' [Hty Hsub]].
     exists T'. split; eauto.
 Qed.
@@ -3545,18 +3102,14 @@ The proof is by a induction on typing derivations of G |- t: T.
 
 Lemma safety: forall G s t T,
   wf_sto G s ->
-  ty_trm ty_general G empty t T ->
-  (normal_form t \/ (exists s' t' G' G'', red t s t' s' /\ G' = G & G'' /\ ty_trm ty_general G' empty t' T /\ wf_sto G' s')).
+  ty_trm ty_general sub_general G t T ->
+  (normal_form t \/ (exists s' t' G' G'', red t s t' s' /\ G' = G & G'' /\ ty_trm ty_general sub_general G' t' T /\ wf_sto G' s')).
 Proof.
   introv Hwf H. dependent induction H; try solve [left; eauto].
   - (* All-E *) right.
-    lets Ax: (var_typing_implies_avar_s H).
-    lets Az: (var_typing_implies_avar_s H0).
-    rewrite Ax in H. rewrite Ax. rewrite Az.
-    destruct z as [vz | vz]. simpl.
     lets C: (canonical_forms_1 Hwf H).
     destruct C as [L [T' [t [Bis [Hsub Hty]]]]].
-    exists s (open_trm (in_sto vz) t) Gs (@empty typ).
+    exists s (open_trm z t) G (@empty typ).
     split.
     apply red_app with (T:=T'). assumption.
     split.
@@ -3564,22 +3117,17 @@ Proof.
     split.
     pick_fresh y. assert (y \notin L) as FrL by auto. specialize (Hty y FrL).
     rewrite subst_intro_typ with (x:=y). rewrite subst_intro_trm with (x:=y).
-    eapply subst_ty_trm.
-    eassumption.
-    eapply Hty.
-    eauto. eauto.
+    eapply subst_ty_trm. eapply Hty.
+    apply ok_push. eapply wf_sto_to_ok_G. eassumption. eauto. eauto.
     rewrite subst_fresh_typ.
     apply ty_sub with (T:=S).
-    intro Contra. false.
+    intro Contra. inversion Contra.
     assumption. apply subtyp_refl.
-    eauto. eauto. eauto. discriminate. eauto. eauto. eauto. eauto.
-    simpl in Az. unfold avar_s in Az. inversions Az.
+    eauto. eauto. eauto. eauto.
   - (* Fld-E *) right.
-    lets Ax: (var_typing_implies_avar_s H).
-    rewrite Ax in H. rewrite Ax.
     lets C: (canonical_forms_2 Hwf H).
     destruct C as [S [ds [t [Bis [Tyds [Has Ty]]]]]].
-    exists s t Gs (@empty typ).
+    exists s t G (@empty typ).
     split.
     apply red_sel with (T:=S) (ds:=ds); try assumption.
     split.
@@ -3594,10 +3142,7 @@ Proof.
         eapply var_typing_implies_avar_f. eassumption.
       }
       destruct A as [x A]. subst a.
-      lets Ax: (var_typing_implies_avar_s H).
-      rewrite Ax in H. rewrite Ax.
-      destruct x as [vx | vx].
-      exists s (open_trm (in_sto vx) u) Gs (@empty typ).
+      exists s (open_trm x u) G (@empty typ).
       split.
       apply red_let_var.
       split.
@@ -3605,81 +3150,61 @@ Proof.
       split.
       pick_fresh y. assert (y \notin L) as FrL by auto. specialize (H0 y FrL).
       rewrite subst_intro_trm with (x:=y).
-      rewrite <- subst_fresh_typ with (x:=y) (y:=(in_sto vx)).
-      eapply subst_ty_trm.
-      eassumption.
-      rewrite concat_empty_l in H0. eapply H0.
-      eauto. eauto.
+      rewrite <- subst_fresh_typ with (x:=y) (y:=x).
+      eapply subst_ty_trm. eapply H0.
+      apply ok_push. eapply wf_sto_to_ok_G. eassumption. eauto. eauto.
       rewrite subst_fresh_typ. assumption. eauto. eauto. eauto. eauto.
-      simpl in Ax. unfold avar_s in Ax. inversions Ax.
     + lets Hv: (val_typing H).
       destruct Hv as [T' [Htyp Hsub]].
       pick_fresh x. assert (x \notin L) as FrL by auto. specialize (H0 x FrL).
-      pick_fresh y.
-      exists (s & y ~ v) (open_trm (in_sto y) u) (Gs & (y ~ T')) (y ~ T').
+      exists (s & x ~ v) (open_trm x u) (G & (x ~ T')) (x ~ T').
       split.
       apply red_let. eauto.
       split. reflexivity. split.
-      assert (subst_trm x (in_sto y) (open_trm (in_ctx x) u)=open_trm (in_sto y) u) as A. {
-        rewrite subst_open_commute_trm. simpl. rewrite If_l.
-        rewrite subst_fresh_trm.
-        reflexivity.
-        eauto. eauto.
-      }
-      rewrite <- A.
-      assert (subst_typ x (in_sto y) U=U) as B. {
-        rewrite subst_fresh_typ.
-        reflexivity. eauto.
-      }
-      rewrite <- B.
-      eapply subst_ty_trm.
-      eapply wf_sto_push. eassumption. eauto. eauto. eassumption.
-      eapply weaken_sto_ty_trm. rewrite concat_empty_l in H0. eapply H0.
-      eapply ok_push; eauto.
-      eapply fv_ctx_types_push. eauto. eauto.
-      eauto.
-      assert (subst_typ x (in_sto y) T=T) as C. {
-        rewrite subst_fresh_typ.
-        reflexivity. eauto.
-      }
-      rewrite C.
-      eapply ty_sub.
-      intros Contra. false.
-      eapply ty_var_s. eauto.
-      eapply weaken_sto_subtyp. eapply Hsub.
-      eapply ok_push; eauto.
-      eapply wf_sto_push. eassumption. eauto. eauto. eassumption.
-    + specialize (IHty_trm Hwf). destruct IHty_trm as [IH | IH]; eauto. inversion IH.
+      apply narrow_typing with (G:=G & x ~ T).
+      assumption.
+      apply subenv_last. assumption.
+      apply ok_push. eapply wf_sto_to_ok_G. eassumption. eauto.
+      apply ok_push. eapply wf_sto_to_ok_G. eassumption. eauto.
+      apply wf_sto_push. assumption. eauto. eauto. assumption.
+    + specialize (IHty_trm Hwf). destruct IHty_trm as [IH | IH]. inversion IH.
       destruct IH as [s' [t' [G' [G'' [IH1 [IH2 [IH3]]]]]]].
       exists s' (trm_let t' u) G' G''.
       split. apply red_let_tgt. assumption.
       split. assumption. split.
       apply ty_let with (L:=L \u dom G') (T:=T); eauto.
-      intros. rewrite IH2. eapply weaken_sto_ty_trm. apply H0. auto.
-      eapply wf_sto_to_ok_G. subst. eassumption. eassumption.
-    + specialize (IHty_trm Hwf). destruct IHty_trm as [IH | IH]; eauto. inversion IH.
+      intros. rewrite IH2. eapply (proj51 weaken_rules). apply H0. auto. reflexivity.
+      rewrite <- IH2. apply ok_push. eapply wf_sto_to_ok_G. eassumption. eauto.
+      rewrite IH2.
+      rewrite <- IH2. eauto.
+    + specialize (IHty_trm Hwf). destruct IHty_trm as [IH | IH]. inversion IH.
       destruct IH as [s' [t' [G' [G'' [IH1 [IH2 [IH3]]]]]]].
       exists s' (trm_let t' u) G' G''.
       split. apply red_let_tgt. assumption.
       split. assumption. split.
       apply ty_let with (L:=L \u dom G') (T:=T); eauto.
-      intros. rewrite IH2. eapply weaken_sto_ty_trm. apply H0. auto.
-      eapply wf_sto_to_ok_G. subst. eassumption. eassumption.
-    + specialize (IHty_trm Hwf). destruct IHty_trm as [IH | IH]; eauto. inversion IH.
+      intros. rewrite IH2. eapply (proj51 weaken_rules). apply H0. auto. reflexivity.
+      rewrite <- IH2. apply ok_push. eapply wf_sto_to_ok_G. eassumption. eauto.
+      rewrite IH2.
+      rewrite <- IH2. eauto.
+    + specialize (IHty_trm Hwf). destruct IHty_trm as [IH | IH]. inversion IH.
       destruct IH as [s' [t' [G' [G'' [IH1 [IH2 [IH3]]]]]]].
       exists s' (trm_let t' u) G' G''.
       split. apply red_let_tgt. assumption.
       split. assumption. split.
       apply ty_let with (L:=L \u dom G') (T:=T); eauto.
-      intros. rewrite IH2. eapply weaken_sto_ty_trm. apply H0. auto.
-      eapply wf_sto_to_ok_G. subst. eassumption. eassumption.
-  - specialize (IHty_trm Hwf). destruct IHty_trm as [IH | IH]; eauto.
+      intros. rewrite IH2. eapply (proj51 weaken_rules). apply H0. auto. reflexivity.
+      rewrite <- IH2. apply ok_push. eapply wf_sto_to_ok_G. eassumption. eauto.
+      rewrite IH2.
+      rewrite <- IH2. eauto.
+  - specialize (IHty_trm Hwf). destruct IHty_trm as [IH | IH].
+    + left. assumption.
     + right. destruct IH as [s' [t' [G' [G'' [IH1 [IH2 [IH3]]]]]]].
       exists s' t' G' G''.
       split; try split; try split; try assumption.
       apply ty_sub with (T:=T).
-      intro Contra. false.
+      intro Contra. inversion Contra.
       assumption.
-      rewrite IH2. apply weaken_sto_subtyp. assumption.
-      eapply wf_sto_to_ok_G. subst. eassumption.
+      rewrite IH2. apply weaken_subtyp. assumption.
+      rewrite <- IH2. eapply wf_sto_to_ok_G. eassumption.
 Qed.
